<https://www.ica.org/standards/RiC/ontology#AgentHierarchicalRelation>
        a       <http://www.w3.org/2002/07/owl#Class> ;
        <http://www.w3.org/2000/01/rdf-schema#comment>
                "Connects at least one Agent to at least another Agent, when the\n            first one is hierarchically superior to the second one."@en ;
        <http://www.w3.org/2000/01/rdf-schema#isDefinedBy>
                <https://www.ica.org/standards/RiC/ontology> ;
        <http://www.w3.org/2000/01/rdf-schema#label>
                "Agent Hierarchical Relation"@en ;
        <http://www.w3.org/2000/01/rdf-schema#subClassOf>
                <https://www.ica.org/standards/RiC/ontology#AgentToAgentRelation> ;
        <https://www.ica.org/standards/RiC/ontology#RiCCMCorrespondingComponent>
                "Class implementation of RiC-R045 and RiC-R045i\n            relations"@en .

<https://www.ica.org/standards/RiC/ontology#agentIsTargetOfAgentHierarchicalRelation>
        a       <http://www.w3.org/2002/07/owl#ObjectProperty> ;
        <http://www.w3.org/2000/01/rdf-schema#comment>
                "Connects one of the hierarchically inferior Agents to an Agent\n            Hierarchical Relation"@en ;
        <http://www.w3.org/2000/01/rdf-schema#domain>
                <https://www.ica.org/standards/RiC/ontology#Agent> ;
        <http://www.w3.org/2000/01/rdf-schema#isDefinedBy>
                <https://www.ica.org/standards/RiC/ontology> ;
        <http://www.w3.org/2000/01/rdf-schema#label>
                "agent is target of agent hierarchical relation "@en ;
        <http://www.w3.org/2000/01/rdf-schema#range>
                <https://www.ica.org/standards/RiC/ontology#AgentHierarchicalRelation> ;
        <http://www.w3.org/2000/01/rdf-schema#subPropertyOf>
                <https://www.ica.org/standards/RiC/ontology#agentIsConnectedToAgentRelation> , <https://www.ica.org/standards/RiC/ontology#thingIsTargetOfRelation> ;
        <http://www.w3.org/2000/01/rdf-schema#subPropertyOf>
                []  ;
        <http://www.w3.org/2000/01/rdf-schema#subPropertyOf>
                []  ;
        <http://www.w3.org/2002/07/owl#inverseOf>
                <https://www.ica.org/standards/RiC/ontology#agentHierarchicalRelationHasTarget> .

<https://www.ica.org/standards/RiC/ontology#agentHierarchicalRelationHasSource>
        a       <http://www.w3.org/2002/07/owl#ObjectProperty> ;
        <http://www.w3.org/2000/01/rdf-schema#comment>
                "Connects an Agent Hierarchical Relation to one of the\n            hierarchically superior Agents"@en ;
        <http://www.w3.org/2000/01/rdf-schema#domain>
                <https://www.ica.org/standards/RiC/ontology#AgentHierarchicalRelation> ;
        <http://www.w3.org/2000/01/rdf-schema#isDefinedBy>
                <https://www.ica.org/standards/RiC/ontology> ;
        <http://www.w3.org/2000/01/rdf-schema#label>
                "agent hierarchical relation has source "@en ;
        <http://www.w3.org/2000/01/rdf-schema#range>
                <https://www.ica.org/standards/RiC/ontology#Agent> ;
        <http://www.w3.org/2000/01/rdf-schema#subPropertyOf>
                <https://www.ica.org/standards/RiC/ontology#relationHasSource> , <https://www.ica.org/standards/RiC/ontology#agentRelationConnects> ;
        <http://www.w3.org/2000/01/rdf-schema#subPropertyOf>
                []  ;
        <http://www.w3.org/2000/01/rdf-schema#subPropertyOf>
                []  ;
        <http://www.w3.org/2002/07/owl#equivalentProperty>
                []  ;
        <http://www.w3.org/2002/07/owl#inverseOf>
                <https://www.ica.org/standards/RiC/ontology#agentIsSourceOfAgentHierarchicalRelation> .

<https://www.ica.org/standards/RiC/ontology#agentHierarchicalRelationHasTarget>
        a       <http://www.w3.org/2002/07/owl#ObjectProperty> ;
        <http://www.w3.org/2000/01/rdf-schema#comment>
                "Connects an Agent Hierarchical Relation to one of the\n            hierarchically inferior Agents"@en ;
        <http://www.w3.org/2000/01/rdf-schema#domain>
                <https://www.ica.org/standards/RiC/ontology#AgentHierarchicalRelation> ;
        <http://www.w3.org/2000/01/rdf-schema#isDefinedBy>
                <https://www.ica.org/standards/RiC/ontology> ;
        <http://www.w3.org/2000/01/rdf-schema#label>
                "agent hierarchical relation has target "@en ;
        <http://www.w3.org/2000/01/rdf-schema#range>
                <https://www.ica.org/standards/RiC/ontology#Agent> ;
        <http://www.w3.org/2000/01/rdf-schema#subPropertyOf>
                <https://www.ica.org/standards/RiC/ontology#agentRelationConnects> , <https://www.ica.org/standards/RiC/ontology#relationHasTarget> ;
        <http://www.w3.org/2000/01/rdf-schema#subPropertyOf>
                []  ;
        <http://www.w3.org/2000/01/rdf-schema#subPropertyOf>
                []  ;
        <http://www.w3.org/2002/07/owl#equivalentProperty>
                []  .

<https://www.ica.org/standards/RiC/ontology#Agent>
        a       <http://www.w3.org/2002/07/owl#Class> ;
        <http://www.w3.org/2000/01/rdf-schema#comment>
                "A Person, or Group, or an entity created by a Person or Group\n            (Mechanism), or a Position, that acts in the world."@en ;
        <http://www.w3.org/2000/01/rdf-schema#isDefinedBy>
                <https://www.ica.org/standards/RiC/ontology> ;
        <http://www.w3.org/2000/01/rdf-schema#label>
                "Agent"@en ;
        <http://www.w3.org/2000/01/rdf-schema#subClassOf>
                <https://www.ica.org/standards/RiC/ontology#Thing> ;
        <http://www.w3.org/2004/02/skos/core#scopeNote>
                "An Agent may have one or more identities; an identity is a\n            constellation of properties or relations that together “identify” the Agent. A Person or\n            Group commonly has one identity, though each also may have one or more alternative\n            identities. Such alternative identities may be shared by more than one Person or Group.\n            Alternative identities include but are not limited to pseudonyms, heteronyms, DBA (Doing\n            Business As), and trade identities. An alternative identity should not be confused with\n            a Position in a Group, for example, presidents, prime ministers, governors, popes,\n            royalty, or bishops. Nor should an alternative identity be confused with a variant name\n            or identifier of the same identity. Agent also includes entities created by a Person or\n            Group that act on behalf of the creating Agent in an autonomous or semi-autonomous\n            manner. Examples of a Mechanism include software agents, robots, and space and\n            underwater probes that generate data (records) in the course of Activity assigned to and\n            in conformance with the instructions given to them by the creating Person or\n            Group."@en ;
        <https://www.ica.org/standards/RiC/ontology#RiCCMCorrespondingComponent>
                "Corresponds to RiC-E07 (Agent\n            entity)"@en .

<https://www.ica.org/standards/RiC/ontology#agentIsSourceOfAgentHierarchicalRelation>
        a       <http://www.w3.org/2002/07/owl#ObjectProperty> ;
        <http://www.w3.org/2000/01/rdf-schema#comment>
                "Connects a hierarchically superior Agent to an Agent\n            Hierarchical Relation"@en ;
        <http://www.w3.org/2000/01/rdf-schema#domain>
                <https://www.ica.org/standards/RiC/ontology#Agent> ;
        <http://www.w3.org/2000/01/rdf-schema#isDefinedBy>
                <https://www.ica.org/standards/RiC/ontology> ;
        <http://www.w3.org/2000/01/rdf-schema#label>
                "agent is source of agent hierarchical relation "@en ;
        <http://www.w3.org/2000/01/rdf-schema#range>
                <https://www.ica.org/standards/RiC/ontology#AgentHierarchicalRelation> ;
        <http://www.w3.org/2000/01/rdf-schema#subPropertyOf>
                <https://www.ica.org/standards/RiC/ontology#thingIsSourceOfRelation> , <https://www.ica.org/standards/RiC/ontology#agentIsConnectedToAgentRelation> ;
        <http://www.w3.org/2000/01/rdf-schema#subPropertyOf>
                []  ;
        <http://www.w3.org/2000/01/rdf-schema#subPropertyOf>
                []  .
