<http://iflastandards.info/ns/fr/frbr/frbroo/F35_Nomen_Use_Statement>
        a       <http://www.w3.org/2002/07/owl#Class> ;
        <http://www.w3.org/2000/01/rdf-schema#comment>
                "This class comprises statements relating a Thema with a particular Nomen and its usage in the context of a common Complex Work realized by one or more KOS.\n"@en ;
        <http://www.w3.org/2000/01/rdf-schema#label>
                "Nomen Use Statement"@en ;
        <http://www.w3.org/2000/01/rdf-schema#subClassOf>
                <http://www.cidoc-crm.org/cidoc-crm/E29_Design_or_Procedure> , <http://iflastandards.info/ns/fr/frbr/frbroo/F2_Expression> .

<http://iflastandards.info/ns/fr/frbr/frbroo/F36_Script_Conversion>
        a       <http://www.w3.org/2002/07/owl#Class> ;
        <http://www.w3.org/2000/01/rdf-schema#comment>
                "This class comprises rule sets for converting signs or arrangements of signs from one script or type set to another.\n"@en ;
        <http://www.w3.org/2000/01/rdf-schema#label>
                "Script Conversion"@en ;
        <http://www.w3.org/2000/01/rdf-schema#subClassOf>
                <http://www.cidoc-crm.org/cidoc-crm/E29_Design_or_Procedure> .

<http://iflastandards.info/ns/fr/frbr/frbroo/R36i_is_script_conversion_used_in>
        a       <http://www.w3.org/2002/07/owl#ObjectProperty> ;
        <http://www.w3.org/2000/01/rdf-schema#comment>
                "This property associates an instance of F35 Nomen Use Statement with the instance of F12 Nomen for which it declares usage.\n"@en ;
        <http://www.w3.org/2000/01/rdf-schema#domain>
                <http://iflastandards.info/ns/fr/frbr/frbroo/F36_Script_Conversion> ;
        <http://www.w3.org/2000/01/rdf-schema#label>
                "is script conversion used in"@en ;
        <http://www.w3.org/2000/01/rdf-schema#range>
                <http://iflastandards.info/ns/fr/frbr/frbroo/F35_Nomen_Use_Statement> ;
        <http://www.w3.org/2000/01/rdf-schema#subPropertyOf>
                <http://www.w3.org/2002/07/owl#topObjectProperty> .

<http://iflastandards.info/ns/fr/frbr/frbroo/R36_uses_script_conversion>
        a       <http://www.w3.org/2002/07/owl#ObjectProperty> ;
        <http://www.w3.org/2000/01/rdf-schema#comment>
                "This property associates an instance of F35 Nomen Use Statement with the instance of F36 Script Conversion that was used to create the Nomen referred to in the Nomen Use Statement. The source of this conversion may or may not be explicitly mentioned. Is shortcut of: F35 Nomen Use Statement R17 was created by (created) F28 Expression Creation P33 used specific technique (was used by) E29 Design or Procedure.\n"@en ;
        <http://www.w3.org/2000/01/rdf-schema#domain>
                <http://iflastandards.info/ns/fr/frbr/frbroo/F35_Nomen_Use_Statement> ;
        <http://www.w3.org/2000/01/rdf-schema#label>
                "uses script conversion"@en ;
        <http://www.w3.org/2000/01/rdf-schema#range>
                <http://iflastandards.info/ns/fr/frbr/frbroo/F36_Script_Conversion> ;
        <http://www.w3.org/2000/01/rdf-schema#subPropertyOf>
                <http://www.w3.org/2002/07/owl#topObjectProperty> .
