<https://www.ica.org/standards/RiC/ontology#Thing>
        a       <http://www.w3.org/2002/07/owl#Class> ;
        <http://www.w3.org/2000/01/rdf-schema#comment>
                "Any idea, material thing, or event within the realm of human\n            experience."@en ;
        <http://www.w3.org/2000/01/rdf-schema#isDefinedBy>
                <https://www.ica.org/standards/RiC/ontology> ;
        <http://www.w3.org/2000/01/rdf-schema#label>
                "Thing"@en ;
        <http://www.w3.org/2000/01/rdf-schema#subClassOf>
                <http://www.w3.org/2002/07/owl#Thing> ;
        <http://www.w3.org/2004/02/skos/core#scopeNote>
                "Includes all RiC entities as well as any concept, material\n            thing, or event that may be the subject of a Record Resource or associated with an\n            Activity. Examples of entities not explicitly addressed in RiC includes but is not\n            limited to the following: abstract concepts; cultural movements, named periods and\n            events; named things, objects and works; legendary, mythical or fictitious figures,\n            characters or beings."@en ;
        <https://www.ica.org/standards/RiC/ontology#RiCCMCorrespondingComponent>
                "Corresponds to RiC-E01 (Thing\n            entity)"@en .

<https://www.ica.org/standards/RiC/ontology#measure>
        a       <http://www.w3.org/2002/07/owl#DatatypeProperty> ;
        <http://www.w3.org/2000/01/rdf-schema#comment>
                "The extent, quantity, amount, or degree of an entity, as\n            determined by measurement or calculation."@en ;
        <http://www.w3.org/2000/01/rdf-schema#domain>
                <https://www.ica.org/standards/RiC/ontology#Thing> ;
        <http://www.w3.org/2000/01/rdf-schema#isDefinedBy>
                <https://www.ica.org/standards/RiC/ontology> ;
        <http://www.w3.org/2000/01/rdf-schema#label>
                "measure"@en ;
        <http://www.w3.org/2000/01/rdf-schema#range>
                <http://www.w3.org/2000/01/rdf-schema#Literal> ;
        <http://www.w3.org/2000/01/rdf-schema#subPropertyOf>
                <http://www.w3.org/2002/07/owl#topDataProperty> .

<https://www.ica.org/standards/RiC/ontology#date>
        a       <http://www.w3.org/2002/07/owl#DatatypeProperty> ;
        <http://www.w3.org/2000/01/rdf-schema#comment>
                "Chronological information associated with an entity that\n            contributes to its identification and contextualization."@en ;
        <http://www.w3.org/2000/01/rdf-schema#domain>
                <https://www.ica.org/standards/RiC/ontology#Thing> ;
        <http://www.w3.org/2000/01/rdf-schema#isDefinedBy>
                <https://www.ica.org/standards/RiC/ontology> ;
        <http://www.w3.org/2000/01/rdf-schema#label>
                "date"@en ;
        <http://www.w3.org/2000/01/rdf-schema#range>
                <http://www.w3.org/2000/01/rdf-schema#Literal> ;
        <http://www.w3.org/2000/01/rdf-schema#subPropertyOf>
                <http://www.w3.org/2002/07/owl#topDataProperty> ;
        <http://www.w3.org/2004/02/skos/core#scopeNote>
                "Provided for usability reasons, like its subproperties. May be\n            deprecated and removed later on. Use only if you don't use Date classes for handling\n            dates."@en ;
        <https://www.ica.org/standards/RiC/ontology#RiCCMCorrespondingComponent>
                "Data property implementation of RiC-E18 (Date\n            entity)"@en .

<https://www.ica.org/standards/RiC/ontology#Person>
        a       <http://www.w3.org/2002/07/owl#Class> ;
        <http://www.w3.org/2000/01/rdf-schema#comment>
                "A human being with a social identity or persona."@en ;
        <http://www.w3.org/2000/01/rdf-schema#isDefinedBy>
                <https://www.ica.org/standards/RiC/ontology> ;
        <http://www.w3.org/2000/01/rdf-schema#label>
                "Person"@en ;
        <http://www.w3.org/2000/01/rdf-schema#subClassOf>
                <https://www.ica.org/standards/RiC/ontology#Agent> ;
        <http://www.w3.org/2002/07/owl#disjointWith>
                <https://www.ica.org/standards/RiC/ontology#Position> ;
        <http://www.w3.org/2004/02/skos/core#scopeNote>
                "Person is a kind of Agent. Most commonly, a human being\n            (biological person) has a single coeval social identity or persona. In everyday\n            discourse, this is the “real person.” Less common though not rare, over the course of a\n            lifetime, personae in addition to the coeval (or “original”) persona may be associated\n            with the human being. Such “alternative personae” are most often created by the original\n            person for specific purposes. Under some circumstances, an alternative persona might\n            eclipse or replace the original person (Mark Twain eclipsing Samuel Clemens; John Wayne\n            eclipsing Marion Mitchell Morrison), that is, the social (shared) alternative identity\n            becomes the predominate identity. Less common is whentwo or more persons collaborate to\n            create a shared persona. Persona shared by two or more Persons constitute a kind of\n            Group. Within the archival context, the original Person generally will be the focus of\n            the description, with alternative personae noted. Exceptionally, an alternative persona\n            may displace the coeval persona.s."@en ;
        <https://www.ica.org/standards/RiC/ontology#RiCCMCorrespondingComponent>
                "Corresponds to RiC-E08 (Person\n            entity)"@en .

<https://www.ica.org/standards/RiC/ontology#creationDate>
        a       <http://www.w3.org/2002/07/owl#DatatypeProperty> ;
        <http://www.w3.org/2000/01/rdf-schema#comment>
                "Date at which an entity was created."@en ;
        <http://www.w3.org/2000/01/rdf-schema#domain>
                <https://www.ica.org/standards/RiC/ontology#Thing> ;
        <http://www.w3.org/2000/01/rdf-schema#isDefinedBy>
                <https://www.ica.org/standards/RiC/ontology> ;
        <http://www.w3.org/2000/01/rdf-schema#label>
                "creation date"@en ;
        <http://www.w3.org/2000/01/rdf-schema#range>
                <http://www.w3.org/2000/01/rdf-schema#Literal> ;
        <http://www.w3.org/2000/01/rdf-schema#subPropertyOf>
                <https://www.ica.org/standards/RiC/ontology#beginningDate> ;
        <http://www.w3.org/2004/02/skos/core#scopeNote>
                "Provided for usability reasons. May be deprecated and removed\n            later on. Use only if you don't use Date classes for handling dates."@en ;
        <https://www.ica.org/standards/RiC/ontology#RiCCMCorrespondingComponent>
                "Data property specialized implementation of\n            RiC-E18 (Date entity)"@en .

<https://www.ica.org/standards/RiC/ontology#birthDate>
        a       <http://www.w3.org/2002/07/owl#DatatypeProperty> ;
        <http://www.w3.org/2000/01/rdf-schema#comment>
                "Date at which a Person was born."@en ;
        <http://www.w3.org/2000/01/rdf-schema#domain>
                <https://www.ica.org/standards/RiC/ontology#Person> ;
        <http://www.w3.org/2000/01/rdf-schema#isDefinedBy>
                <https://www.ica.org/standards/RiC/ontology> ;
        <http://www.w3.org/2000/01/rdf-schema#label>
                "birth date"@en ;
        <http://www.w3.org/2000/01/rdf-schema#range>
                <http://www.w3.org/2000/01/rdf-schema#Literal> ;
        <http://www.w3.org/2000/01/rdf-schema#subPropertyOf>
                <https://www.ica.org/standards/RiC/ontology#beginningDate> ;
        <http://www.w3.org/2004/02/skos/core#scopeNote>
                "Provided for usability reasons. May be deprecated and removed\n            later on. Use only if you don't use Date classes for handling dates."@en ;
        <https://www.ica.org/standards/RiC/ontology#RiCCMCorrespondingComponent>
                "Data property specialized implementation of\n            RiC-E18 (Date entity)"@en .

<https://www.ica.org/standards/RiC/ontology#height>
        a       <http://www.w3.org/2002/07/owl#DatatypeProperty> ;
        <http://www.w3.org/2000/01/rdf-schema#comment>
                "Vertical dimension of an entity."@en ;
        <http://www.w3.org/2000/01/rdf-schema#domain>
                <https://www.ica.org/standards/RiC/ontology#Thing> ;
        <http://www.w3.org/2000/01/rdf-schema#isDefinedBy>
                <https://www.ica.org/standards/RiC/ontology> ;
        <http://www.w3.org/2000/01/rdf-schema#label>
                "height"@en ;
        <http://www.w3.org/2000/01/rdf-schema#range>
                <http://www.w3.org/2000/01/rdf-schema#Literal> ;
        <http://www.w3.org/2000/01/rdf-schema#subPropertyOf>
                <https://www.ica.org/standards/RiC/ontology#measure> .

<https://www.ica.org/standards/RiC/ontology#modificationDate>
        a       <http://www.w3.org/2002/07/owl#DatatypeProperty> ;
        <http://www.w3.org/2000/01/rdf-schema#comment>
                "Date of the modification of an entity."@en ;
        <http://www.w3.org/2000/01/rdf-schema#domain>
                <https://www.ica.org/standards/RiC/ontology#Thing> ;
        <http://www.w3.org/2000/01/rdf-schema#isDefinedBy>
                <https://www.ica.org/standards/RiC/ontology> ;
        <http://www.w3.org/2000/01/rdf-schema#label>
                "modification date"@en ;
        <http://www.w3.org/2000/01/rdf-schema#range>
                <http://www.w3.org/2000/01/rdf-schema#Literal> ;
        <http://www.w3.org/2000/01/rdf-schema#subPropertyOf>
                <https://www.ica.org/standards/RiC/ontology#date> ;
        <http://www.w3.org/2004/02/skos/core#scopeNote>
                "Provided for usability reasons. May be deprecated and removed\n            later on. Use only if you don't use Date classes for handling dates."@en ;
        <https://www.ica.org/standards/RiC/ontology#RiCCMCorrespondingComponent>
                "Data property specialized implementation of\n            RiC-E18 (Date entity)"@en .

<https://www.ica.org/standards/RiC/ontology#deletionDate>
        a       <http://www.w3.org/2002/07/owl#DatatypeProperty> ;
        <http://www.w3.org/2000/01/rdf-schema#comment>
                "Date at which an entity was deleted."@en ;
        <http://www.w3.org/2000/01/rdf-schema#domain>
                <https://www.ica.org/standards/RiC/ontology#Thing> ;
        <http://www.w3.org/2000/01/rdf-schema#isDefinedBy>
                <https://www.ica.org/standards/RiC/ontology> ;
        <http://www.w3.org/2000/01/rdf-schema#label>
                "deletion date"@en ;
        <http://www.w3.org/2000/01/rdf-schema#range>
                <http://www.w3.org/2000/01/rdf-schema#Literal> ;
        <http://www.w3.org/2000/01/rdf-schema#subPropertyOf>
                <https://www.ica.org/standards/RiC/ontology#endDate> ;
        <http://www.w3.org/2004/02/skos/core#scopeNote>
                "Provided for usability reasons. May be deprecated and removed\n            later on. Use only if you don't use Date classes for handling dates."@en ;
        <https://www.ica.org/standards/RiC/ontology#RiCCMCorrespondingComponent>
                "Data property specialized implementation of\n            RiC-E18 (Date entity)"@en .

<https://www.ica.org/standards/RiC/ontology#Agent>
        a       <http://www.w3.org/2002/07/owl#Class> ;
        <http://www.w3.org/2000/01/rdf-schema#comment>
                "A Person, or Group, or an entity created by a Person or Group\n            (Mechanism), or a Position, that acts in the world."@en ;
        <http://www.w3.org/2000/01/rdf-schema#isDefinedBy>
                <https://www.ica.org/standards/RiC/ontology> ;
        <http://www.w3.org/2000/01/rdf-schema#label>
                "Agent"@en ;
        <http://www.w3.org/2000/01/rdf-schema#subClassOf>
                <https://www.ica.org/standards/RiC/ontology#Thing> ;
        <http://www.w3.org/2004/02/skos/core#scopeNote>
                "An Agent may have one or more identities; an identity is a\n            constellation of properties or relations that together “identify” the Agent. A Person or\n            Group commonly has one identity, though each also may have one or more alternative\n            identities. Such alternative identities may be shared by more than one Person or Group.\n            Alternative identities include but are not limited to pseudonyms, heteronyms, DBA (Doing\n            Business As), and trade identities. An alternative identity should not be confused with\n            a Position in a Group, for example, presidents, prime ministers, governors, popes,\n            royalty, or bishops. Nor should an alternative identity be confused with a variant name\n            or identifier of the same identity. Agent also includes entities created by a Person or\n            Group that act on behalf of the creating Agent in an autonomous or semi-autonomous\n            manner. Examples of a Mechanism include software agents, robots, and space and\n            underwater probes that generate data (records) in the course of Activity assigned to and\n            in conformance with the instructions given to them by the creating Person or\n            Group."@en ;
        <https://www.ica.org/standards/RiC/ontology#RiCCMCorrespondingComponent>
                "Corresponds to RiC-E07 (Agent\n            entity)"@en .

<https://www.ica.org/standards/RiC/ontology#width>
        a       <http://www.w3.org/2002/07/owl#DatatypeProperty> ;
        <http://www.w3.org/2000/01/rdf-schema#comment>
                "Horizontal dimension of an entity."@en ;
        <http://www.w3.org/2000/01/rdf-schema#domain>
                <https://www.ica.org/standards/RiC/ontology#Thing> ;
        <http://www.w3.org/2000/01/rdf-schema#isDefinedBy>
                <https://www.ica.org/standards/RiC/ontology> ;
        <http://www.w3.org/2000/01/rdf-schema#label>
                "width"@en ;
        <http://www.w3.org/2000/01/rdf-schema#range>
                <http://www.w3.org/2000/01/rdf-schema#Literal> ;
        <http://www.w3.org/2000/01/rdf-schema#subPropertyOf>
                <https://www.ica.org/standards/RiC/ontology#measure> .

<https://www.ica.org/standards/RiC/ontology#location>
        a       <http://www.w3.org/2002/07/owl#DatatypeProperty> ;
        <http://www.w3.org/2000/01/rdf-schema#comment>
                "A delimitation of the physical territory of a place. This\n            datatype property is used to describe basic human-readable text such as an address, a\n            cadastral reference, or less precise information found in a record."@en ;
        <http://www.w3.org/2000/01/rdf-schema#domain>
                <https://www.ica.org/standards/RiC/ontology#Place> ;
        <http://www.w3.org/2000/01/rdf-schema#isDefinedBy>
                <https://www.ica.org/standards/RiC/ontology> ;
        <http://www.w3.org/2000/01/rdf-schema#label>
                "location"@en ;
        <http://www.w3.org/2000/01/rdf-schema#range>
                <http://www.w3.org/2000/01/rdf-schema#Literal> ;
        <http://www.w3.org/2000/01/rdf-schema#subPropertyOf>
                <http://www.w3.org/2002/07/owl#topDataProperty> ;
        <http://www.w3.org/2004/02/skos/core#changeNote>
                []  ;
        <http://www.w3.org/2004/02/skos/core#example>
                "« Montreal »"@en , "25 rue Saint-Denis à Paris"@fr , "near the church"@en ;
        <http://www.w3.org/2004/02/skos/core#scopeNote>
                "Use only if you don't use PhysicalLocation class with Place.\n            Use the geographicalCoordinates property, or the Coordinates class, record the\n            geographical coordinates of the Place.s"@en ;
        <https://www.ica.org/standards/RiC/ontology#RiCCMCorrespondingComponent>
                "Corresponds to RiC-A27 (Location\n            attribute)"@en .

<https://www.ica.org/standards/RiC/ontology#endDate>
        a       <http://www.w3.org/2002/07/owl#DatatypeProperty> ;
        <http://www.w3.org/2000/01/rdf-schema#comment>
                "Date at which something ended."@en ;
        <http://www.w3.org/2000/01/rdf-schema#domain>
                <https://www.ica.org/standards/RiC/ontology#Thing> ;
        <http://www.w3.org/2000/01/rdf-schema#isDefinedBy>
                <https://www.ica.org/standards/RiC/ontology> ;
        <http://www.w3.org/2000/01/rdf-schema#label>
                "end date"@en ;
        <http://www.w3.org/2000/01/rdf-schema#range>
                <http://www.w3.org/2000/01/rdf-schema#Literal> ;
        <http://www.w3.org/2000/01/rdf-schema#subPropertyOf>
                <https://www.ica.org/standards/RiC/ontology#date> ;
        <http://www.w3.org/2004/02/skos/core#scopeNote>
                "Provided for usability reasons. May be deprecated and removed\n            later on. Use only if you don't use Date classes for handling dates."@en ;
        <https://www.ica.org/standards/RiC/ontology#RiCCMCorrespondingComponent>
                "Data property specialized implementation of\n            RiC-E18 (Date entity)"@en .

<https://www.ica.org/standards/RiC/ontology#referenceSystem>
        a       <http://www.w3.org/2002/07/owl#DatatypeProperty> ;
        <http://www.w3.org/2000/01/rdf-schema#comment>
                "Framework or standard used to represent an\n            information."@en ;
        <http://www.w3.org/2000/01/rdf-schema#domain>
                <https://www.ica.org/standards/RiC/ontology#Thing> ;
        <http://www.w3.org/2000/01/rdf-schema#isDefinedBy>
                <https://www.ica.org/standards/RiC/ontology> ;
        <http://www.w3.org/2000/01/rdf-schema#label>
                "reference system"@en ;
        <http://www.w3.org/2000/01/rdf-schema#range>
                <http://www.w3.org/2000/01/rdf-schema#Literal> ;
        <http://www.w3.org/2000/01/rdf-schema#subPropertyOf>
                <http://www.w3.org/2002/07/owl#topDataProperty> .

<https://www.ica.org/standards/RiC/ontology#Place>
        a       <http://www.w3.org/2002/07/owl#Class> ;
        <http://www.w3.org/2000/01/rdf-schema#comment>
                "Bounded, named geographic area or region."@en ;
        <http://www.w3.org/2000/01/rdf-schema#isDefinedBy>
                <https://www.ica.org/standards/RiC/ontology> ;
        <http://www.w3.org/2000/01/rdf-schema#label>
                "Place"@en ;
        <http://www.w3.org/2000/01/rdf-schema#subClassOf>
                <https://www.ica.org/standards/RiC/ontology#Thing> ;
        <http://www.w3.org/2004/02/skos/core#scopeNote>
                "A Place may be a jurisdiction, a manmade structure, or a\n            natural feature. A manmade structure or natural feature may also be a jurisdiction. A\n            Place may be referenced to a Physical Location on the earth, or (if you don't want to\n            use the PhysicalLocation class) directly to geographic coordinates. Both jurisdictions\n            and natural features are historical entities. A Place thus may have begin and end dates,\n            and changing boundaries that result from human or natural events. A Jurisdiction is the\n            bounded geographic area within which an Agent has the authority to perform specified\n            activities constrained by rules."@en ;
        <https://www.ica.org/standards/RiC/ontology#RiCCMCorrespondingComponent>
                "Corresponds to RiC-E22 (Place\n            entity)"@en .

<https://www.ica.org/standards/RiC/ontology#identifier>
        a       <http://www.w3.org/2002/07/owl#DatatypeProperty> ;
        <http://www.w3.org/2000/01/rdf-schema#comment>
                "A word, number, letter, symbol, or any combination of these used\n            to uniquely identify or reference an individual instance of an entity within a specific\n            information domain. Includes Global Persistent Identifiers (globally unique and\n            persistently resolvable identifier for the entity) and/or Local\n            Identifiers."@en ;
        <http://www.w3.org/2000/01/rdf-schema#domain>
                <https://www.ica.org/standards/RiC/ontology#Thing> ;
        <http://www.w3.org/2000/01/rdf-schema#isDefinedBy>
                <https://www.ica.org/standards/RiC/ontology> ;
        <http://www.w3.org/2000/01/rdf-schema#label>
                "identifier"@en ;
        <http://www.w3.org/2000/01/rdf-schema#range>
                <http://www.w3.org/2000/01/rdf-schema#Literal> ;
        <http://www.w3.org/2000/01/rdf-schema#subPropertyOf>
                <http://www.w3.org/2002/07/owl#topDataProperty> ;
        <http://www.w3.org/2004/02/skos/core#changeNote>
                []  ;
        <http://www.w3.org/2004/02/skos/core#example>
                "SNAC ID: 83847206"@en , "ISNI : 0000000073572182"@en , "BUD-01-F002 [example of a classification number from a corporate\n            file plan]"@en , "NAS1/A/1.1 [example of local identifier for a\n            Record]"@en , "F 1204 [example of a local identifier for a Record Set assigned\n            by a repository]"@en , "Ark ID: w6tz44ht"@en ;
        <http://www.w3.org/2004/02/skos/core#scopeNote>
                "Use only if you don't use Identifier class for handling\n            identifiers. Within a given domain (a closed system), identifiers are used to uniquely\n            reference instances of an entity. Identifiers are instruments of control that facilitate\n            management of the entities within the domain. The formulation of identifiers commonly is\n            based on rules."@en ;
        <https://www.ica.org/standards/RiC/ontology#RiCCMCorrespondingComponent>
                "Corresponds to RiC-A22 (Identifier\n            attribute)"@en .

<https://www.ica.org/standards/RiC/ontology#ruleFollowed>
        a       <http://www.w3.org/2002/07/owl#DatatypeProperty> ;
        <http://www.w3.org/2000/01/rdf-schema#comment>
                "The rule or conditions that govern the existence or lifecycle of\n            a Thing."@en ;
        <http://www.w3.org/2000/01/rdf-schema#domain>
                <https://www.ica.org/standards/RiC/ontology#Thing> ;
        <http://www.w3.org/2000/01/rdf-schema#isDefinedBy>
                <https://www.ica.org/standards/RiC/ontology> ;
        <http://www.w3.org/2000/01/rdf-schema#label>
                "rule followed"@en ;
        <http://www.w3.org/2000/01/rdf-schema#range>
                <http://www.w3.org/2000/01/rdf-schema#Literal> ;
        <http://www.w3.org/2000/01/rdf-schema#subPropertyOf>
                <http://www.w3.org/2002/07/owl#topDataProperty> ;
        <http://www.w3.org/2004/02/skos/core#scopeNote>
                "Provided for usability reasons. May be deprecated and removed\n            later on. Use only if you don't use the Rule class for handling rules."@en .

<https://www.ica.org/standards/RiC/ontology#descriptiveNote>
        a       <http://www.w3.org/2002/07/owl#DatatypeProperty> ;
        <http://www.w3.org/2000/01/rdf-schema#comment>
                "Descriptive information about an entity that is not otherwise\n            addressed."@en ;
        <http://www.w3.org/2000/01/rdf-schema#domain>
                <https://www.ica.org/standards/RiC/ontology#Thing> ;
        <http://www.w3.org/2000/01/rdf-schema#isDefinedBy>
                <https://www.ica.org/standards/RiC/ontology> ;
        <http://www.w3.org/2000/01/rdf-schema#label>
                "descriptive note"@en ;
        <http://www.w3.org/2000/01/rdf-schema#range>
                <http://www.w3.org/2000/01/rdf-schema#Literal> ;
        <http://www.w3.org/2000/01/rdf-schema#subPropertyOf>
                <http://www.w3.org/2002/07/owl#topDataProperty> ;
        <https://www.ica.org/standards/RiC/ontology#RiCCMCorrespondingComponent>
                "Corresponds to RiC-A16 (Descriptive Note\n            attribute)"@en .

<https://www.ica.org/standards/RiC/ontology#lastModificationDate>
        a       <http://www.w3.org/2002/07/owl#DatatypeProperty> ;
        <http://www.w3.org/2000/01/rdf-schema#comment>
                "Date at which an entity was last updated."@en ;
        <http://www.w3.org/2000/01/rdf-schema#domain>
                <https://www.ica.org/standards/RiC/ontology#Thing> ;
        <http://www.w3.org/2000/01/rdf-schema#isDefinedBy>
                <https://www.ica.org/standards/RiC/ontology> ;
        <http://www.w3.org/2000/01/rdf-schema#label>
                "last modification date"@en ;
        <http://www.w3.org/2000/01/rdf-schema#range>
                <http://www.w3.org/2000/01/rdf-schema#Literal> ;
        <http://www.w3.org/2000/01/rdf-schema#subPropertyOf>
                <https://www.ica.org/standards/RiC/ontology#modificationDate> ;
        <http://www.w3.org/2004/02/skos/core#scopeNote>
                "Provided for usability reasons. May be deprecated and removed\n            later on. Use only if you don't use Date classes for handling dates."@en ;
        <https://www.ica.org/standards/RiC/ontology#RiCCMCorrespondingComponent>
                "Data property specialized implementation of\n            RiC-E18 (Date entity)"@en .

<https://www.ica.org/standards/RiC/ontology#name>
        a       <http://www.w3.org/2002/07/owl#DatatypeProperty> ;
        <http://www.w3.org/2000/01/rdf-schema#comment>
                "A label, title or term designating the entity in order to make\n            it distinguishable from other similar entities. For Record Resource or Instantiation,\n            the Name is generally assigned by an Agent as most do not have a Name given when\n            created."@en ;
        <http://www.w3.org/2000/01/rdf-schema#domain>
                <https://www.ica.org/standards/RiC/ontology#Thing> ;
        <http://www.w3.org/2000/01/rdf-schema#isDefinedBy>
                <https://www.ica.org/standards/RiC/ontology> ;
        <http://www.w3.org/2000/01/rdf-schema#label>
                "name"@en ;
        <http://www.w3.org/2000/01/rdf-schema#range>
                <http://www.w3.org/2000/01/rdf-schema#Literal> ;
        <http://www.w3.org/2000/01/rdf-schema#subPropertyOf>
                <http://www.w3.org/2002/07/owl#topDataProperty> ;
        <http://www.w3.org/2004/02/skos/core#changeNote>
                []  ;
        <http://www.w3.org/2004/02/skos/core#example>
                "hearing services"@en , "4 March 1842"@en , "Digital copy of the Pomarius archival inventory from\n            1575"@en , "fundraising, University of Glasgow"@en , "Papers of the Earls of Liverpool"@en , "The Letter of Neacsu from Campulung to the Mayor of\n            Brasov"@en , "Sketch Map of the Qatar Peninsula"@en , "Nelson Mandela"@en ;
        <http://www.w3.org/2004/02/skos/core#scopeNote>
                "Use only if you don't use Name class for handling\n            names."@en ;
        <https://www.ica.org/standards/RiC/ontology#RiCCMCorrespondingComponent>
                "Corrresponds to RiC-A28 (Name\n            attribute)"@en .

<https://www.ica.org/standards/RiC/ontology#beginningDate>
        a       <http://www.w3.org/2002/07/owl#DatatypeProperty> ;
        <http://www.w3.org/2000/01/rdf-schema#comment>
                "Date at which something began."@en ;
        <http://www.w3.org/2000/01/rdf-schema#domain>
                <https://www.ica.org/standards/RiC/ontology#Thing> ;
        <http://www.w3.org/2000/01/rdf-schema#isDefinedBy>
                <https://www.ica.org/standards/RiC/ontology> ;
        <http://www.w3.org/2000/01/rdf-schema#label>
                "beginning date"@en ;
        <http://www.w3.org/2000/01/rdf-schema#range>
                <http://www.w3.org/2000/01/rdf-schema#Literal> ;
        <http://www.w3.org/2000/01/rdf-schema#subPropertyOf>
                <https://www.ica.org/standards/RiC/ontology#date> ;
        <http://www.w3.org/2004/02/skos/core#scopeNote>
                "Provided for usability reasons. May be deprecated and removed\n            later on. Use only if you don't use Date classes for handling dates."@en ;
        <https://www.ica.org/standards/RiC/ontology#RiCCMCorrespondingComponent>
                "Data property specialized implementation of\n            RiC-E18 (Date entity)"@en .

<https://www.ica.org/standards/RiC/ontology#type>
        a       <http://www.w3.org/2002/07/owl#DatatypeProperty> ;
        <http://www.w3.org/2000/01/rdf-schema#comment>
                "A term used to characterize an entity."@en ;
        <http://www.w3.org/2000/01/rdf-schema#domain>
                <https://www.ica.org/standards/RiC/ontology#Thing> ;
        <http://www.w3.org/2000/01/rdf-schema#isDefinedBy>
                <https://www.ica.org/standards/RiC/ontology> ;
        <http://www.w3.org/2000/01/rdf-schema#label>
                "type"@en ;
        <http://www.w3.org/2000/01/rdf-schema#range>
                <http://www.w3.org/2000/01/rdf-schema#Literal> ;
        <http://www.w3.org/2000/01/rdf-schema#subPropertyOf>
                <http://www.w3.org/2002/07/owl#topDataProperty> ;
        <http://www.w3.org/2004/02/skos/core#scopeNote>
                "Provided for usability reasons. May be deprecated and removed\n            later on. Use only if you don't use Type subclasses for handling\n            categories."@en .

<https://www.ica.org/standards/RiC/ontology#authorizingMandate>
        a       <http://www.w3.org/2002/07/owl#DatatypeProperty> ;
        <http://www.w3.org/2000/01/rdf-schema#comment>
                "Information on a Mandate that authorizes an Agent to perform an\n            Activity."@en ;
        <http://www.w3.org/2000/01/rdf-schema#domain>
                <https://www.ica.org/standards/RiC/ontology#Agent> ;
        <http://www.w3.org/2000/01/rdf-schema#isDefinedBy>
                <https://www.ica.org/standards/RiC/ontology> ;
        <http://www.w3.org/2000/01/rdf-schema#label>
                "authorizing mandate"@en ;
        <http://www.w3.org/2000/01/rdf-schema#range>
                <http://www.w3.org/2000/01/rdf-schema#Literal> ;
        <http://www.w3.org/2000/01/rdf-schema#subPropertyOf>
                <https://www.ica.org/standards/RiC/ontology#ruleFollowed> ;
        <http://www.w3.org/2004/02/skos/core#scopeNote>
                "Provided for usability reasons. May be deprecated and removed\n            later on. Use only if you don't use the Mandate class for handling\n            mandates."@en .
