<https://www.ica.org/standards/RiC/ontology#hasSibling>
        a       <http://www.w3.org/2002/07/owl#ObjectProperty> , <http://www.w3.org/2002/07/owl#SymmetricProperty> ;
        <http://www.w3.org/2000/01/rdf-schema#comment>
                "Connects two Persons that are siblings. This relation is\n            symmetric."@en ;
        <http://www.w3.org/2000/01/rdf-schema#domain>
                <https://www.ica.org/standards/RiC/ontology#Person> ;
        <http://www.w3.org/2000/01/rdf-schema#isDefinedBy>
                <https://www.ica.org/standards/RiC/ontology> ;
        <http://www.w3.org/2000/01/rdf-schema#label>
                "has sibling"@en ;
        <http://www.w3.org/2000/01/rdf-schema#range>
                <https://www.ica.org/standards/RiC/ontology#Person> ;
        <http://www.w3.org/2000/01/rdf-schema#subPropertyOf>
                <https://www.ica.org/standards/RiC/ontology#hasFamilyAssociationWith> ;
        <http://www.w3.org/2000/01/rdf-schema#subPropertyOf>
                []  ;
        <http://www.w3.org/2002/07/owl#equivalentProperty>
                []  ;
        <http://www.w3.org/2002/07/owl#inverseOf>
                <https://www.ica.org/standards/RiC/ontology#hasSibling> ;
        <http://www.w3.org/2002/07/owl#propertyChainAxiom>
                []  ;
        <http://www.w3.org/2004/02/skos/core#changeNote>
                []  ;
        <https://www.ica.org/standards/RiC/ontology#RiCCMCorrespondingComponent>
                "RiC-R048 ('has sibling'\n            relation)"@en .

<https://www.ica.org/standards/RiC/ontology#hasOrHadSpouse>
        a       <http://www.w3.org/2002/07/owl#SymmetricProperty> , <http://www.w3.org/2002/07/owl#ObjectProperty> ;
        <http://www.w3.org/2000/01/rdf-schema#comment>
                "Connects two Persons that are or were married. This relation is\n            symmetric."@en ;
        <http://www.w3.org/2000/01/rdf-schema#domain>
                <https://www.ica.org/standards/RiC/ontology#Person> ;
        <http://www.w3.org/2000/01/rdf-schema#isDefinedBy>
                <https://www.ica.org/standards/RiC/ontology> ;
        <http://www.w3.org/2000/01/rdf-schema#label>
                "has or had spouse"@en ;
        <http://www.w3.org/2000/01/rdf-schema#range>
                <https://www.ica.org/standards/RiC/ontology#Person> ;
        <http://www.w3.org/2000/01/rdf-schema#subPropertyOf>
                <https://www.ica.org/standards/RiC/ontology#hasFamilyAssociationWith> ;
        <http://www.w3.org/2000/01/rdf-schema#subPropertyOf>
                []  ;
        <http://www.w3.org/2002/07/owl#equivalentProperty>
                []  ;
        <http://www.w3.org/2002/07/owl#inverseOf>
                <https://www.ica.org/standards/RiC/ontology#hasOrHadSpouse> ;
        <http://www.w3.org/2002/07/owl#propertyChainAxiom>
                []  ;
        <http://www.w3.org/2004/02/skos/core#changeNote>
                []  ;
        <https://www.ica.org/standards/RiC/ontology#RiCCMCorrespondingComponent>
                "RiC-R049 ('has or had spouse'\n            relation)"@en .

<https://www.ica.org/standards/RiC/ontology#deathDate>
        a       <http://www.w3.org/2002/07/owl#DatatypeProperty> ;
        <http://www.w3.org/2000/01/rdf-schema#comment>
                "Date at which a Person died."@en ;
        <http://www.w3.org/2000/01/rdf-schema#domain>
                <https://www.ica.org/standards/RiC/ontology#Person> ;
        <http://www.w3.org/2000/01/rdf-schema#isDefinedBy>
                <https://www.ica.org/standards/RiC/ontology> ;
        <http://www.w3.org/2000/01/rdf-schema#label>
                "death date"@en ;
        <http://www.w3.org/2000/01/rdf-schema#range>
                <http://www.w3.org/2000/01/rdf-schema#Literal> ;
        <http://www.w3.org/2000/01/rdf-schema#subPropertyOf>
                <https://www.ica.org/standards/RiC/ontology#endDate> ;
        <http://www.w3.org/2004/02/skos/core#scopeNote>
                "Provided for usability reasons. May be deprecated and removed\n            later on. Use only if you don't use Date classes for handling dates."@en ;
        <https://www.ica.org/standards/RiC/ontology#RiCCMCorrespondingComponent>
                "Data property specialized implementation of\n            RiC-E18 (Date entity)"@en .

<https://www.ica.org/standards/RiC/ontology#hasFamilyAssociationWith>
        a       <http://www.w3.org/2002/07/owl#SymmetricProperty> , <http://www.w3.org/2002/07/owl#ObjectProperty> ;
        <http://www.w3.org/2000/01/rdf-schema#comment>
                "Connects two Persons that have some type of family link, i.e.\n            belong to the same family. This relation is symmetric."@en ;
        <http://www.w3.org/2000/01/rdf-schema#domain>
                <https://www.ica.org/standards/RiC/ontology#Person> ;
        <http://www.w3.org/2000/01/rdf-schema#isDefinedBy>
                <https://www.ica.org/standards/RiC/ontology> ;
        <http://www.w3.org/2000/01/rdf-schema#label>
                "has family association with"@en ;
        <http://www.w3.org/2000/01/rdf-schema#range>
                <https://www.ica.org/standards/RiC/ontology#Person> ;
        <http://www.w3.org/2000/01/rdf-schema#subPropertyOf>
                <https://www.ica.org/standards/RiC/ontology#isAgentAssociatedWithAgent> ;
        <http://www.w3.org/2000/01/rdf-schema#subPropertyOf>
                []  ;
        <http://www.w3.org/2002/07/owl#equivalentProperty>
                []  ;
        <http://www.w3.org/2002/07/owl#inverseOf>
                <https://www.ica.org/standards/RiC/ontology#hasFamilyAssociationWith> ;
        <http://www.w3.org/2002/07/owl#propertyChainAxiom>
                []  ;
        <http://www.w3.org/2004/02/skos/core#changeNote>
                []  ;
        <https://www.ica.org/standards/RiC/ontology#RiCCMCorrespondingComponent>
                "RiC-R047 ('has family association with'\n            relation)"@en .

<https://www.ica.org/standards/RiC/ontology#knowsOf>
        a       <http://www.w3.org/2002/07/owl#ObjectProperty> ;
        <http://www.w3.org/2000/01/rdf-schema#comment>
                "Connects a Person to another Person they have some knowledge of\n            through time or space."@en ;
        <http://www.w3.org/2000/01/rdf-schema#domain>
                <https://www.ica.org/standards/RiC/ontology#Person> ;
        <http://www.w3.org/2000/01/rdf-schema#isDefinedBy>
                <https://www.ica.org/standards/RiC/ontology> ;
        <http://www.w3.org/2000/01/rdf-schema#label>
                "knows of "@en ;
        <http://www.w3.org/2000/01/rdf-schema#range>
                <https://www.ica.org/standards/RiC/ontology#Person> ;
        <http://www.w3.org/2000/01/rdf-schema#subPropertyOf>
                <https://www.ica.org/standards/RiC/ontology#isAgentAssociatedWithAgent> ;
        <http://www.w3.org/2000/01/rdf-schema#subPropertyOf>
                []  ;
        <http://www.w3.org/2002/07/owl#propertyChainAxiom>
                []  ;
        <https://www.ica.org/standards/RiC/ontology#RiCCMCorrespondingComponent>
                "RiC-R050 ('knows of'\n            relation)"@en .

<https://www.ica.org/standards/RiC/ontology#knows>
        a       <http://www.w3.org/2002/07/owl#ObjectProperty> , <http://www.w3.org/2002/07/owl#SymmetricProperty> ;
        <http://www.w3.org/2000/01/rdf-schema#comment>
                "Connects two Persons that directly know each other during their\n            existence. This object property is symmetric."@en ;
        <http://www.w3.org/2000/01/rdf-schema#domain>
                <https://www.ica.org/standards/RiC/ontology#Person> ;
        <http://www.w3.org/2000/01/rdf-schema#isDefinedBy>
                <https://www.ica.org/standards/RiC/ontology> ;
        <http://www.w3.org/2000/01/rdf-schema#label>
                "knows "@en ;
        <http://www.w3.org/2000/01/rdf-schema#range>
                <https://www.ica.org/standards/RiC/ontology#Person> ;
        <http://www.w3.org/2000/01/rdf-schema#subPropertyOf>
                <https://www.ica.org/standards/RiC/ontology#isAgentAssociatedWithAgent> ;
        <http://www.w3.org/2000/01/rdf-schema#subPropertyOf>
                []  ;
        <http://www.w3.org/2002/07/owl#equivalentProperty>
                []  ;
        <http://www.w3.org/2002/07/owl#inverseOf>
                <https://www.ica.org/standards/RiC/ontology#knows> ;
        <http://www.w3.org/2002/07/owl#propertyChainAxiom>
                []  ;
        <https://www.ica.org/standards/RiC/ontology#RiCCMCorrespondingComponent>
                "RiC-R051 ('knows'\n            relation)"@en .

<https://www.ica.org/standards/RiC/ontology#hasDescendant>
        a       <http://www.w3.org/2002/07/owl#ObjectProperty> ;
        <http://www.w3.org/2000/01/rdf-schema#comment>
                "Connects a Person to one of their descendants."@en ;
        <http://www.w3.org/2000/01/rdf-schema#domain>
                <https://www.ica.org/standards/RiC/ontology#Person> ;
        <http://www.w3.org/2000/01/rdf-schema#isDefinedBy>
                <https://www.ica.org/standards/RiC/ontology> ;
        <http://www.w3.org/2000/01/rdf-schema#label>
                "has descendant"@en ;
        <http://www.w3.org/2000/01/rdf-schema#range>
                <https://www.ica.org/standards/RiC/ontology#Person> ;
        <http://www.w3.org/2000/01/rdf-schema#subPropertyOf>
                <https://www.ica.org/standards/RiC/ontology#hasFamilyAssociationWith> , <https://www.ica.org/standards/RiC/ontology#hasSuccessor> ;
        <http://www.w3.org/2000/01/rdf-schema#subPropertyOf>
                []  ;
        <http://www.w3.org/2000/01/rdf-schema#subPropertyOf>
                []  ;
        <http://www.w3.org/2002/07/owl#inverseOf>
                <https://www.ica.org/standards/RiC/ontology#hasAncestor> ;
        <http://www.w3.org/2002/07/owl#propertyChainAxiom>
                []  ;
        <http://www.w3.org/2004/02/skos/core#changeNote>
                []  ;
        <https://www.ica.org/standards/RiC/ontology#RiCCMCorrespondingComponent>
                "RiC-R017 ('has descendant'\n            relation)"@en .

<https://www.ica.org/standards/RiC/ontology#hasOrHadStudent>
        a       <http://www.w3.org/2002/07/owl#ObjectProperty> ;
        <http://www.w3.org/2000/01/rdf-schema#comment>
                "Inverse of 'has or had teacher' object property."@en ;
        <http://www.w3.org/2000/01/rdf-schema#domain>
                <https://www.ica.org/standards/RiC/ontology#Person> ;
        <http://www.w3.org/2000/01/rdf-schema#isDefinedBy>
                <https://www.ica.org/standards/RiC/ontology> ;
        <http://www.w3.org/2000/01/rdf-schema#label>
                "has or had student"@en ;
        <http://www.w3.org/2000/01/rdf-schema#range>
                <https://www.ica.org/standards/RiC/ontology#Person> ;
        <http://www.w3.org/2000/01/rdf-schema#subPropertyOf>
                <https://www.ica.org/standards/RiC/ontology#knows> ;
        <http://www.w3.org/2000/01/rdf-schema#subPropertyOf>
                []  ;
        <http://www.w3.org/2002/07/owl#equivalentProperty>
                []  ;
        <http://www.w3.org/2002/07/owl#propertyChainAxiom>
                []  ;
        <http://www.w3.org/2004/02/skos/core#changeNote>
                []  ;
        <https://www.ica.org/standards/RiC/ontology#RiCCMCorrespondingComponent>
                "RiC-R053i ('has or had student'\n            relation)"@en .

<https://www.ica.org/standards/RiC/ontology#isChildOf>
        a       <http://www.w3.org/2002/07/owl#ObjectProperty> ;
        <http://www.w3.org/2000/01/rdf-schema#comment>
                "Inverse of 'has child' object property."@en ;
        <http://www.w3.org/2000/01/rdf-schema#domain>
                <https://www.ica.org/standards/RiC/ontology#Person> ;
        <http://www.w3.org/2000/01/rdf-schema#isDefinedBy>
                <https://www.ica.org/standards/RiC/ontology> ;
        <http://www.w3.org/2000/01/rdf-schema#label>
                "is child of"@en ;
        <http://www.w3.org/2000/01/rdf-schema#range>
                <https://www.ica.org/standards/RiC/ontology#Person> ;
        <http://www.w3.org/2000/01/rdf-schema#subPropertyOf>
                <https://www.ica.org/standards/RiC/ontology#hasAncestor> ;
        <http://www.w3.org/2000/01/rdf-schema#subPropertyOf>
                []  ;
        <http://www.w3.org/2004/02/skos/core#changeNote>
                []  ;
        <https://www.ica.org/standards/RiC/ontology#RiCCMCorrespondingComponent>
                "RiC-R018i ('is child of'\n            relation)"@en .

<https://www.ica.org/standards/RiC/ontology#hasOrHadCorrespondent>
        a       <http://www.w3.org/2002/07/owl#SymmetricProperty> , <http://www.w3.org/2002/07/owl#ObjectProperty> ;
        <http://www.w3.org/2000/01/rdf-schema#comment>
                "Connects two Persons that correspond or have corresponded with\n            each other. This relation is symmetric."@en ;
        <http://www.w3.org/2000/01/rdf-schema#domain>
                <https://www.ica.org/standards/RiC/ontology#Person> ;
        <http://www.w3.org/2000/01/rdf-schema#isDefinedBy>
                <https://www.ica.org/standards/RiC/ontology> ;
        <http://www.w3.org/2000/01/rdf-schema#label>
                "has or had correspondent"@en ;
        <http://www.w3.org/2000/01/rdf-schema#range>
                <https://www.ica.org/standards/RiC/ontology#Person> ;
        <http://www.w3.org/2000/01/rdf-schema#subPropertyOf>
                <https://www.ica.org/standards/RiC/ontology#knows> ;
        <http://www.w3.org/2000/01/rdf-schema#subPropertyOf>
                []  ;
        <http://www.w3.org/2002/07/owl#equivalentProperty>
                []  ;
        <http://www.w3.org/2002/07/owl#inverseOf>
                <https://www.ica.org/standards/RiC/ontology#hasOrHadCorrespondent> ;
        <http://www.w3.org/2002/07/owl#propertyChainAxiom>
                []  ;
        <http://www.w3.org/2004/02/skos/core#changeNote>
                []  ;
        <https://www.ica.org/standards/RiC/ontology#RiCCMCorrespondingComponent>
                "RiC-R052 ('has or had correspondent'\n            relation)"@en .

<https://www.ica.org/standards/RiC/ontology#hasAncestor>
        a       <http://www.w3.org/2002/07/owl#ObjectProperty> ;
        <http://www.w3.org/2000/01/rdf-schema#comment>
                "Inverse of 'has descendant' object property."@en ;
        <http://www.w3.org/2000/01/rdf-schema#domain>
                <https://www.ica.org/standards/RiC/ontology#Person> ;
        <http://www.w3.org/2000/01/rdf-schema#isDefinedBy>
                <https://www.ica.org/standards/RiC/ontology> ;
        <http://www.w3.org/2000/01/rdf-schema#label>
                "has ancestor"@en ;
        <http://www.w3.org/2000/01/rdf-schema#range>
                <https://www.ica.org/standards/RiC/ontology#Person> ;
        <http://www.w3.org/2000/01/rdf-schema#subPropertyOf>
                <https://www.ica.org/standards/RiC/ontology#hasFamilyAssociationWith> , <https://www.ica.org/standards/RiC/ontology#isSuccessorOf> ;
        <http://www.w3.org/2000/01/rdf-schema#subPropertyOf>
                []  ;
        <http://www.w3.org/2000/01/rdf-schema#subPropertyOf>
                []  ;
        <http://www.w3.org/2002/07/owl#equivalentProperty>
                []  ;
        <http://www.w3.org/2002/07/owl#propertyChainAxiom>
                []  ;
        <http://www.w3.org/2004/02/skos/core#changeNote>
                []  ;
        <https://www.ica.org/standards/RiC/ontology#RiCCMCorrespondingComponent>
                "RiC-R017i (has ancestor\n            relation)"@en .

<https://www.ica.org/standards/RiC/ontology#hasOrHadTeacher>
        a       <http://www.w3.org/2002/07/owl#ObjectProperty> ;
        <http://www.w3.org/2000/01/rdf-schema#comment>
                "Connects a Person to another Person who is or was their\n            student."@en ;
        <http://www.w3.org/2000/01/rdf-schema#domain>
                <https://www.ica.org/standards/RiC/ontology#Person> ;
        <http://www.w3.org/2000/01/rdf-schema#isDefinedBy>
                <https://www.ica.org/standards/RiC/ontology> ;
        <http://www.w3.org/2000/01/rdf-schema#label>
                "has or had teacher"@en ;
        <http://www.w3.org/2000/01/rdf-schema#range>
                <https://www.ica.org/standards/RiC/ontology#Person> ;
        <http://www.w3.org/2000/01/rdf-schema#subPropertyOf>
                <https://www.ica.org/standards/RiC/ontology#knows> ;
        <http://www.w3.org/2000/01/rdf-schema#subPropertyOf>
                []  ;
        <http://www.w3.org/2002/07/owl#inverseOf>
                <https://www.ica.org/standards/RiC/ontology#hasOrHadStudent> ;
        <http://www.w3.org/2002/07/owl#propertyChainAxiom>
                []  ;
        <http://www.w3.org/2004/02/skos/core#changeNote>
                []  ;
        <https://www.ica.org/standards/RiC/ontology#RiCCMCorrespondingComponent>
                "RiC-R053 ('has or had teacher'\n            relation)"@en .

<https://www.ica.org/standards/RiC/ontology#Person>
        a       <http://www.w3.org/2002/07/owl#Class> ;
        <http://www.w3.org/2000/01/rdf-schema#comment>
                "A human being with a social identity or persona."@en ;
        <http://www.w3.org/2000/01/rdf-schema#isDefinedBy>
                <https://www.ica.org/standards/RiC/ontology> ;
        <http://www.w3.org/2000/01/rdf-schema#label>
                "Person"@en ;
        <http://www.w3.org/2000/01/rdf-schema#subClassOf>
                <https://www.ica.org/standards/RiC/ontology#Agent> ;
        <http://www.w3.org/2002/07/owl#disjointWith>
                <https://www.ica.org/standards/RiC/ontology#Position> ;
        <http://www.w3.org/2004/02/skos/core#scopeNote>
                "Person is a kind of Agent. Most commonly, a human being\n            (biological person) has a single coeval social identity or persona. In everyday\n            discourse, this is the “real person.” Less common though not rare, over the course of a\n            lifetime, personae in addition to the coeval (or “original”) persona may be associated\n            with the human being. Such “alternative personae” are most often created by the original\n            person for specific purposes. Under some circumstances, an alternative persona might\n            eclipse or replace the original person (Mark Twain eclipsing Samuel Clemens; John Wayne\n            eclipsing Marion Mitchell Morrison), that is, the social (shared) alternative identity\n            becomes the predominate identity. Less common is whentwo or more persons collaborate to\n            create a shared persona. Persona shared by two or more Persons constitute a kind of\n            Group. Within the archival context, the original Person generally will be the focus of\n            the description, with alternative personae noted. Exceptionally, an alternative persona\n            may displace the coeval persona.s."@en ;
        <https://www.ica.org/standards/RiC/ontology#RiCCMCorrespondingComponent>
                "Corresponds to RiC-E08 (Person\n            entity)"@en .

<https://www.ica.org/standards/RiC/ontology#knownBy>
        a       <http://www.w3.org/2002/07/owl#ObjectProperty> ;
        <http://www.w3.org/2000/01/rdf-schema#comment>
                "Inverse of 'knows of' object property."@en ;
        <http://www.w3.org/2000/01/rdf-schema#domain>
                <https://www.ica.org/standards/RiC/ontology#Person> ;
        <http://www.w3.org/2000/01/rdf-schema#isDefinedBy>
                <https://www.ica.org/standards/RiC/ontology> ;
        <http://www.w3.org/2000/01/rdf-schema#label>
                "known by "@en ;
        <http://www.w3.org/2000/01/rdf-schema#range>
                <https://www.ica.org/standards/RiC/ontology#Person> ;
        <http://www.w3.org/2000/01/rdf-schema#subPropertyOf>
                <https://www.ica.org/standards/RiC/ontology#isAgentAssociatedWithAgent> ;
        <http://www.w3.org/2000/01/rdf-schema#subPropertyOf>
                []  ;
        <http://www.w3.org/2002/07/owl#equivalentProperty>
                []  ;
        <http://www.w3.org/2002/07/owl#inverseOf>
                <https://www.ica.org/standards/RiC/ontology#knowsOf> ;
        <http://www.w3.org/2002/07/owl#propertyChainAxiom>
                []  ;
        <https://www.ica.org/standards/RiC/ontology#RiCCMCorrespondingComponent>
                "RiC-R050i ('known by'\n            relation)"@en .

<https://www.ica.org/standards/RiC/ontology#hasChild>
        a       <http://www.w3.org/2002/07/owl#ObjectProperty> ;
        <http://www.w3.org/2000/01/rdf-schema#comment>
                "Connects a Person to one of their children."@en ;
        <http://www.w3.org/2000/01/rdf-schema#domain>
                <https://www.ica.org/standards/RiC/ontology#Person> ;
        <http://www.w3.org/2000/01/rdf-schema#isDefinedBy>
                <https://www.ica.org/standards/RiC/ontology> ;
        <http://www.w3.org/2000/01/rdf-schema#label>
                "has child"@en ;
        <http://www.w3.org/2000/01/rdf-schema#range>
                <https://www.ica.org/standards/RiC/ontology#Person> ;
        <http://www.w3.org/2000/01/rdf-schema#subPropertyOf>
                <https://www.ica.org/standards/RiC/ontology#hasDescendant> ;
        <http://www.w3.org/2000/01/rdf-schema#subPropertyOf>
                []  ;
        <http://www.w3.org/2002/07/owl#equivalentProperty>
                []  ;
        <http://www.w3.org/2002/07/owl#inverseOf>
                <https://www.ica.org/standards/RiC/ontology#isChildOf> ;
        <http://www.w3.org/2002/07/owl#propertyChainAxiom>
                []  ;
        <http://www.w3.org/2004/02/skos/core#changeNote>
                []  ;
        <https://www.ica.org/standards/RiC/ontology#RiCCMCorrespondingComponent>
                "RiC-R018 ('has child'\n            relation)"@en .
