<http://iflastandards.info/ns/fr/frbr/pressoo/Y29i_continues>
        a       <http://www.w3.org/2002/07/owl#ObjectProperty> ;
        <http://www.w3.org/2000/01/rdf-schema#domain>
                <http://iflastandards.info/ns/fr/frbr/frbroo/F18_Serial_Work> ;
        <http://www.w3.org/2000/01/rdf-schema#label>
                "continues"@en ;
        <http://www.w3.org/2000/01/rdf-schema#range>
                <http://iflastandards.info/ns/fr/frbr/frbroo/F18_Serial_Work> ;
        <http://www.w3.org/2000/01/rdf-schema#subPropertyOf>
                <http://www.w3.org/2002/07/owl#topObjectProperty> .

<http://iflastandards.info/ns/fr/frbr/frbroo/F18_Serial_Work>
        a       <http://www.w3.org/2002/07/owl#Class> ;
        <http://www.w3.org/2000/01/rdf-schema#subClassOf>
                <http://www.w3.org/2002/07/owl#Thing> .

<http://iflastandards.info/ns/fr/frbr/pressoo/Y31i_superseded>
        a       <http://www.w3.org/2002/07/owl#ObjectProperty> ;
        <http://www.w3.org/2000/01/rdf-schema#domain>
                <http://iflastandards.info/ns/fr/frbr/frbroo/F18_Serial_Work> ;
        <http://www.w3.org/2000/01/rdf-schema#label>
                "superseded"@en ;
        <http://www.w3.org/2000/01/rdf-schema#range>
                <http://iflastandards.info/ns/fr/frbr/frbroo/F18_Serial_Work> ;
        <http://www.w3.org/2000/01/rdf-schema#subPropertyOf>
                <http://www.w3.org/2002/07/owl#topObjectProperty> .

<http://iflastandards.info/ns/fr/frbr/pressoo/Y30i_was_separated_from>
        a       <http://www.w3.org/2002/07/owl#ObjectProperty> ;
        <http://www.w3.org/2000/01/rdf-schema#domain>
                <http://iflastandards.info/ns/fr/frbr/frbroo/F18_Serial_Work> ;
        <http://www.w3.org/2000/01/rdf-schema#label>
                "was separated from"@en ;
        <http://www.w3.org/2000/01/rdf-schema#range>
                <http://iflastandards.info/ns/fr/frbr/frbroo/F18_Serial_Work> ;
        <http://www.w3.org/2000/01/rdf-schema#subPropertyOf>
                <http://www.w3.org/2002/07/owl#topObjectProperty> .

<http://iflastandards.info/ns/fr/frbr/pressoo/Y35_was_absorbed_in>
        a       <http://www.w3.org/2002/07/owl#ObjectProperty> ;
        <http://www.w3.org/2000/01/rdf-schema#comment>
                "This property associates instances of F18 Serial Work with the instances of F18 Serial Work that absorbed them."@en ;
        <http://www.w3.org/2000/01/rdf-schema#domain>
                <http://iflastandards.info/ns/fr/frbr/frbroo/F18_Serial_Work> ;
        <http://www.w3.org/2000/01/rdf-schema#label>
                "was absorbed in"@en ;
        <http://www.w3.org/2000/01/rdf-schema#range>
                <http://iflastandards.info/ns/fr/frbr/frbroo/F18_Serial_Work> ;
        <http://www.w3.org/2000/01/rdf-schema#subPropertyOf>
                <http://www.w3.org/2002/07/owl#topObjectProperty> .

<http://iflastandards.info/ns/fr/frbr/pressoo/Y29_evolved_into>
        a       <http://www.w3.org/2002/07/owl#ObjectProperty> ;
        <http://www.w3.org/2000/01/rdf-schema#comment>
                "This property associates an instance of F18 Serial Work with the instance of F18 Serial Work into which it was transformed, due to a ‘major’ title change."@en ;
        <http://www.w3.org/2000/01/rdf-schema#domain>
                <http://iflastandards.info/ns/fr/frbr/frbroo/F18_Serial_Work> ;
        <http://www.w3.org/2000/01/rdf-schema#label>
                "evolved into"@en ;
        <http://www.w3.org/2000/01/rdf-schema#range>
                <http://iflastandards.info/ns/fr/frbr/frbroo/F18_Serial_Work> ;
        <http://www.w3.org/2000/01/rdf-schema#subPropertyOf>
                <http://www.w3.org/2002/07/owl#topObjectProperty> .

<http://iflastandards.info/ns/fr/frbr/pressoo/Y30_was_partially_continued_by>
        a       <http://www.w3.org/2002/07/owl#ObjectProperty> ;
        <http://www.w3.org/2000/01/rdf-schema#comment>
                "This property associates an instance of F18 Serial Work with an instance of F18 Serial Work that was separated from it through an instance of Z3 Separation"@en ;
        <http://www.w3.org/2000/01/rdf-schema#domain>
                <http://iflastandards.info/ns/fr/frbr/frbroo/F18_Serial_Work> ;
        <http://www.w3.org/2000/01/rdf-schema#label>
                "was partially continued by"@en ;
        <http://www.w3.org/2000/01/rdf-schema#range>
                <http://iflastandards.info/ns/fr/frbr/frbroo/F18_Serial_Work> ;
        <http://www.w3.org/2000/01/rdf-schema#subPropertyOf>
                <http://www.w3.org/2002/07/owl#topObjectProperty> .

<http://iflastandards.info/ns/fr/frbr/pressoo/Y34_was_merged_to_form>
        a       <http://www.w3.org/2002/07/owl#ObjectProperty> ;
        <http://www.w3.org/2000/01/rdf-schema#comment>
                "This property associates instances of F18 Serial Work with an instance of F18 Serial Work that was created by merging them."@en ;
        <http://www.w3.org/2000/01/rdf-schema#domain>
                <http://iflastandards.info/ns/fr/frbr/frbroo/F18_Serial_Work> ;
        <http://www.w3.org/2000/01/rdf-schema#label>
                "was merged to form"@en ;
        <http://www.w3.org/2000/01/rdf-schema#range>
                <http://iflastandards.info/ns/fr/frbr/frbroo/F18_Serial_Work> ;
        <http://www.w3.org/2000/01/rdf-schema#subPropertyOf>
                <http://www.w3.org/2002/07/owl#topObjectProperty> .

<http://iflastandards.info/ns/fr/frbr/pressoo/Y34i_resulted_from_merging>
        a       <http://www.w3.org/2002/07/owl#ObjectProperty> ;
        <http://www.w3.org/2000/01/rdf-schema#domain>
                <http://iflastandards.info/ns/fr/frbr/frbroo/F18_Serial_Work> ;
        <http://www.w3.org/2000/01/rdf-schema#label>
                "resulted from merging"@en ;
        <http://www.w3.org/2000/01/rdf-schema#range>
                <http://iflastandards.info/ns/fr/frbr/frbroo/F18_Serial_Work> ;
        <http://www.w3.org/2000/01/rdf-schema#subPropertyOf>
                <http://www.w3.org/2002/07/owl#topObjectProperty> .

<http://iflastandards.info/ns/fr/frbr/pressoo/Y32_was_split_into>
        a       <http://www.w3.org/2002/07/owl#ObjectProperty> ;
        <http://www.w3.org/2000/01/rdf-schema#comment>
                "This property associates an instance of F18 Serial Work with any one of the instances of F18 Serial Work that were created on the occasion of its split."@en ;
        <http://www.w3.org/2000/01/rdf-schema#domain>
                <http://iflastandards.info/ns/fr/frbr/frbroo/F18_Serial_Work> ;
        <http://www.w3.org/2000/01/rdf-schema#label>
                "was split into"@en ;
        <http://www.w3.org/2000/01/rdf-schema#range>
                <http://iflastandards.info/ns/fr/frbr/frbroo/F18_Serial_Work> ;
        <http://www.w3.org/2000/01/rdf-schema#subPropertyOf>
                <http://www.w3.org/2002/07/owl#topObjectProperty> .

<http://iflastandards.info/ns/fr/frbr/pressoo/Y31_was_superseded_by>
        a       <http://www.w3.org/2002/07/owl#ObjectProperty> ;
        <http://www.w3.org/2000/01/rdf-schema#comment>
                "This property associates an instance of Z1 Serial Transformation with an instance of F18 Serial Work that was created with the distinct intention of being published in lieu of another instance of F18 Serial Work the publication of which had ceased."@en ;
        <http://www.w3.org/2000/01/rdf-schema#domain>
                <http://iflastandards.info/ns/fr/frbr/frbroo/F18_Serial_Work> ;
        <http://www.w3.org/2000/01/rdf-schema#label>
                "was superseded by"@en ;
        <http://www.w3.org/2000/01/rdf-schema#range>
                <http://iflastandards.info/ns/fr/frbr/frbroo/F18_Serial_Work> ;
        <http://www.w3.org/2000/01/rdf-schema#subPropertyOf>
                <http://www.w3.org/2002/07/owl#topObjectProperty> .

<http://iflastandards.info/ns/fr/frbr/pressoo/Y35i_was_enhanced_by_absorbing>
        a       <http://www.w3.org/2002/07/owl#ObjectProperty> ;
        <http://www.w3.org/2000/01/rdf-schema#domain>
                <http://iflastandards.info/ns/fr/frbr/frbroo/F18_Serial_Work> ;
        <http://www.w3.org/2000/01/rdf-schema#label>
                "was enhanced by absorbing"@en ;
        <http://www.w3.org/2000/01/rdf-schema#range>
                <http://iflastandards.info/ns/fr/frbr/frbroo/F18_Serial_Work> ;
        <http://www.w3.org/2000/01/rdf-schema#subPropertyOf>
                <http://www.w3.org/2002/07/owl#topObjectProperty> .

<http://iflastandards.info/ns/fr/frbr/pressoo/Y33_was_merged_with>
        a       <http://www.w3.org/2002/07/owl#ObjectProperty> ;
        <http://www.w3.org/2000/01/rdf-schema#comment>
                "This symmetrical property associates an instance of F18 Serial Work with any one of the instances of F18 Serial Work with which it was merged in order to create a new instance of F18 Serial Work."@en ;
        <http://www.w3.org/2000/01/rdf-schema#domain>
                <http://iflastandards.info/ns/fr/frbr/frbroo/F18_Serial_Work> ;
        <http://www.w3.org/2000/01/rdf-schema#label>
                "was merged with"@en ;
        <http://www.w3.org/2000/01/rdf-schema#range>
                <http://iflastandards.info/ns/fr/frbr/frbroo/F18_Serial_Work> ;
        <http://www.w3.org/2000/01/rdf-schema#subPropertyOf>
                <http://www.w3.org/2002/07/owl#topObjectProperty> .

<http://iflastandards.info/ns/fr/frbr/pressoo/Y36i_was_surrogate_for>
        a       <http://www.w3.org/2002/07/owl#ObjectProperty> ;
        <http://www.w3.org/2000/01/rdf-schema#domain>
                <http://iflastandards.info/ns/fr/frbr/frbroo/F18_Serial_Work> ;
        <http://www.w3.org/2000/01/rdf-schema#label>
                "was surrogate for"@en ;
        <http://www.w3.org/2000/01/rdf-schema#range>
                <http://iflastandards.info/ns/fr/frbr/frbroo/F18_Serial_Work> ;
        <http://www.w3.org/2000/01/rdf-schema#subPropertyOf>
                <http://www.w3.org/2002/07/owl#topObjectProperty> .

<http://iflastandards.info/ns/fr/frbr/pressoo/Y36_had_surrogate>
        a       <http://www.w3.org/2002/07/owl#ObjectProperty> ;
        <http://www.w3.org/2000/01/rdf-schema#comment>
                "This property associates an instance of F18 Serial Work with an instance of F18 Serial Work that temporarily replaced it."@en ;
        <http://www.w3.org/2000/01/rdf-schema#domain>
                <http://iflastandards.info/ns/fr/frbr/frbroo/F18_Serial_Work> ;
        <http://www.w3.org/2000/01/rdf-schema#label>
                "had surrogate"@en ;
        <http://www.w3.org/2000/01/rdf-schema#range>
                <http://iflastandards.info/ns/fr/frbr/frbroo/F18_Serial_Work> ;
        <http://www.w3.org/2000/01/rdf-schema#subPropertyOf>
                <http://www.w3.org/2002/07/owl#topObjectProperty> .

<http://iflastandards.info/ns/fr/frbr/pressoo/Y32i_resulted_from_splitting>
        a       <http://www.w3.org/2002/07/owl#ObjectProperty> ;
        <http://www.w3.org/2000/01/rdf-schema#domain>
                <http://iflastandards.info/ns/fr/frbr/frbroo/F18_Serial_Work> ;
        <http://www.w3.org/2000/01/rdf-schema#label>
                "resulted from splitting"@en ;
        <http://www.w3.org/2000/01/rdf-schema#range>
                <http://iflastandards.info/ns/fr/frbr/frbroo/F18_Serial_Work> ;
        <http://www.w3.org/2000/01/rdf-schema#subPropertyOf>
                <http://www.w3.org/2002/07/owl#topObjectProperty> .
