<https://www.ica.org/standards/RiC/ontology#RecordSet>
        a       <http://www.w3.org/2002/07/owl#Class> ;
        <http://www.w3.org/2000/01/rdf-schema#comment>
                "One or more records that are associated by categorization and/or\n            physical aggregation by the creator or other Agent."@en ;
        <http://www.w3.org/2000/01/rdf-schema#isDefinedBy>
                <https://www.ica.org/standards/RiC/ontology> ;
        <http://www.w3.org/2000/01/rdf-schema#label>
                "Record Set"@en ;
        <http://www.w3.org/2000/01/rdf-schema#subClassOf>
                <https://www.ica.org/standards/RiC/ontology#RecordResource> ;
        <http://www.w3.org/2004/02/skos/core#scopeNote>
                "Record Set is a kind of Record Resource. The Record members in\n            a Record Set may physically reside together, though physical proximity is not essential.\n            In a particular context, an Agent (e.g. administrator, records manager, archivist,\n            end-user, etc.) may select the Record members of a Record Set based on a shared\n            attribute or attributes, or a shared Relation or Relations. The grouping of the Records\n            serves a purpose or purposes specific to the context of the Agent. All Record members of\n            a Record Set may share the attribute of having been accumulated by the same Agent, or\n            all share the same Documentary Form Type and are created over time by the same Activity.\n            A Record Set may represent the act of classifying the Records in accordance with a\n            formal classification scheme that may be based on Activity, subject, organizational\n            structure, or other criteria; an act of archival arrangement (e.g. based on common\n            provenance); or some other selection and grouping that fulfils a particular purpose or\n            purposes (e.g. a classification that reflects or supports the purposes of a researcher).\n            By exception, some Records are brought together based on their not belonging in the\n            context of selection to other designated groups: a ‘Miscellaneous’ series, for example.\n            A Record Set accumulated by an Agent in the course of life or work Activity should be\n            kept in a manner that preserves context and evidential value. Records Sets may also\n            contain other Records Sets. Both a Record Set and a Record may simultaneously be a\n            member of more than one Record Set, and over the course of its existence, a Record Set\n            or Record may be a member of an indeterminate number of Record Sets in an indeterminate\n            number of contexts. Record Sets and Records contained within a Record Set may be ordered\n            into a sequence based on a common property or relation, or common properties or\n            relations (e.g. alphabetical by Agent or related Place name; chronological order by an\n            allocated Date); or some other criterion (e.g. an imposed order by\n            relevance)."@en ;
        <https://www.ica.org/standards/RiC/ontology#RiCCMCorrespondingComponent>
                "Corresponds to RiC-E03 (Record Set\n            entity)"@en .

<https://www.ica.org/standards/RiC/ontology#hasOrHadSomeMembersWithRecordState>
        a       <http://www.w3.org/2002/07/owl#ObjectProperty> ;
        <http://www.w3.org/2000/01/rdf-schema#comment>
                "Connects a Record Set and a Record State that categorizes some\n            of the Records or Record Parts that are or were included in the Record\n            Set."@en ;
        <http://www.w3.org/2000/01/rdf-schema#domain>
                <https://www.ica.org/standards/RiC/ontology#RecordSet> ;
        <http://www.w3.org/2000/01/rdf-schema#isDefinedBy>
                <https://www.ica.org/standards/RiC/ontology> ;
        <http://www.w3.org/2000/01/rdf-schema#label>
                "has or had some members with record state"@en ;
        <http://www.w3.org/2000/01/rdf-schema#range>
                <https://www.ica.org/standards/RiC/ontology#RecordState> ;
        <http://www.w3.org/2000/01/rdf-schema#subPropertyOf>
                <https://www.ica.org/standards/RiC/ontology#hasOrHadSomeMembersWithCategory> ;
        <http://www.w3.org/2000/01/rdf-schema#subPropertyOf>
                []  ;
        <http://www.w3.org/2002/07/owl#equivalentProperty>
                []  ;
        <http://www.w3.org/2002/07/owl#inverseOf>
                <https://www.ica.org/standards/RiC/ontology#isOrWasRecordStateOfSomeMembersOf> ;
        <http://www.w3.org/2004/02/skos/core#changeNote>
                []  .

<https://www.ica.org/standards/RiC/ontology#hasOrHadAllMembersWithRecordState>
        a       <http://www.w3.org/2002/07/owl#ObjectProperty> ;
        <http://www.w3.org/2000/01/rdf-schema#comment>
                "Connects a Record Set and a Record State that categorizes all\n            the Records or Record Parts that are or were included in the Record Set."@en ;
        <http://www.w3.org/2000/01/rdf-schema#domain>
                <https://www.ica.org/standards/RiC/ontology#RecordSet> ;
        <http://www.w3.org/2000/01/rdf-schema#isDefinedBy>
                <https://www.ica.org/standards/RiC/ontology> ;
        <http://www.w3.org/2000/01/rdf-schema#label>
                "has of had all members with record state"@en ;
        <http://www.w3.org/2000/01/rdf-schema#range>
                <https://www.ica.org/standards/RiC/ontology#RecordState> ;
        <http://www.w3.org/2000/01/rdf-schema#subPropertyOf>
                <https://www.ica.org/standards/RiC/ontology#hasOrHadAllMembersWithCategory> ;
        <http://www.w3.org/2000/01/rdf-schema#subPropertyOf>
                []  ;
        <http://www.w3.org/2002/07/owl#equivalentProperty>
                []  ;
        <http://www.w3.org/2002/07/owl#inverseOf>
                <https://www.ica.org/standards/RiC/ontology#isOrWasRecordStateOfAllMembersOf> ;
        <http://www.w3.org/2004/02/skos/core#changeNote>
                []  .

<https://www.ica.org/standards/RiC/ontology#isOrWasRecordStateOfAllMembersOf>
        a       <http://www.w3.org/2002/07/owl#ObjectProperty> ;
        <http://www.w3.org/2000/01/rdf-schema#comment>
                "Connects a Record State and a Record Set whose all past or\n            present Record or Record Part members have that Record State."@en ;
        <http://www.w3.org/2000/01/rdf-schema#domain>
                <https://www.ica.org/standards/RiC/ontology#RecordState> ;
        <http://www.w3.org/2000/01/rdf-schema#isDefinedBy>
                <https://www.ica.org/standards/RiC/ontology> ;
        <http://www.w3.org/2000/01/rdf-schema#label>
                "is or was record state of all members of"@en ;
        <http://www.w3.org/2000/01/rdf-schema#range>
                <https://www.ica.org/standards/RiC/ontology#RecordSet> ;
        <http://www.w3.org/2000/01/rdf-schema#subPropertyOf>
                <https://www.ica.org/standards/RiC/ontology#isOrWasCategoryOfAllMembersOf> ;
        <http://www.w3.org/2000/01/rdf-schema#subPropertyOf>
                []  ;
        <http://www.w3.org/2004/02/skos/core#changeNote>
                []  .

<https://www.ica.org/standards/RiC/ontology#isOrWasRecordStateOfSomeMembersOf>
        a       <http://www.w3.org/2002/07/owl#ObjectProperty> ;
        <http://www.w3.org/2000/01/rdf-schema#comment>
                "Connects a Record State and a Record Set whose some past or\n            present Record or Record Part members have that Record State."@en ;
        <http://www.w3.org/2000/01/rdf-schema#domain>
                <https://www.ica.org/standards/RiC/ontology#RecordState> ;
        <http://www.w3.org/2000/01/rdf-schema#isDefinedBy>
                <https://www.ica.org/standards/RiC/ontology> ;
        <http://www.w3.org/2000/01/rdf-schema#label>
                "is or was record state of some members of"@en ;
        <http://www.w3.org/2000/01/rdf-schema#range>
                <https://www.ica.org/standards/RiC/ontology#RecordSet> ;
        <http://www.w3.org/2000/01/rdf-schema#subPropertyOf>
                <https://www.ica.org/standards/RiC/ontology#isOrWasCategoryOfSomeMembersOf> ;
        <http://www.w3.org/2000/01/rdf-schema#subPropertyOf>
                []  ;
        <http://www.w3.org/2004/02/skos/core#changeNote>
                []  .

<https://www.ica.org/standards/RiC/ontology#RecordState>
        a       <http://www.w3.org/2002/07/owl#Class> ;
        <http://www.w3.org/2000/01/rdf-schema#comment>
                "Categorization of the production or reproduction status of a\n            Record or Record Part."@en ;
        <http://www.w3.org/2000/01/rdf-schema#isDefinedBy>
                <https://www.ica.org/standards/RiC/ontology> ;
        <http://www.w3.org/2000/01/rdf-schema#label>
                "Record State"@en ;
        <http://www.w3.org/2000/01/rdf-schema#subClassOf>
                <https://www.ica.org/standards/RiC/ontology#Type> ;
        <http://www.w3.org/2004/02/skos/core#scopeNote>
                "Can in particular refer to a record state of development or\n            its status of transmission once finished (draft, original, copy...). Specifying that a\n            record resource has state copy usually implies that another record resource existed or\n            exists, of which the one described is the copy. In such a case you can also use 'is copy\n            of' object property."@en ;
        <https://www.ica.org/standards/RiC/ontology#RiCCMCorrespondingComponent>
                "Corresponds to RiC-A39 (State\n            attribute)"@en .
