<https://d-nb.info/standards/elementset/gnd#academicDegree>
        a       <http://www.w3.org/2002/07/owl#DatatypeProperty> , <http://www.w3.org/2002/07/owl#ObjectProperty> ;
        <http://www.w3.org/2000/01/rdf-schema#comment>
                "An academic degree."@en , "Ein Rang, der als Bestätigung für wissenschaftliche Leistungen verliehen wird."@de ;
        <http://www.w3.org/2000/01/rdf-schema#domain>
                <https://d-nb.info/standards/elementset/gnd#DifferentiatedPerson> ;
        <http://www.w3.org/2000/01/rdf-schema#isDefinedBy>
                <https://d-nb.info/standards/elementset/gnd#> ;
        <http://www.w3.org/2000/01/rdf-schema#label>
                "Akademischer Grad"@de , "Academic degree"@en ;
        <http://www.w3.org/2000/01/rdf-schema#subPropertyOf>
                <http://xmlns.com/foaf/0.1/title> , <http://www.w3.org/2002/07/owl#topDataProperty> ;
        <https://d-nb.info/standards/elementset/gnd#marc21equivalent>
                "550 $a $g $4=akad" .

<https://d-nb.info/standards/elementset/gnd#placeOfBirthAsLiteral>
        a       <http://www.w3.org/2002/07/owl#ObjectProperty> , <http://www.w3.org/2002/07/owl#DatatypeProperty> , <http://www.w3.org/2002/07/owl#AnnotationProperty> ;
        <http://www.w3.org/2000/01/rdf-schema#comment>
                "This property is equivalent to gndo:placeOfBirth but gives a literal instead of\n\t\ta reference to a geographic entity"@en , "Diese Property ist äquivalent zu gndo:placeOfBirth, zeigt aber ein Literal\n\t\tstatt einer Referenz zu einer geografischen Entität"@de ;
        <http://www.w3.org/2000/01/rdf-schema#domain>
                <https://d-nb.info/standards/elementset/gnd#DifferentiatedPerson> ;
        <http://www.w3.org/2000/01/rdf-schema#isDefinedBy>
                <https://d-nb.info/standards/elementset/gnd#> ;
        <http://www.w3.org/2000/01/rdf-schema#label>
                "Place of Birth (Literal)"@en , "Geburtsort (Literal)"@de ;
        <http://www.w3.org/2000/01/rdf-schema#seeAlso>
                <https://d-nb.info/standards/elementset/gnd#placeOfBirth> ;
        <http://www.w3.org/2000/01/rdf-schema#subPropertyOf>
                <http://rdaregistry.info/Elements/a/P50119> , <http://www.w3.org/2002/07/owl#topDataProperty> , <https://d-nb.info/standards/elementset/gnd#associatedPlace> ;
        <https://d-nb.info/standards/elementset/gnd#marc21equivalent>
                "551 $a $g $z $4=ortg" .

<https://d-nb.info/standards/elementset/gnd#titleOfNobilityAsLiteral>
        a       <http://www.w3.org/2002/07/owl#DatatypeProperty> , <http://www.w3.org/2002/07/owl#ObjectProperty> ;
        <http://www.w3.org/2000/01/rdf-schema#comment>
                "Adelstitel einer Person oder Adelstitel im Erbtitel\n\t\teiner Familie. Diese Property ist äquivalent zu gndo:titleOfNobility, zeigt\n\t\taber ein Literal statt einer Referenz zu einem Schlagwort."@de , "A title of nobility held by a person or family.\n\t\tThis property is equivalent to gndo:titleOfNobility\n\t\tbut gives a literal instead of a reference to a subject heading."@en ;
        <http://www.w3.org/2000/01/rdf-schema#domain>
                <https://d-nb.info/standards/elementset/gnd#DifferentiatedPerson> ;
        <http://www.w3.org/2000/01/rdf-schema#isDefinedBy>
                <https://d-nb.info/standards/elementset/gnd#> ;
        <http://www.w3.org/2000/01/rdf-schema#label>
                "Title of nobility (Literal)"@en , "Adelstitel (Literal)"@de ;
        <http://www.w3.org/2000/01/rdf-schema#seeAlso>
                <https://d-nb.info/standards/elementset/gnd#titleOfNobility> ;
        <http://www.w3.org/2000/01/rdf-schema#subPropertyOf>
                <http://www.w3.org/2002/07/owl#topDataProperty> , <http://rdaregistry.info/Elements/a/P50059> , <http://rdaregistry.info/Elements/a/P50110> , <http://xmlns.com/foaf/0.1/title> ;
        <https://d-nb.info/standards/elementset/gnd#marc21equivalent>
                "550 $a $g $4=adel" .

<https://d-nb.info/standards/elementset/gnd#realIdentity>
        a       <http://www.w3.org/2002/07/owl#ObjectProperty> ;
        <http://www.w3.org/2000/01/rdf-schema#comment>
                "Links an identity under which one or more persons act, e. g. write, compose or create art, but that is not their real name (i. e. a pseudonym) to their real identity."@en , "Verknüpft eine Identität, unter der eine oder mehrere Personen agieren, z. B. schreiben, komponieren oder Kunstwerke schaffen, aber die nicht der wirkliche Name der Person ist (Pseudonym), mit der echten Identität der Person."@de ;
        <http://www.w3.org/2000/01/rdf-schema#domain>
                <https://d-nb.info/standards/elementset/gnd#DifferentiatedPerson> ;
        <http://www.w3.org/2000/01/rdf-schema#isDefinedBy>
                <https://d-nb.info/standards/elementset/gnd#> ;
        <http://www.w3.org/2000/01/rdf-schema#label>
                "Echte Identität"@de , "Real identity"@en ;
        <http://www.w3.org/2000/01/rdf-schema#range>
                <https://d-nb.info/standards/elementset/gnd#DifferentiatedPerson> ;
        <http://www.w3.org/2000/01/rdf-schema#subPropertyOf>
                <http://rdaregistry.info/Elements/a/P50106> , <https://d-nb.info/standards/elementset/gnd#relatedPerson> ;
        <http://www.w3.org/2000/01/rdf-schema#subPropertyOf>
                []  ;
        <http://www.w3.org/2000/01/rdf-schema#subPropertyOf>
                []  ;
        <http://www.w3.org/2002/07/owl#inverseOf>
                <https://d-nb.info/standards/elementset/gnd#pseudonym> ;
        <https://d-nb.info/standards/elementset/gnd#marc21equivalent>
                "500 $0 $4=nawi" .

<https://d-nb.info/standards/elementset/gnd#SubjectHeading>
        a       <http://www.w3.org/2002/07/owl#Class> ;
        <http://www.w3.org/2000/01/rdf-schema#isDefinedBy>
                <https://d-nb.info/standards/elementset/gnd#> ;
        <http://www.w3.org/2000/01/rdf-schema#label>
                "Subject heading"@en , "Schlagwort"@de ;
        <http://www.w3.org/2000/01/rdf-schema#subClassOf>
                <https://d-nb.info/standards/elementset/gnd#AuthorityResource> ;
        <https://d-nb.info/standards/elementset/gnd#marc21equivalent>
                "079 $v=szz" , "079 $b=s" .

<https://d-nb.info/standards/elementset/gnd#Work>
        a       <http://www.w3.org/2002/07/owl#Class> ;
        <http://www.w3.org/2000/01/rdf-schema#isDefinedBy>
                <https://d-nb.info/standards/elementset/gnd#> ;
        <http://www.w3.org/2000/01/rdf-schema#label>
                "Work"@en , "Werk"@de ;
        <http://www.w3.org/2000/01/rdf-schema#subClassOf>
                <https://d-nb.info/standards/elementset/gnd#AuthorityResource> ;
        <https://d-nb.info/standards/elementset/gnd#marc21equivalent>
                "079 $v=wit" , "079 $b=u" .

<https://d-nb.info/standards/elementset/gnd#memberOfTheFamily>
        a       <http://www.w3.org/2002/07/owl#ObjectProperty> , <http://www.w3.org/2002/07/owl#AnnotationProperty> ;
        <http://www.w3.org/2000/01/rdf-schema#comment>
                "Die beschriebene Person (Subjekt) ist ein bedeutendes \n\tMitglied der verknüpften Familie (Objekt). Für Göttergruppen und Gruppen\n\tmythologischer Gestalten wird gndo:broaderTermPartitive verwendet."@de ;
        <http://www.w3.org/2000/01/rdf-schema#domain>
                <https://d-nb.info/standards/elementset/gnd#DifferentiatedPerson> ;
        <http://www.w3.org/2000/01/rdf-schema#isDefinedBy>
                <https://d-nb.info/standards/elementset/gnd#> ;
        <http://www.w3.org/2000/01/rdf-schema#label>
                "Member of the family"@en , "Familienmitglied"@de ;
        <http://www.w3.org/2000/01/rdf-schema#range>
                <https://d-nb.info/standards/elementset/gnd#Family> ;
        <http://www.w3.org/2000/01/rdf-schema#seeAlso>
                <https://d-nb.info/standards/elementset/gnd#broaderTermPartitive> ;
        <http://www.w3.org/2000/01/rdf-schema#subPropertyOf>
                <https://d-nb.info/standards/elementset/gnd#member> , <http://rdaregistry.info/Elements/a/P50056> , <https://d-nb.info/standards/elementset/agrelon#isMemberOf> ;
        <https://d-nb.info/standards/elementset/gnd#marc21equivalent>
                "500 $0 $4=mitg" .

<https://d-nb.info/standards/elementset/gnd#pseudonym>
        a       <http://www.w3.org/2002/07/owl#ObjectProperty> ;
        <http://www.w3.org/2000/01/rdf-schema#comment>
                "Verknüpft eine echte Identität einer Person mit einer Identität, unter der eine oder mehrere Personen agieren, z. B. schreiben, komponieren oder Kunstwerke schaffen, aber die nicht der wirkliche Name der Person ist (Pseudonym)."@de , "Links a person's real identity to an identity under which one or more persons act, e. g. write, compose or create art, but that is not the person's real name (i. e. a pseudonym)."@en ;
        <http://www.w3.org/2000/01/rdf-schema#domain>
                <https://d-nb.info/standards/elementset/gnd#DifferentiatedPerson> ;
        <http://www.w3.org/2000/01/rdf-schema#isDefinedBy>
                <https://d-nb.info/standards/elementset/gnd#> ;
        <http://www.w3.org/2000/01/rdf-schema#label>
                "Pseudonym"@en , "Pseudonym"@de ;
        <http://www.w3.org/2000/01/rdf-schema#range>
                <https://d-nb.info/standards/elementset/gnd#DifferentiatedPerson> ;
        <http://www.w3.org/2000/01/rdf-schema#subPropertyOf>
                <http://rdaregistry.info/Elements/a/P50105> , <https://d-nb.info/standards/elementset/gnd#relatedPerson> ;
        <http://www.w3.org/2000/01/rdf-schema#subPropertyOf>
                []  ;
        <http://www.w3.org/2000/01/rdf-schema#subPropertyOf>
                []  ;
        <http://www.w3.org/2002/07/owl#equivalentProperty>
                []  ;
        <https://d-nb.info/standards/elementset/gnd#marc21equivalent>
                "500 $0 $4=pseu" .

<https://d-nb.info/standards/elementset/gnd#compiler>
        a       <http://www.w3.org/2002/07/owl#ObjectProperty> ;
        <http://www.w3.org/2000/01/rdf-schema#comment>
                "A person, family, or organization responsible for creating a new work (e.g., a bibliography, a directory) through the act of compilation, e.g., selecting, arranging, aggregating, and editing data, information, etc"@en ;
        <http://www.w3.org/2000/01/rdf-schema#domain>
                <https://d-nb.info/standards/elementset/gnd#Work> ;
        <http://www.w3.org/2000/01/rdf-schema#isDefinedBy>
                <https://d-nb.info/standards/elementset/gnd#> ;
        <http://www.w3.org/2000/01/rdf-schema#label>
                "Kompilator"@de , "Compiler"@en ;
        <http://www.w3.org/2000/01/rdf-schema#range>
                <https://d-nb.info/standards/elementset/gnd#DifferentiatedPerson> ;
        <http://www.w3.org/2000/01/rdf-schema#subPropertyOf>
                <http://rdaregistry.info/Elements/u/P60428> ;
        <https://d-nb.info/standards/elementset/gnd#marc21equivalent>
                "500 $0 $4=comp" .

<https://d-nb.info/standards/elementset/gnd#Family>
        a       <http://www.w3.org/2002/07/owl#Class> ;
        <http://www.w3.org/2000/01/rdf-schema#isDefinedBy>
                <https://d-nb.info/standards/elementset/gnd#> ;
        <http://www.w3.org/2000/01/rdf-schema#label>
                "Family"@en , "Familie"@de ;
        <http://www.w3.org/2000/01/rdf-schema#subClassOf>
                <https://d-nb.info/standards/elementset/gnd#AuthorityResource> , <http://rdaregistry.info/Elements/c/C10008> ;
        <https://d-nb.info/standards/elementset/gnd#marc21equivalent>
                "079 $v=pif" .

<https://d-nb.info/standards/elementset/gnd#DifferentiatedPerson>
        a       <http://www.w3.org/2002/07/owl#Class> ;
        <http://www.w3.org/2000/01/rdf-schema#isDefinedBy>
                <https://d-nb.info/standards/elementset/gnd#> ;
        <http://www.w3.org/2000/01/rdf-schema#label>
                "Differentiated person"@en , "Individualisierte Person"@de ;
        <http://www.w3.org/2000/01/rdf-schema#subClassOf>
                <https://d-nb.info/standards/elementset/gnd#Person> , <http://xmlns.com/foaf/0.1/Person> , <http://rdaregistry.info/Elements/c/C10004> ;
        <http://www.w3.org/2002/07/owl#disjointWith>
                <https://d-nb.info/standards/elementset/gnd#UndifferentiatedPerson> ;
        <https://d-nb.info/standards/elementset/gnd#marc21equivalent>
                "079 $v=piz" , "079 $b=p" .

<https://d-nb.info/standards/elementset/gnd#narrator>
        a       <http://www.w3.org/2002/07/owl#ObjectProperty> , <http://www.w3.org/2002/07/owl#AnnotationProperty> ;
        <http://www.w3.org/2000/01/rdf-schema#comment>
                "A performer contributing to a resource by reading or speaking in order to give an account of an act, occurrence, course of events, etc"@en ;
        <http://www.w3.org/2000/01/rdf-schema#domain>
                <https://d-nb.info/standards/elementset/gnd#Work> ;
        <http://www.w3.org/2000/01/rdf-schema#isDefinedBy>
                <https://d-nb.info/standards/elementset/gnd#> ;
        <http://www.w3.org/2000/01/rdf-schema#label>
                "Sprecher"@de , "Narrator"@en ;
        <http://www.w3.org/2000/01/rdf-schema#range>
                <https://d-nb.info/standards/elementset/gnd#DifferentiatedPerson> ;
        <http://www.w3.org/2000/01/rdf-schema#subPropertyOf>
                <http://www.w3.org/2002/07/owl#topObjectProperty> , <http://rdaregistry.info/Elements/u/P60153> ;
        <https://d-nb.info/standards/elementset/gnd#marc21equivalent>
                "500 $0 $4=spre" .

<https://d-nb.info/standards/elementset/gnd#titleOfNobility>
        a       <http://www.w3.org/2002/07/owl#ObjectProperty> ;
        <http://www.w3.org/2000/01/rdf-schema#comment>
                "A title of nobility held by a person or family."@en , "Adelstitel einer Person oder einer Familie."@de ;
        <http://www.w3.org/2000/01/rdf-schema#domain>
                <https://d-nb.info/standards/elementset/gnd#DifferentiatedPerson> ;
        <http://www.w3.org/2000/01/rdf-schema#isDefinedBy>
                <https://d-nb.info/standards/elementset/gnd#> ;
        <http://www.w3.org/2000/01/rdf-schema#label>
                "Title of nobility"@en , "Adelstitel"@de ;
        <http://www.w3.org/2000/01/rdf-schema#range>
                <https://d-nb.info/standards/elementset/gnd#SubjectHeading> ;
        <http://www.w3.org/2000/01/rdf-schema#seeAlso>
                <https://d-nb.info/standards/elementset/gnd#titleOfNobilityAsLiteral> ;
        <http://www.w3.org/2000/01/rdf-schema#subPropertyOf>
                <http://rdaregistry.info/Elements/a/P50110> , <http://xmlns.com/foaf/0.1/title> , <http://rdaregistry.info/Elements/a/P50059> ;
        <https://d-nb.info/standards/elementset/gnd#marc21equivalent>
                "550 $0 $4=adel" .

<https://d-nb.info/standards/elementset/gnd#placeOfDeathAsLiteral>
        a       <http://www.w3.org/2002/07/owl#AnnotationProperty> , <http://www.w3.org/2002/07/owl#ObjectProperty> , <http://www.w3.org/2002/07/owl#DatatypeProperty> ;
        <http://www.w3.org/2000/01/rdf-schema#comment>
                "This property is equivalent to gndo:placeOfDeath but gives a literal instead of\n\t\ta reference to a geographic entity"@en , "Diese Property ist äquivalent zu gndo:placeOfDeath, zeigt aber ein Literal\n\t\tstatt einer Referenz zu einer geografischen Entität"@de ;
        <http://www.w3.org/2000/01/rdf-schema#domain>
                <https://d-nb.info/standards/elementset/gnd#DifferentiatedPerson> ;
        <http://www.w3.org/2000/01/rdf-schema#isDefinedBy>
                <https://d-nb.info/standards/elementset/gnd#> ;
        <http://www.w3.org/2000/01/rdf-schema#label>
                "Sterbeort (Literal)"@de , "Place of death (Literal)"@en ;
        <http://www.w3.org/2000/01/rdf-schema#seeAlso>
                <https://d-nb.info/standards/elementset/gnd#placeOfDeath> ;
        <http://www.w3.org/2000/01/rdf-schema#subPropertyOf>
                <http://www.w3.org/2002/07/owl#topDataProperty> , <https://d-nb.info/standards/elementset/gnd#associatedPlace> , <http://rdaregistry.info/Elements/a/P50118> ;
        <https://d-nb.info/standards/elementset/gnd#marc21equivalent>
                "551 $a $g $z $4=orts" .
