<https://www.ica.org/standards/RiC/ontology#isFunctionallyEquivalentTo>
        a       <http://www.w3.org/2002/07/owl#ObjectProperty> , <http://www.w3.org/2002/07/owl#SymmetricProperty> ;
        <http://www.w3.org/2000/01/rdf-schema#comment>
                "Connects two Instantiations which may be considered as\n            equivalent. This relation is symmetric."@en ;
        <http://www.w3.org/2000/01/rdf-schema#domain>
                <https://www.ica.org/standards/RiC/ontology#Instantiation> ;
        <http://www.w3.org/2000/01/rdf-schema#isDefinedBy>
                <https://www.ica.org/standards/RiC/ontology> ;
        <http://www.w3.org/2000/01/rdf-schema#label>
                "is functionally equivalent to"@en ;
        <http://www.w3.org/2000/01/rdf-schema#range>
                <https://www.ica.org/standards/RiC/ontology#Instantiation> ;
        <http://www.w3.org/2000/01/rdf-schema#subPropertyOf>
                <https://www.ica.org/standards/RiC/ontology#isInstantiationAssociatedWithInstantiation> , <https://www.ica.org/standards/RiC/ontology#isEquivalentTo> ;
        <http://www.w3.org/2000/01/rdf-schema#subPropertyOf>
                []  ;
        <http://www.w3.org/2000/01/rdf-schema#subPropertyOf>
                []  ;
        <http://www.w3.org/2002/07/owl#equivalentProperty>
                []  ;
        <http://www.w3.org/2002/07/owl#inverseOf>
                <https://www.ica.org/standards/RiC/ontology#isFunctionallyEquivalentTo> ;
        <http://www.w3.org/2002/07/owl#propertyChainAxiom>
                []  ;
        <http://www.w3.org/2004/02/skos/core#changeNote>
                []  ;
        <http://www.w3.org/2004/02/skos/core#scopeNote>
                "Two Instantiations, from some point of view, may be considered\n            as equivalent. This equivalence is usually based upon the fact that the Instantiations\n            have at least the same intellectual content (they instantiate the same Record\n            Resource)."@en ;
        <https://www.ica.org/standards/RiC/ontology#RiCCMCorrespondingComponent>
                "RiC-R035 ('is functionally equivalent to'\n            relation)"@en .

<https://www.ica.org/standards/RiC/ontology#hasOrHadComponent>
        a       <http://www.w3.org/2002/07/owl#ObjectProperty> ;
        <http://www.w3.org/2000/01/rdf-schema#comment>
                "Connects an Instantiation to one of its present or past\n            component instantiations."@en ;
        <http://www.w3.org/2000/01/rdf-schema#domain>
                <https://www.ica.org/standards/RiC/ontology#Instantiation> ;
        <http://www.w3.org/2000/01/rdf-schema#isDefinedBy>
                <https://www.ica.org/standards/RiC/ontology> ;
        <http://www.w3.org/2000/01/rdf-schema#label>
                "has or had component"@en ;
        <http://www.w3.org/2000/01/rdf-schema#range>
                <https://www.ica.org/standards/RiC/ontology#Instantiation> ;
        <http://www.w3.org/2000/01/rdf-schema#subPropertyOf>
                <https://www.ica.org/standards/RiC/ontology#isInstantiationAssociatedWithInstantiation> , <https://www.ica.org/standards/RiC/ontology#hasOrHadPart> ;
        <http://www.w3.org/2000/01/rdf-schema#subPropertyOf>
                []  ;
        <http://www.w3.org/2000/01/rdf-schema#subPropertyOf>
                []  ;
        <http://www.w3.org/2002/07/owl#equivalentProperty>
                []  ;
        <http://www.w3.org/2002/07/owl#inverseOf>
                <https://www.ica.org/standards/RiC/ontology#isOrWasComponentOf> ;
        <http://www.w3.org/2004/02/skos/core#changeNote>
                []  ;
        <https://www.ica.org/standards/RiC/ontology#RiCCMCorrespondingComponent>
                "RiC-R004 ('has or had component'\n            relation)"@en .

<https://www.ica.org/standards/RiC/ontology#isDerivedFromInstantiation>
        a       <http://www.w3.org/2002/07/owl#ObjectProperty> ;
        <http://www.w3.org/2000/01/rdf-schema#comment>
                "Inverse of 'has derived instantiation' object\n            property."@en ;
        <http://www.w3.org/2000/01/rdf-schema#domain>
                <https://www.ica.org/standards/RiC/ontology#Instantiation> ;
        <http://www.w3.org/2000/01/rdf-schema#isDefinedBy>
                <https://www.ica.org/standards/RiC/ontology> ;
        <http://www.w3.org/2000/01/rdf-schema#label>
                "is derived from instantiation "@en ;
        <http://www.w3.org/2000/01/rdf-schema#range>
                <https://www.ica.org/standards/RiC/ontology#Instantiation> ;
        <http://www.w3.org/2000/01/rdf-schema#subPropertyOf>
                <https://www.ica.org/standards/RiC/ontology#followsInTime> , <https://www.ica.org/standards/RiC/ontology#isInstantiationAssociatedWithInstantiation> ;
        <http://www.w3.org/2000/01/rdf-schema#subPropertyOf>
                []  ;
        <http://www.w3.org/2000/01/rdf-schema#subPropertyOf>
                []  ;
        <https://www.ica.org/standards/RiC/ontology#RiCCMCorrespondingComponent>
                "RiC-R014i ('is derived from instantiation'\n            relation)"@en .

<https://www.ica.org/standards/RiC/ontology#hasDerivedInstantiation>
        a       <http://www.w3.org/2002/07/owl#ObjectProperty> ;
        <http://www.w3.org/2000/01/rdf-schema#comment>
                "Connects an Instantiation to an Instantiation that is derived\n            from it."@en ;
        <http://www.w3.org/2000/01/rdf-schema#domain>
                <https://www.ica.org/standards/RiC/ontology#Instantiation> ;
        <http://www.w3.org/2000/01/rdf-schema#isDefinedBy>
                <https://www.ica.org/standards/RiC/ontology> ;
        <http://www.w3.org/2000/01/rdf-schema#label>
                "has derived instantiation "@en ;
        <http://www.w3.org/2000/01/rdf-schema#range>
                <https://www.ica.org/standards/RiC/ontology#Instantiation> ;
        <http://www.w3.org/2000/01/rdf-schema#subPropertyOf>
                <https://www.ica.org/standards/RiC/ontology#precedesInTime> , <https://www.ica.org/standards/RiC/ontology#isInstantiationAssociatedWithInstantiation> ;
        <http://www.w3.org/2000/01/rdf-schema#subPropertyOf>
                []  ;
        <http://www.w3.org/2000/01/rdf-schema#subPropertyOf>
                []  ;
        <http://www.w3.org/2002/07/owl#equivalentProperty>
                []  ;
        <http://www.w3.org/2002/07/owl#inverseOf>
                <https://www.ica.org/standards/RiC/ontology#isDerivedFromInstantiation> ;
        <http://www.w3.org/2002/07/owl#propertyChainAxiom>
                []  ;
        <https://www.ica.org/standards/RiC/ontology#RiCCMCorrespondingComponent>
                "RiC-R014 ('has derived instantiation'\n            relation)"@en .

<https://www.ica.org/standards/RiC/ontology#instantiationStructure>
        a       <http://www.w3.org/2002/07/owl#DatatypeProperty> ;
        <http://www.w3.org/2000/01/rdf-schema#comment>
                "Information about the physical arrangement and composition of an\n            Instantiation."@en ;
        <http://www.w3.org/2000/01/rdf-schema#domain>
                <https://www.ica.org/standards/RiC/ontology#Instantiation> ;
        <http://www.w3.org/2000/01/rdf-schema#isDefinedBy>
                <https://www.ica.org/standards/RiC/ontology> ;
        <http://www.w3.org/2000/01/rdf-schema#label>
                "Instantiation structure"@en ;
        <http://www.w3.org/2000/01/rdf-schema#range>
                <http://www.w3.org/2000/01/rdf-schema#Literal> ;
        <http://www.w3.org/2000/01/rdf-schema#subPropertyOf>
                <https://www.ica.org/standards/RiC/ontology#structure> ;
        <http://www.w3.org/2004/02/skos/core#changeNote>
                []  ;
        <https://www.ica.org/standards/RiC/ontology#RiCCMCorrespondingComponent>
                "Specialization of RiC-A40 (Structure\n            attribute)"@en .

<https://www.ica.org/standards/RiC/ontology#isOrWasComponentOf>
        a       <http://www.w3.org/2002/07/owl#ObjectProperty> ;
        <http://www.w3.org/2000/01/rdf-schema#comment>
                "Inverse of 'has or had component' object\n            property."@en ;
        <http://www.w3.org/2000/01/rdf-schema#domain>
                <https://www.ica.org/standards/RiC/ontology#Instantiation> ;
        <http://www.w3.org/2000/01/rdf-schema#isDefinedBy>
                <https://www.ica.org/standards/RiC/ontology> ;
        <http://www.w3.org/2000/01/rdf-schema#label>
                "is or was component of"@en ;
        <http://www.w3.org/2000/01/rdf-schema#range>
                <https://www.ica.org/standards/RiC/ontology#Instantiation> ;
        <http://www.w3.org/2000/01/rdf-schema#subPropertyOf>
                <https://www.ica.org/standards/RiC/ontology#isInstantiationAssociatedWithInstantiation> , <https://www.ica.org/standards/RiC/ontology#isOrWasPartOf> ;
        <http://www.w3.org/2000/01/rdf-schema#subPropertyOf>
                []  ;
        <http://www.w3.org/2000/01/rdf-schema#subPropertyOf>
                []  ;
        <http://www.w3.org/2004/02/skos/core#changeNote>
                []  ;
        <https://www.ica.org/standards/RiC/ontology#RiCCMCorrespondingComponent>
                "RiC-R004i ('is or was component of'\n            relation)"@en .

<https://www.ica.org/standards/RiC/ontology#qualityOfRepresentation>
        a       <http://www.w3.org/2002/07/owl#DatatypeProperty> ;
        <http://www.w3.org/2000/01/rdf-schema#comment>
                "Conditions of an Instantiation that impact the legibility or\n            completeness of Record Resource, and thus the viability of its use. Conditions may be\n            associated with deficiencies in the processes of Record (re)creation or capture, or the\n            deterioration of the Instantiation (e.g. its carrier) causing loss of information of the\n            record over time"@en ;
        <http://www.w3.org/2000/01/rdf-schema#domain>
                <https://www.ica.org/standards/RiC/ontology#Instantiation> ;
        <http://www.w3.org/2000/01/rdf-schema#isDefinedBy>
                <https://www.ica.org/standards/RiC/ontology> ;
        <http://www.w3.org/2000/01/rdf-schema#label>
                "quality of representation"@en ;
        <http://www.w3.org/2000/01/rdf-schema#range>
                <http://www.w3.org/2000/01/rdf-schema#Literal> ;
        <http://www.w3.org/2000/01/rdf-schema#subPropertyOf>
                <http://www.w3.org/2002/07/owl#topDataProperty> ;
        <http://www.w3.org/2004/02/skos/core#changeNote>
                []  ;
        <http://www.w3.org/2004/02/skos/core#example>
                "some loss of text due to rodent damage"@en , "Black and white digitization may have led to loss of some\n            information."@en , "some loss of information due to poor quality of image\n            capture"@en ;
        <https://www.ica.org/standards/RiC/ontology#RiCCMCorrespondingComponent>
                "Corresponds to RiC-A34 (Quality of Representation\n            attribute)"@en .

<https://www.ica.org/standards/RiC/ontology#carrierExtent>
        a       <http://www.w3.org/2002/07/owl#DatatypeProperty> ;
        <http://www.w3.org/2000/01/rdf-schema#comment>
                "Number of physical units and/or physical dimensions of the\n            carrier of a record resource instantiation. Various carriers, depending on specific\n            needs, may have more than one relevant dimension. In some cases, indicating the number\n            of physical units may be sufficient, while in other case, relevant dimensions should be\n            used in order to characterize the carrier."@en ;
        <http://www.w3.org/2000/01/rdf-schema#domain>
                <https://www.ica.org/standards/RiC/ontology#Instantiation> ;
        <http://www.w3.org/2000/01/rdf-schema#isDefinedBy>
                <https://www.ica.org/standards/RiC/ontology> ;
        <http://www.w3.org/2000/01/rdf-schema#label>
                "carrier extent"@en ;
        <http://www.w3.org/2000/01/rdf-schema#range>
                <http://www.w3.org/2000/01/rdf-schema#Literal> ;
        <http://www.w3.org/2000/01/rdf-schema#subPropertyOf>
                <https://www.ica.org/standards/RiC/ontology#physicalOrLogicalExtent> ;
        <http://www.w3.org/2004/02/skos/core#changeNote>
                []  ;
        <http://www.w3.org/2004/02/skos/core#example>
                "2 pieces of parchment, 30 x 50 cm and 32,5 x 49\n            cm"@en , "3GB USB key"@en , "1 page"@en , "17 x 34.5 cm"@en ;
        <http://www.w3.org/2004/02/skos/core#scopeNote>
                "For electronic resources, it indicates the size of storage\n            capacity (disk, tape, film etc.). Carrier Extent should not be confused with Record\n            Resource Extent or Instantiation Extent. For a given Record Resource, the Instantiation\n            Extent may vary, based on format, density of information on the carrier, etc. For\n            example, 1500 words (Record Resource Extent) may have Instantiation Extent 3kb as a Word\n            document and 5kb as a PDF file, and instantiations may be represented on a CD of 700mb\n            (Carrier Extent). Use if you don't use CarrierExtent class and its properties for\n            handling such information."@en ;
        <https://www.ica.org/standards/RiC/ontology#RiCCMCorrespondingComponent>
                "Corresponds to RiC-A04 (Carrier Extent\n            attribute)"@en .

<https://www.ica.org/standards/RiC/ontology#productionTechnique>
        a       <http://www.w3.org/2002/07/owl#DatatypeProperty> ;
        <http://www.w3.org/2000/01/rdf-schema#comment>
                "Method used in the representation of information on the\n            Instantiation."@en ;
        <http://www.w3.org/2000/01/rdf-schema#domain>
                <https://www.ica.org/standards/RiC/ontology#Instantiation> ;
        <http://www.w3.org/2000/01/rdf-schema#isDefinedBy>
                <https://www.ica.org/standards/RiC/ontology> ;
        <http://www.w3.org/2000/01/rdf-schema#label>
                "production technique"@en ;
        <http://www.w3.org/2000/01/rdf-schema#range>
                <http://www.w3.org/2000/01/rdf-schema#Literal> ;
        <http://www.w3.org/2000/01/rdf-schema#subPropertyOf>
                <http://www.w3.org/2002/07/owl#topDataProperty> ;
        <http://www.w3.org/2004/02/skos/core#changeNote>
                []  ;
        <http://www.w3.org/2004/02/skos/core#example>
                "handwriting"@en , "engraving"@en , "optical recording"@en , "magnetic recording"@en ;
        <http://www.w3.org/2004/02/skos/core#scopeNote>
                "Use only if you have free text or don't have a controlled\n            vocabulary for production techniques (in this case, use the ProductionTechniqueType\n            class)"@en ;
        <https://www.ica.org/standards/RiC/ontology#RiCCMCorrespondingComponent>
                "Corresponds to RiC-A33 (Production Technique\n            attribute)"@en .

<https://www.ica.org/standards/RiC/ontology#migratedInto>
        a       <http://www.w3.org/2002/07/owl#ObjectProperty> ;
        <http://www.w3.org/2000/01/rdf-schema#comment>
                "Connects an Instantiation to a version it has been migrated\n            to."@en ;
        <http://www.w3.org/2000/01/rdf-schema#domain>
                <https://www.ica.org/standards/RiC/ontology#Instantiation> ;
        <http://www.w3.org/2000/01/rdf-schema#isDefinedBy>
                <https://www.ica.org/standards/RiC/ontology> ;
        <http://www.w3.org/2000/01/rdf-schema#label>
                "migrated into"@en ;
        <http://www.w3.org/2000/01/rdf-schema#range>
                <https://www.ica.org/standards/RiC/ontology#Instantiation> ;
        <http://www.w3.org/2000/01/rdf-schema#subPropertyOf>
                <https://www.ica.org/standards/RiC/ontology#hasDerivedInstantiation> ;
        <http://www.w3.org/2000/01/rdf-schema#subPropertyOf>
                []  ;
        <http://www.w3.org/2002/07/owl#propertyChainAxiom>
                []  ;
        <http://www.w3.org/2004/02/skos/core#changeNote>
                []  ;
        <http://www.w3.org/2004/02/skos/core#scopeNote>
                "Use for digital instantiations."@en ;
        <https://www.ica.org/standards/RiC/ontology#RiCCMCorrespondingComponent>
                "RiC-R015 ('migrated into'\n            relation)"@en .

<https://www.ica.org/standards/RiC/ontology#migratedFrom>
        a       <http://www.w3.org/2002/07/owl#ObjectProperty> ;
        <http://www.w3.org/2000/01/rdf-schema#comment>
                "Inverse of 'migrated into' object property."@en ;
        <http://www.w3.org/2000/01/rdf-schema#domain>
                <https://www.ica.org/standards/RiC/ontology#Instantiation> ;
        <http://www.w3.org/2000/01/rdf-schema#isDefinedBy>
                <https://www.ica.org/standards/RiC/ontology> ;
        <http://www.w3.org/2000/01/rdf-schema#label>
                "migrated from"@en ;
        <http://www.w3.org/2000/01/rdf-schema#range>
                <https://www.ica.org/standards/RiC/ontology#Instantiation> ;
        <http://www.w3.org/2000/01/rdf-schema#subPropertyOf>
                <https://www.ica.org/standards/RiC/ontology#isDerivedFromInstantiation> ;
        <http://www.w3.org/2000/01/rdf-schema#subPropertyOf>
                []  ;
        <http://www.w3.org/2002/07/owl#equivalentProperty>
                []  ;
        <http://www.w3.org/2002/07/owl#inverseOf>
                <https://www.ica.org/standards/RiC/ontology#migratedInto> ;
        <http://www.w3.org/2002/07/owl#propertyChainAxiom>
                []  ;
        <http://www.w3.org/2004/02/skos/core#changeNote>
                []  ;
        <https://www.ica.org/standards/RiC/ontology#RiCCMCorrespondingComponent>
                "RiC-R015i ('migrated from'\n            relation)"@en .

<https://www.ica.org/standards/RiC/ontology#Instantiation>
        a       <http://www.w3.org/2002/07/owl#Class> ;
        <http://www.w3.org/2000/01/rdf-schema#comment>
                "The inscription of information made by an Agent on a physical\n            carrier in any persistent, recoverable form as a means of communicating information\n            through time and space."@en ;
        <http://www.w3.org/2000/01/rdf-schema#isDefinedBy>
                <https://www.ica.org/standards/RiC/ontology> ;
        <http://www.w3.org/2000/01/rdf-schema#label>
                "Instantiation"@en ;
        <http://www.w3.org/2000/01/rdf-schema#subClassOf>
                <https://www.ica.org/standards/RiC/ontology#Thing> ;
        <http://www.w3.org/2004/02/skos/core#scopeNote>
                "A Record or Record Part must have been instantiated at least\n            once, though this instantiation may no longer exist at the moment of description. An\n            instantiation might also exist at the moment of description, but be destroyed at a later\n            moment in time, when, for example, a derived instantiation might become the only\n            remaining instantiation. A Record Set may have an instantiation, which is to say that it\n            is not a necessary condition. An Instantiation may be derived from another\n            Instantiation. A Record Resource may have many Instantiations simultaneously (for\n            instance, a record printed and saved in the same time as DOCX and PDF/A would have 3\n            concurrent instantiations) or through time (for example, copy of a record). Depending on\n            the context, a new instantiation may be seen as a new or as the same record resource.\n            During in the process of re-instantiation something is lost and something is preserved,\n            but it is up to the context and the Agent that produces or uses that Instantiation to\n            assess whether the two instantiations are functionally equivalent or not. For instance,\n            a postcard representing a town map from 1874 (Instantiation 1) is digitized and kept as\n            a JPEG file (Instantiation 2). The digital copy may be considered as instantiating the\n            \"same\" Record by an Agent considering the information transmitted by the Record (e.g.,\n            the urban landscape displayed), but as a\" different\" Record by an antiquarian more\n            focused on the materiality of the carrier. Successive instantiations may change the\n            perceivable boundaries of a Record Resource. For instance, a case file comprising many\n            records may be digitized and saved as one single PDF file, which, from management\n            perspective, may be treated as one Record. Similarly, a large Record Set (a fonds or a\n            series) may be maintained as one database. On the other hand, one record (main document\n            and its annexes) may be digitized in separate files and each one may be managed as a\n            discrete “physical” item. Instantiations may require mediation to communicate the\n            information in the Record Resource. While a traditional Record on paper can simply be\n            read by an Agent in order to understand the information, a vinyl recording, a video\n            cassette or a digital file needs a device (mediator) to codify or decodify the\n            information conveyed. This mediator may imply simple physical components (a turntable\n            needle, for example), or a complex gallery of software and hardware elements.\n            Instantiations are more than the mere informational content of Record Resource and may\n            be the focus of preservation and physical management of records. The use of particular\n            document types for records, such as a medieval charter, may have implications for the\n            authenticity of the records. Hence, the way a Record Resource is instantiated\n            contributes to the contextualizing of the content.record resource is instantiated\n            contributes to the contextualizing the content. Distinguishing the message conveyed\n            (Record Resource) and its physical representations (Instantiation) allows for the\n            efficient management of their descriptions, and preserve information about a Record\n            Resource even when no physical representation of it exists or is known to exist anymore.\n            The relations between distinct instantiations can then be expressed wherever they\n            coexist, and they can be related to the Record Resource they\n            instantiate."@en ;
        <https://www.ica.org/standards/RiC/ontology#RiCCMCorrespondingComponent>
                "Corresponds to RiC-E06 (Instantiation\n            entity)"@en ;
        <https://www.ica.org/standards/RiC/ontology#closeTo>
                "PREMIS Representation"@en .

<https://www.ica.org/standards/RiC/ontology#physicalCharacteristics>
        a       <http://www.w3.org/2002/07/owl#DatatypeProperty> ;
        <http://www.w3.org/2000/01/rdf-schema#comment>
                "Information about the physical features of the Instantiation.\n            Includes information about the physical nature and condition such as conservation\n            status."@en ;
        <http://www.w3.org/2000/01/rdf-schema#domain>
                <https://www.ica.org/standards/RiC/ontology#Instantiation> ;
        <http://www.w3.org/2000/01/rdf-schema#isDefinedBy>
                <https://www.ica.org/standards/RiC/ontology> ;
        <http://www.w3.org/2000/01/rdf-schema#label>
                "physical characteristics"@en ;
        <http://www.w3.org/2000/01/rdf-schema#range>
                <http://www.w3.org/2000/01/rdf-schema#Literal> ;
        <http://www.w3.org/2000/01/rdf-schema#subPropertyOf>
                <http://www.w3.org/2002/07/owl#topDataProperty> ;
        <http://www.w3.org/2004/02/skos/core#changeNote>
                []  ;
        <http://www.w3.org/2004/02/skos/core#example>
                "watermarked"@en , "emulsion flaking"@en , "carrier heavily foxed"@en , "British Library binding"@en ;
        <https://www.ica.org/standards/RiC/ontology#RiCCMCorrespondingComponent>
                "Corresponds to RiC-A31 (Physical Characteristics\n            attribute)"@en .

<https://www.ica.org/standards/RiC/ontology#isInstantiationAssociatedWithInstantiation>
        a       <http://www.w3.org/2002/07/owl#ObjectProperty> , <http://www.w3.org/2002/07/owl#SymmetricProperty> ;
        <http://www.w3.org/2000/01/rdf-schema#comment>
                "Connects two Instantiations. This object property is\n            symmetric."@en ;
        <http://www.w3.org/2000/01/rdf-schema#domain>
                <https://www.ica.org/standards/RiC/ontology#Instantiation> ;
        <http://www.w3.org/2000/01/rdf-schema#isDefinedBy>
                <https://www.ica.org/standards/RiC/ontology> ;
        <http://www.w3.org/2000/01/rdf-schema#label>
                "is instantiation associated with instantiation "@en ;
        <http://www.w3.org/2000/01/rdf-schema#range>
                <https://www.ica.org/standards/RiC/ontology#Instantiation> ;
        <http://www.w3.org/2000/01/rdf-schema#subPropertyOf>
                <https://www.ica.org/standards/RiC/ontology#isRelatedTo> ;
        <http://www.w3.org/2000/01/rdf-schema#subPropertyOf>
                []  ;
        <http://www.w3.org/2002/07/owl#equivalentProperty>
                []  ;
        <http://www.w3.org/2002/07/owl#inverseOf>
                <https://www.ica.org/standards/RiC/ontology#isInstantiationAssociatedWithInstantiation> ;
        <http://www.w3.org/2002/07/owl#propertyChainAxiom>
                []  ;
        <https://www.ica.org/standards/RiC/ontology#RiCCMCorrespondingComponent>
                "RiC-R034 ('is instantiation associated with\n            instantiation' relation)"@en .

<https://www.ica.org/standards/RiC/ontology#instantiationExtent>
        a       <http://www.w3.org/2002/07/owl#DatatypeProperty> ;
        <http://www.w3.org/2000/01/rdf-schema#comment>
                "Countable characteristics of the Instantiation expressed as a\n            quantity."@en ;
        <http://www.w3.org/2000/01/rdf-schema#domain>
                <https://www.ica.org/standards/RiC/ontology#Instantiation> ;
        <http://www.w3.org/2000/01/rdf-schema#isDefinedBy>
                <https://www.ica.org/standards/RiC/ontology> ;
        <http://www.w3.org/2000/01/rdf-schema#label>
                "Instantiation extent"@en ;
        <http://www.w3.org/2000/01/rdf-schema#range>
                <http://www.w3.org/2000/01/rdf-schema#Literal> ;
        <http://www.w3.org/2000/01/rdf-schema#subPropertyOf>
                <https://www.ica.org/standards/RiC/ontology#physicalOrLogicalExtent> ;
        <http://www.w3.org/2004/02/skos/core#changeNote>
                []  ;
        <http://www.w3.org/2004/02/skos/core#example>
                "Size of PDF-file: 1.5 MB"@en , "The book register has 345 written leaves."@en ;
        <http://www.w3.org/2004/02/skos/core#scopeNote>
                "For a given Record Resource, the Instantiation Extent may\n            vary, based on format, density of information on the carrier, etc. For example, a file\n            of 1500 words (Record Resource Extent) may have Instantiation Extent 3kb as a Word\n            document and 5kb as a PDF file, and instantiations may be represented on a CD of 700mb\n            (Carrier Extent). Use if you don't use InstantiationExtent class and its properties for\n            handling such information."@en ;
        <https://www.ica.org/standards/RiC/ontology#RiCCMCorrespondingComponent>
                "Corresponds to RiC-A23 (Instantiation Extent\n            attribute)"@en .
