<http://www.cidoc-crm.org/cidoc-crm/E52_Time-Span>
        a       <http://www.w3.org/2002/07/owl#Class> ;
        <http://www.w3.org/2000/01/rdf-schema#comment>
                "This class comprises abstract temporal extents, in the sense of Galilean physics, having a beginning, an end and a duration. \nTime Span has no other semantic connotations. Time-Spans are used to define the temporal extent of instances of E4 Period, E5 Event and any other phenomena valid for a certain time. An E52 Time-Span may be identified by one or more instances of E49 Time Appellation. \nSince our knowledge of history is imperfect, instances of E52 Time-Span can best be considered as approximations of the actual Time-Spans of temporal entities. The properties of E52 Time-Span are intended to allow these approximations to be expressed precisely.  An extreme case of approximation, might, for example, define an E52 Time-Span having unknown beginning, end and duration. Used as a common E52 Time-Span for two events, it would nevertheless define them as being simultaneous, even if nothing else was known. \n\tAutomatic processing and querying of instances of E52 Time-Span is facilitated if data can be parsed into an E61 Time Primitive.\n"@en ;
        <http://www.w3.org/2000/01/rdf-schema#label>
                "Χρονικό Διάστημα"@el , "Período de Tempo"@pt , "时段"@zh , "Time-Span"@en , "Zeitspanne"@de , "Durée"@fr , "Интервал Времени"@ru ;
        <http://www.w3.org/2000/01/rdf-schema#subClassOf>
                <http://www.cidoc-crm.org/cidoc-crm/E1_CRM_Entity> .

<http://www.cidoc-crm.org/cidoc-crm/E53_Place>
        a       <http://www.w3.org/2002/07/owl#Class> ;
        <http://www.w3.org/2000/01/rdf-schema#comment>
                "This class comprises extents in space, in particular on the surface of the earth, in the pure sense of physics: independent from temporal phenomena and matter. \nThe instances of E53 Place are usually determined by reference to the position of “immobile” objects such as buildings, cities, mountains, rivers, or dedicated geodetic marks. A Place can be determined by combining a frame of reference and a location with respect to this frame. It may be identified by one or more instances of E44 Place Appellation.\n It is sometimes argued that instances of E53 Place are best identified by global coordinates or absolute reference systems. However, relative references are often more relevant in the context of cultural documentation and tend to be more precise. In particular, we are often interested in position in relation to large, mobile objects, such as ships. For example, the Place at which Nelson died is known with reference to a large mobile object – H.M.S Victory. A resolution of this Place in terms of absolute coordinates would require knowledge of the movements of the vessel and the precise time of death, either of which may be revised, and the result would lack historical and cultural relevance.\nAny object can serve as a frame of reference for E53 Place determination. The model foresees the notion of a \"section\" of an E19 Physical Object as a valid E53 Place determination."@en ;
        <http://www.w3.org/2000/01/rdf-schema#label>
                "Place"@en , "Место"@ru , "Local"@pt , "Τόπος"@el , "地点"@zh , "Ort"@de , "Lieu"@fr ;
        <http://www.w3.org/2000/01/rdf-schema#subClassOf>
                <http://www.cidoc-crm.org/cidoc-crm/E1_CRM_Entity> .

<http://www.cidoc-crm.org/cidoc-crm/E92_Spacetime_Volume>
        a       <http://www.w3.org/2002/07/owl#Class> ;
        <http://www.w3.org/2000/01/rdf-schema#comment>
                "This class comprises 4 dimensional point sets (volumes) in physical spacetime regardless its true geometric form. They may derive their identity from being the extent of a material phenomenon or from being the interpretation of an expression defining an extent in spacetime. \n\tIntersections of instances of E92 Spacetime Volume, Place and Timespan are also regarded as instances of E92 Spacetime Volume.  An instance of E92 Spacetime Volume is either contiguous or composed of a finite number of contiguous subsets. \n\tIts boundaries may be fuzzy due to the properties of the phenomena it derives from or due to the limited precision up to which defining expression can be identified with a real extent in spacetime. The duration of existence of an instance of a spacetime volume is trivially its projection on time.\n"@en ;
        <http://www.w3.org/2000/01/rdf-schema#label>
                "Spacetime Volume"@en ;
        <http://www.w3.org/2000/01/rdf-schema#subClassOf>
                <http://www.cidoc-crm.org/cidoc-crm/E1_CRM_Entity> .

<http://www.cidoc-crm.org/cidoc-crm/P166i_had_presence>
        a       <http://www.w3.org/2002/07/owl#ObjectProperty> ;
        <http://www.w3.org/2000/01/rdf-schema#domain>
                <http://www.cidoc-crm.org/cidoc-crm/E92_Spacetime_Volume> ;
        <http://www.w3.org/2000/01/rdf-schema#label>
                "had presence"@en ;
        <http://www.w3.org/2000/01/rdf-schema#range>
                <http://www.cidoc-crm.org/cidoc-crm/E93_Presence> ;
        <http://www.w3.org/2000/01/rdf-schema#subPropertyOf>
                <http://www.w3.org/2002/07/owl#topObjectProperty> .

<http://www.cidoc-crm.org/cidoc-crm/P166_was_a_presence_of>
        a       <http://www.w3.org/2002/07/owl#ObjectProperty> ;
        <http://www.w3.org/2000/01/rdf-schema#comment>
                "This property relates an E93 Presence with the STV it is part of… \n\t"@en ;
        <http://www.w3.org/2000/01/rdf-schema#domain>
                <http://www.cidoc-crm.org/cidoc-crm/E93_Presence> ;
        <http://www.w3.org/2000/01/rdf-schema#label>
                "was a presence of"@en ;
        <http://www.w3.org/2000/01/rdf-schema#range>
                <http://www.cidoc-crm.org/cidoc-crm/E92_Spacetime_Volume> ;
        <http://www.w3.org/2000/01/rdf-schema#subPropertyOf>
                <http://www.w3.org/2002/07/owl#topObjectProperty> .

<http://www.cidoc-crm.org/cidoc-crm/P167i_was_place_of>
        a       <http://www.w3.org/2002/07/owl#ObjectProperty> ;
        <http://www.w3.org/2000/01/rdf-schema#domain>
                <http://www.cidoc-crm.org/cidoc-crm/E53_Place> ;
        <http://www.w3.org/2000/01/rdf-schema#label>
                "was place of"@en ;
        <http://www.w3.org/2000/01/rdf-schema#range>
                <http://www.cidoc-crm.org/cidoc-crm/E93_Presence> ;
        <http://www.w3.org/2000/01/rdf-schema#subPropertyOf>
                <http://www.w3.org/2002/07/owl#topObjectProperty> .

<http://www.cidoc-crm.org/cidoc-crm/P164i_was_time-span_of>
        a       <http://www.w3.org/2002/07/owl#ObjectProperty> ;
        <http://www.w3.org/2000/01/rdf-schema#domain>
                <http://www.cidoc-crm.org/cidoc-crm/E52_Time-Span> ;
        <http://www.w3.org/2000/01/rdf-schema#label>
                "was time-span of"@en ;
        <http://www.w3.org/2000/01/rdf-schema#range>
                <http://www.cidoc-crm.org/cidoc-crm/E93_Presence> ;
        <http://www.w3.org/2000/01/rdf-schema#subPropertyOf>
                <http://www.cidoc-crm.org/cidoc-crm/P160i_is_temporal_projection_of> .

<http://www.cidoc-crm.org/cidoc-crm/P167_at>
        a       <http://www.w3.org/2002/07/owl#ObjectProperty> ;
        <http://www.w3.org/2000/01/rdf-schema#comment>
                "This property points to a wider area in which my thing /event was… \n\t"@en ;
        <http://www.w3.org/2000/01/rdf-schema#domain>
                <http://www.cidoc-crm.org/cidoc-crm/E93_Presence> ;
        <http://www.w3.org/2000/01/rdf-schema#label>
                "at"@en ;
        <http://www.w3.org/2000/01/rdf-schema#range>
                <http://www.cidoc-crm.org/cidoc-crm/E53_Place> ;
        <http://www.w3.org/2000/01/rdf-schema#subPropertyOf>
                <http://www.w3.org/2002/07/owl#topObjectProperty> .

<http://www.cidoc-crm.org/cidoc-crm/E93_Presence>
        a       <http://www.w3.org/2002/07/owl#Class> ;
        <http://www.w3.org/2000/01/rdf-schema#comment>
                "This class comprises instances of E92 Spacetime Volume that result from intersection of instances of E92 Spacetime Volume with an instance of E52 Time-Span.  The identity of an instance of this class is determined by the identities of the  constituing spacetime volume and the time-span. \n\t\nThis class can be used to define temporal snapshots at a particular time-span, such as the extent of the Roman Empire at 33 B.C., or the extent occupied by a museum object at rest in an exhibit. In particular, it can be used to define the spatial projection of a spacetime volume during a particular time-span,  such as the maximal spatial extent of a flood at some particular hour, or all areas covered by the Poland within the 20th century AD.\n"@en ;
        <http://www.w3.org/2000/01/rdf-schema#label>
                "Presence"@en ;
        <http://www.w3.org/2000/01/rdf-schema#subClassOf>
                <http://www.cidoc-crm.org/cidoc-crm/E92_Spacetime_Volume> .
