<http://iflastandards.info/ns/fr/frbr/pressoo/Y12_separated_from>
        a       <http://www.w3.org/2002/07/owl#ObjectProperty> , <http://www.w3.org/2002/07/owl#AnnotationProperty> ;
        <http://www.w3.org/2000/01/rdf-schema#comment>
                "This property associates an instance of Z3 Separation with the instance of F18 Serial Work that was diminished through the separation."@en ;
        <http://www.w3.org/2000/01/rdf-schema#domain>
                <http://iflastandards.info/ns/fr/frbr/pressoo/Z3_Separation> ;
        <http://www.w3.org/2000/01/rdf-schema#label>
                "separated from"@en ;
        <http://www.w3.org/2000/01/rdf-schema#range>
                <http://iflastandards.info/ns/fr/frbr/frbroo/F18_Serial_Work> ;
        <http://www.w3.org/2000/01/rdf-schema#subPropertyOf>
                <http://www.w3.org/2002/07/owl#topObjectProperty> , <http://www.cidoc-crm.org/cidoc-crm/P12_occurred_in_the_presence_of> .

<http://iflastandards.info/ns/fr/frbr/frbroo/F18_Serial_Work>
        a       <http://www.w3.org/2002/07/owl#Class> ;
        <http://www.w3.org/2000/01/rdf-schema#subClassOf>
                <http://www.w3.org/2002/07/owl#Thing> .

<http://iflastandards.info/ns/fr/frbr/pressoo/Y12i_was_diminished_through>
        a       <http://www.w3.org/2002/07/owl#ObjectProperty> , <http://www.w3.org/2002/07/owl#AnnotationProperty> ;
        <http://www.w3.org/2000/01/rdf-schema#domain>
                <http://iflastandards.info/ns/fr/frbr/frbroo/F18_Serial_Work> ;
        <http://www.w3.org/2000/01/rdf-schema#label>
                "was diminished through"@en ;
        <http://www.w3.org/2000/01/rdf-schema#range>
                <http://iflastandards.info/ns/fr/frbr/pressoo/Z3_Separation> ;
        <http://www.w3.org/2000/01/rdf-schema#subPropertyOf>
                <http://www.w3.org/2002/07/owl#topObjectProperty> , <http://www.cidoc-crm.org/cidoc-crm/P12i_was_present_at> .

<http://iflastandards.info/ns/fr/frbr/pressoo/Y11_separated>
        a       <http://www.w3.org/2002/07/owl#ObjectProperty> , <http://www.w3.org/2002/07/owl#AnnotationProperty> ;
        <http://www.w3.org/2000/01/rdf-schema#comment>
                "This property associates an instance of Z3 Separation with an instance of F18 Serial Work that resulted from the separation."@en ;
        <http://www.w3.org/2000/01/rdf-schema#domain>
                <http://iflastandards.info/ns/fr/frbr/pressoo/Z3_Separation> ;
        <http://www.w3.org/2000/01/rdf-schema#label>
                "separated"@en ;
        <http://www.w3.org/2000/01/rdf-schema#range>
                <http://iflastandards.info/ns/fr/frbr/frbroo/F18_Serial_Work> ;
        <http://www.w3.org/2000/01/rdf-schema#subPropertyOf>
                <http://www.w3.org/2002/07/owl#topObjectProperty> , <http://iflastandards.info/ns/fr/frbr/frbroo/R16_initiated> .

<http://iflastandards.info/ns/fr/frbr/pressoo/Z3_Separation>
        a       <http://www.w3.org/2002/07/owl#Class> ;
        <http://www.w3.org/2000/01/rdf-schema#comment>
                "This class comprises activities that result in new instances of F18 Serial Work coming into being as the ‘offspring’ of pre-existing instances of F18 Serial Work that continue to be published after the separation has occurred."@en ;
        <http://www.w3.org/2000/01/rdf-schema#label>
                "Separation"@en ;
        <http://www.w3.org/2000/01/rdf-schema#subClassOf>
                <http://iflastandards.info/ns/fr/frbr/frbroo/F27_Work_Conception> .

<http://iflastandards.info/ns/fr/frbr/pressoo/Y11i_was_separated_through>
        a       <http://www.w3.org/2002/07/owl#ObjectProperty> , <http://www.w3.org/2002/07/owl#AnnotationProperty> ;
        <http://www.w3.org/2000/01/rdf-schema#domain>
                <http://iflastandards.info/ns/fr/frbr/frbroo/F18_Serial_Work> ;
        <http://www.w3.org/2000/01/rdf-schema#label>
                "was separated through"@en ;
        <http://www.w3.org/2000/01/rdf-schema#range>
                <http://iflastandards.info/ns/fr/frbr/pressoo/Z3_Separation> ;
        <http://www.w3.org/2000/01/rdf-schema#subPropertyOf>
                <http://www.w3.org/2002/07/owl#topObjectProperty> , <http://iflastandards.info/ns/fr/frbr/frbroo/R16i_was_initiated_by> .
