<http://www.cidoc-crm.org/cidoc-crm/E1_CRM_Entity>
        a       <http://www.w3.org/2002/07/owl#Class> ;
        <http://www.w3.org/2000/01/rdf-schema#subClassOf>
                <http://www.w3.org/2002/07/owl#Thing> .

<http://iflastandards.info/ns/fr/frbr/frbroo/R38i_is_thema_of>
        a       <http://www.w3.org/2002/07/owl#ObjectProperty> ;
        <http://www.w3.org/2000/01/rdf-schema#comment>
                "\n"@en ;
        <http://www.w3.org/2000/01/rdf-schema#domain>
                <http://www.cidoc-crm.org/cidoc-crm/E1_CRM_Entity> ;
        <http://www.w3.org/2000/01/rdf-schema#label>
                "is thema of"@en ;
        <http://www.w3.org/2000/01/rdf-schema#range>
                <http://iflastandards.info/ns/fr/frbr/frbroo/F35_Nomen_Use_Statement> ;
        <http://www.w3.org/2000/01/rdf-schema#subPropertyOf>
                <http://www.w3.org/2002/07/owl#topObjectProperty> .

<http://iflastandards.info/ns/fr/frbr/frbroo/F35_Nomen_Use_Statement>
        a       <http://www.w3.org/2002/07/owl#Class> ;
        <http://www.w3.org/2000/01/rdf-schema#comment>
                "This class comprises statements relating a Thema with a particular Nomen and its usage in the context of a common Complex Work realized by one or more KOS.\n"@en ;
        <http://www.w3.org/2000/01/rdf-schema#label>
                "Nomen Use Statement"@en ;
        <http://www.w3.org/2000/01/rdf-schema#subClassOf>
                <http://www.cidoc-crm.org/cidoc-crm/E29_Design_or_Procedure> , <http://iflastandards.info/ns/fr/frbr/frbroo/F2_Expression> .

<http://iflastandards.info/ns/fr/frbr/frbroo/R38_refers_to_thema>
        a       <http://www.w3.org/2002/07/owl#ObjectProperty> ;
        <http://www.w3.org/2000/01/rdf-schema#comment>
                "This property associates an instance of F35 Nomen Use Statement with the instance of E1 CRM Entity for which it declares the usage of a nomen.\n"@en ;
        <http://www.w3.org/2000/01/rdf-schema#domain>
                <http://iflastandards.info/ns/fr/frbr/frbroo/F35_Nomen_Use_Statement> ;
        <http://www.w3.org/2000/01/rdf-schema#label>
                "refers to thema"@en ;
        <http://www.w3.org/2000/01/rdf-schema#range>
                <http://www.cidoc-crm.org/cidoc-crm/E1_CRM_Entity> ;
        <http://www.w3.org/2000/01/rdf-schema#subPropertyOf>
                <http://www.w3.org/2002/07/owl#topObjectProperty> .

<http://iflastandards.info/ns/fr/frbr/frbroo/F52_Name_Use_Activity>
        a       <http://www.w3.org/2002/07/owl#Class> ;
        <http://www.w3.org/2000/01/rdf-schema#comment>
                "This class comprises periods of continuous use of a specific instance of E41 Appellation for a particular instance of E1 CRM Entity by an E39 Actor. It includes in particular the use of the name by its carrier. Characteristically, actors performing an activity may choose a particular appellation for themselves in the context of this activity. Such cases should be modelled by additionally classifying these activities as instances of F52 Name Use Activity.\nIt is possible to specify the type of name use, through the P2 has type property, e.g.: use of a pseudonym, use of a married name, use of a birth name, use of a blended name, use of a religious name, etc.\n"@en ;
        <http://www.w3.org/2000/01/rdf-schema#label>
                "Name Use Activity"@en ;
        <http://www.w3.org/2000/01/rdf-schema#subClassOf>
                <http://www.cidoc-crm.org/cidoc-crm/E13_Attribute_Assignment> .

<http://iflastandards.info/ns/fr/frbr/frbroo/R63_named>
        a       <http://www.w3.org/2002/07/owl#ObjectProperty> ;
        <http://www.w3.org/2000/01/rdf-schema#comment>
                "This property associates an instance of F52 Name Use Activity with the instance of E1 CRM Entity that the associated name was used for.\n"@en ;
        <http://www.w3.org/2000/01/rdf-schema#domain>
                <http://iflastandards.info/ns/fr/frbr/frbroo/F52_Name_Use_Activity> ;
        <http://www.w3.org/2000/01/rdf-schema#label>
                "named"@en ;
        <http://www.w3.org/2000/01/rdf-schema#range>
                <http://www.cidoc-crm.org/cidoc-crm/E1_CRM_Entity> ;
        <http://www.w3.org/2000/01/rdf-schema#subPropertyOf>
                <http://www.w3.org/2002/07/owl#topObjectProperty> .
