<http://www.cidoc-crm.org/cidoc-crm/P128i_is_carried_by>
        a       <http://www.w3.org/2002/07/owl#ObjectProperty> ;
        <http://www.w3.org/2000/01/rdf-schema#domain>
                <http://www.cidoc-crm.org/cidoc-crm/E90_Symbolic_Object> ;
        <http://www.w3.org/2000/01/rdf-schema#label>
                "wird getragen von"@de , "is carried by"@en , "被承载于"@zh , "a pour support"@fr , "переносится посредством"@ru , "φέρεται από"@el , "é suportado por"@pt ;
        <http://www.w3.org/2000/01/rdf-schema#range>
                <http://www.cidoc-crm.org/cidoc-crm/E18_Physical_Thing> ;
        <http://www.w3.org/2000/01/rdf-schema#subPropertyOf>
                <http://www.cidoc-crm.org/cidoc-crm/P130i_features_are_also_found_on> .

<http://www.cidoc-crm.org/cidoc-crm/E90_Symbolic_Object>
        a       <http://www.w3.org/2002/07/owl#Class> ;
        <http://www.w3.org/2000/01/rdf-schema#comment>
                "This class comprises identifiable symbols and any aggregation of symbols, such as characters, identifiers, traffic signs, emblems, texts, data sets, images, musical scores, multimedia objects, computer program code or mathematical formulae that have an objectively recognizable structure and that are documented as single units.\n\tIt includes sets of signs of any nature, which may serve to designate something, or to communicate some propositional content.\n\tAn instance of E90 Symbolic Object does not depend on a specific physical carrier, which can include human memory, and it can exist on one or more carriers simultaneously. An instance of E90 Symbolic Object may or may not have a specific meaning, for example an arbitrary character string.\n\tIn some cases, the content of an instance of E90 Symbolic Object may completely be represented by a serialized content model, such.. as the property P3 has note allows for describing this content model…P3.1 has type: E55 Type to specify the encoding..\n"@en ;
        <http://www.w3.org/2000/01/rdf-schema#label>
                "符号物件"@zh , "Symbolisches Objekt"@de , "Symbolic Object"@en ;
        <http://www.w3.org/2000/01/rdf-schema#subClassOf>
                <http://www.cidoc-crm.org/cidoc-crm/E72_Legal_Object> , <http://www.cidoc-crm.org/cidoc-crm/E28_Conceptual_Object> .

<http://www.cidoc-crm.org/cidoc-crm/P142i_was_used_in>
        a       <http://www.w3.org/2002/07/owl#ObjectProperty> ;
        <http://www.w3.org/2000/01/rdf-schema#domain>
                <http://www.cidoc-crm.org/cidoc-crm/E90_Symbolic_Object> ;
        <http://www.w3.org/2000/01/rdf-schema#label>
                "被用来构成称号於"@zh , "wurde benutzt in"@de , "was used in"@en ;
        <http://www.w3.org/2000/01/rdf-schema#range>
                <http://www.cidoc-crm.org/cidoc-crm/E15_Identifier_Assignment> ;
        <http://www.w3.org/2000/01/rdf-schema#subPropertyOf>
                <http://www.cidoc-crm.org/cidoc-crm/P16i_was_used_for> .

<http://www.cidoc-crm.org/cidoc-crm/P106_is_composed_of>
        a       <http://www.w3.org/2002/07/owl#ObjectProperty> ;
        <http://www.w3.org/2000/01/rdf-schema#comment>
                "This property associates an instance of E90 Symbolic Object with a part of it that is by itself an instance of E90 Symbolic Object, such as fragments of texts or clippings from an image.\n"@en ;
        <http://www.w3.org/2000/01/rdf-schema#domain>
                <http://www.cidoc-crm.org/cidoc-crm/E90_Symbolic_Object> ;
        <http://www.w3.org/2000/01/rdf-schema#label>
                " ist zusammengesetzt aus"@de , "αποτελείται από"@el , "est composé de"@fr , "é composto de"@pt , "составлен из"@ru , "有组成元素"@zh , "is composed of"@en ;
        <http://www.w3.org/2000/01/rdf-schema#range>
                <http://www.cidoc-crm.org/cidoc-crm/E90_Symbolic_Object> ;
        <http://www.w3.org/2000/01/rdf-schema#subPropertyOf>
                <http://www.w3.org/2002/07/owl#topObjectProperty> .

<http://www.cidoc-crm.org/cidoc-crm/P142_used_constituent>
        a       <http://www.w3.org/2002/07/owl#ObjectProperty> ;
        <http://www.w3.org/2000/01/rdf-schema#comment>
                "This property associates the event of assigning an instance of E42 Identifier to an entity, with  the instances of E41 Appellation that were used as elements of the identifier.\n"@en ;
        <http://www.w3.org/2000/01/rdf-schema#domain>
                <http://www.cidoc-crm.org/cidoc-crm/E15_Identifier_Assignment> ;
        <http://www.w3.org/2000/01/rdf-schema#label>
                "使用称号构成部分"@zh , "used constituent"@en , "benutzte Bestandteil"@de ;
        <http://www.w3.org/2000/01/rdf-schema#range>
                <http://www.cidoc-crm.org/cidoc-crm/E90_Symbolic_Object> ;
        <http://www.w3.org/2000/01/rdf-schema#subPropertyOf>
                <http://www.cidoc-crm.org/cidoc-crm/P16_used_specific_object> .

<http://www.cidoc-crm.org/cidoc-crm/P128_carries>
        a       <http://www.w3.org/2002/07/owl#ObjectProperty> ;
        <http://www.w3.org/2000/01/rdf-schema#comment>
                "This property identifies an E90 Symbolic Object carried by an instance of E18 Physical Thing.\n"@en ;
        <http://www.w3.org/2000/01/rdf-schema#domain>
                <http://www.cidoc-crm.org/cidoc-crm/E18_Physical_Thing> ;
        <http://www.w3.org/2000/01/rdf-schema#label>
                "несет"@ru , "trägt"@de , "est le support de"@fr , "φέρει"@el , "承载信息"@zh , "é o suporte de"@pt , "carries"@en ;
        <http://www.w3.org/2000/01/rdf-schema#range>
                <http://www.cidoc-crm.org/cidoc-crm/E90_Symbolic_Object> ;
        <http://www.w3.org/2000/01/rdf-schema#subPropertyOf>
                <http://www.cidoc-crm.org/cidoc-crm/P130_shows_features_of> .

<http://www.cidoc-crm.org/cidoc-crm/E18_Physical_Thing>
        a       <http://www.w3.org/2002/07/owl#Class> ;
        <http://www.w3.org/2000/01/rdf-schema#comment>
                "This class comprises all persistent physical items with a relatively stable form, man-made or natural.\n\nDepending on the existence of natural boundaries of such things, the CRM distinguishes the instances of E19 Physical Object from instances of E26 Physical Feature, such as holes, rivers, pieces of land etc. Most instances of E19 Physical Object can be moved (if not too heavy), whereas features are integral to the surrounding matter.\n\nAn instance of E18 Physical Thing occupies not only a particular geometric space, but in the course of its existence it also forms a trajectory through spacetime, which occupies a real, that is phenomenal, volume in spacetime. We include in the occupied space the space filled by the matter of the physical thing and all its inner spaces, such as the interior of a box. Physical things consisting of aggregations of physically unconnected objects, such as a set of chessmen, occupy a number of individually contiguous spacetime volumes equal to the number of unconnected objects that constitute the set.\n\nWe model E18 Physical Thing to be a subclass of E72 Legal Object and of E92 Spacetime volume. The latter is intended as a phenomenal spacetime volume as defined in CRMgeo (Doerr and Hiebel 2013). By virtue of this multiple inheritance we can discuss the physical extent of an E18 Physical Thing without representing each instance of it together with an instance of its associated spacetime volume. This model combines two quite different kinds of substance: an instance of E18 Physical Thing is matter while a spacetime volume is an aggregation of points in spacetime. However, the real spatiotemporal extent of an instance of E18 Physical Thing is regarded to be unique to it, due to all its details and fuzziness; its identity and existence depends uniquely on the identity of the instance of E18 Physical Thing. Therefore this multiple inheritance is unambiguous and effective and furthermore corresponds to the intuitions of natural language.\n\nThe CIDOC CRM is generally not concerned with amounts of matter in fluid or gaseous states. \n"@en ;
        <http://www.w3.org/2000/01/rdf-schema#label>
                "Υλικό Πράγμα"@el , "Chose matérielle"@fr , "Physical Thing"@en , "实体物"@zh , "Физическая Вещь"@ru , "Materielles"@de , "Coisa Material"@pt ;
        <http://www.w3.org/2000/01/rdf-schema#subClassOf>
                <http://www.cidoc-crm.org/cidoc-crm/E72_Legal_Object> , <http://www.cidoc-crm.org/cidoc-crm/E92_Spacetime_Volume> .

<http://www.cidoc-crm.org/cidoc-crm/P106i_forms_part_of>
        a       <http://www.w3.org/2002/07/owl#ObjectProperty> ;
        <http://www.w3.org/2000/01/rdf-schema#domain>
                <http://www.cidoc-crm.org/cidoc-crm/E90_Symbolic_Object> ;
        <http://www.w3.org/2000/01/rdf-schema#label>
                "bildet Teil von"@de , "αποτελεί μέρος του/της"@el , "组成了"@zh , "fait partie de"@fr , "forms part of"@en , "формирует часть"@ru , "faz parte de"@pt ;
        <http://www.w3.org/2000/01/rdf-schema#range>
                <http://www.cidoc-crm.org/cidoc-crm/E90_Symbolic_Object> ;
        <http://www.w3.org/2000/01/rdf-schema#subPropertyOf>
                <http://www.w3.org/2002/07/owl#topObjectProperty> .

<http://www.cidoc-crm.org/cidoc-crm/E15_Identifier_Assignment>
        a       <http://www.w3.org/2002/07/owl#Class> ;
        <http://www.w3.org/2000/01/rdf-schema#comment>
                "This class comprises activities that result in the allocation of an identifier to an instance of E1 CRM Entity. An E15 Identifier Assignment may include the creation of the identifier from multiple constituents, which themselves may be instances of E41 Appellation. The syntax and kinds of constituents to be used may be declared in a rule constituting an instance of E29 Design or Procedure.\nExamples of such identifiers include Find Numbers, Inventory Numbers, uniform titles in the sense of librarianship and Digital Object Identifiers (DOI). Documenting the act of identifier assignment and deassignment is especially useful when objects change custody or the identification system of an organization is changed. In order to keep track of the identity of things in such cases, it is important to document by whom, when and for what purpose an identifier is assigned to an item.\nThe fact that an identifier is a preferred one for an organisation can be expressed by using the property E1 CRM Entity. P48 has preferred identifier (is preferred identifier of): E42 Identifier. It can better be expressed in a context independent form by assigning a suitable E55 Type, such as “preferred identifier assignment”, to the respective instance of E15 Identifier Assignment via the P2 has type property.\n"@en ;
        <http://www.w3.org/2000/01/rdf-schema#label>
                "Identifier Assignment"@en , "Назначение Идентификатора"@ru , "Kennzeichenzuweisung"@de , "Απόδοση Αναγνωριστικού"@el , "标识符指定"@zh , "Attribution d’identificateur"@fr , "Atribuição de Identificador"@pt ;
        <http://www.w3.org/2000/01/rdf-schema#subClassOf>
                <http://www.cidoc-crm.org/cidoc-crm/E13_Attribute_Assignment> .
