<https://www.ica.org/standards/RiC/ontology#GroupSubdivisionRelation>
        a       <http://www.w3.org/2002/07/owl#Class> ;
        <http://www.w3.org/2000/01/rdf-schema#comment>
                "Connects a Group and at least another Group, when the first one\n            as the second one(s) among its subdivisions."@en ;
        <http://www.w3.org/2000/01/rdf-schema#isDefinedBy>
                <https://www.ica.org/standards/RiC/ontology> ;
        <http://www.w3.org/2000/01/rdf-schema#label>
                "Group Subdivision Relation"@en ;
        <http://www.w3.org/2000/01/rdf-schema#subClassOf>
                <https://www.ica.org/standards/RiC/ontology#WholePartRelation> , <https://www.ica.org/standards/RiC/ontology#AgentHierarchicalRelation> ;
        <https://www.ica.org/standards/RiC/ontology#RiCCMCorrespondingComponent>
                "Class implementation of RiC-R005 and RiC-R005i\n            relations"@en .

<https://www.ica.org/standards/RiC/ontology#groupIsSourceOfGroupSubdivisionRelation>
        a       <http://www.w3.org/2002/07/owl#InverseFunctionalProperty> , <http://www.w3.org/2002/07/owl#ObjectProperty> ;
        <http://www.w3.org/2000/01/rdf-schema#comment>
                "Connects the Group that has at least a subdivision, to a Group\n            Subdivision Relation"@en ;
        <http://www.w3.org/2000/01/rdf-schema#domain>
                <https://www.ica.org/standards/RiC/ontology#Group> ;
        <http://www.w3.org/2000/01/rdf-schema#isDefinedBy>
                <https://www.ica.org/standards/RiC/ontology> ;
        <http://www.w3.org/2000/01/rdf-schema#label>
                "group is source of group subdivision relation "@en ;
        <http://www.w3.org/2000/01/rdf-schema#range>
                <https://www.ica.org/standards/RiC/ontology#GroupSubdivisionRelation> ;
        <http://www.w3.org/2000/01/rdf-schema#subPropertyOf>
                <https://www.ica.org/standards/RiC/ontology#thingIsSourceOfWholePartRelation> , <https://www.ica.org/standards/RiC/ontology#agentIsSourceOfAgentHierarchicalRelation> ;
        <http://www.w3.org/2000/01/rdf-schema#subPropertyOf>
                []  ;
        <http://www.w3.org/2000/01/rdf-schema#subPropertyOf>
                []  ;
        <http://www.w3.org/2002/07/owl#equivalentProperty>
                []  ;
        <http://www.w3.org/2002/07/owl#inverseOf>
                <https://www.ica.org/standards/RiC/ontology#groupSubdivisionRelationHasSource> .

<https://www.ica.org/standards/RiC/ontology#groupSubdivisionRelationHasTarget>
        a       <http://www.w3.org/2002/07/owl#ObjectProperty> ;
        <http://www.w3.org/2000/01/rdf-schema#comment>
                "Connects a Group Subdivision Relation to one of the Groups that\n            is a subdivision"@en ;
        <http://www.w3.org/2000/01/rdf-schema#domain>
                <https://www.ica.org/standards/RiC/ontology#GroupSubdivisionRelation> ;
        <http://www.w3.org/2000/01/rdf-schema#isDefinedBy>
                <https://www.ica.org/standards/RiC/ontology> ;
        <http://www.w3.org/2000/01/rdf-schema#label>
                "group subdivision relation has target "@en ;
        <http://www.w3.org/2000/01/rdf-schema#range>
                <https://www.ica.org/standards/RiC/ontology#Group> ;
        <http://www.w3.org/2000/01/rdf-schema#subPropertyOf>
                <https://www.ica.org/standards/RiC/ontology#wholePartRelationHasTarget> , <https://www.ica.org/standards/RiC/ontology#agentHierarchicalRelationHasTarget> ;
        <http://www.w3.org/2000/01/rdf-schema#subPropertyOf>
                []  ;
        <http://www.w3.org/2000/01/rdf-schema#subPropertyOf>
                []  ;
        <http://www.w3.org/2002/07/owl#inverseOf>
                <https://www.ica.org/standards/RiC/ontology#groupIsTargetOfGroupSubdivisionRelation> .

<https://www.ica.org/standards/RiC/ontology#groupSubdivisionRelationHasSource>
        a       <http://www.w3.org/2002/07/owl#FunctionalProperty> , <http://www.w3.org/2002/07/owl#ObjectProperty> ;
        <http://www.w3.org/2000/01/rdf-schema#comment>
                "Connects a Group Subdivision Relation to the Group that has\n            subdivisions"@en ;
        <http://www.w3.org/2000/01/rdf-schema#domain>
                <https://www.ica.org/standards/RiC/ontology#GroupSubdivisionRelation> ;
        <http://www.w3.org/2000/01/rdf-schema#isDefinedBy>
                <https://www.ica.org/standards/RiC/ontology> ;
        <http://www.w3.org/2000/01/rdf-schema#label>
                "group subdivision relation has source "@en ;
        <http://www.w3.org/2000/01/rdf-schema#range>
                <https://www.ica.org/standards/RiC/ontology#Group> ;
        <http://www.w3.org/2000/01/rdf-schema#subPropertyOf>
                <https://www.ica.org/standards/RiC/ontology#wholePartRelationHasSource> , <https://www.ica.org/standards/RiC/ontology#agentHierarchicalRelationHasSource> ;
        <http://www.w3.org/2000/01/rdf-schema#subPropertyOf>
                []  ;
        <http://www.w3.org/2000/01/rdf-schema#subPropertyOf>
                []  .

<https://www.ica.org/standards/RiC/ontology#Group>
        a       <http://www.w3.org/2002/07/owl#Class> ;
        <http://www.w3.org/2000/01/rdf-schema#comment>
                "Two or more Agents that act together as an Agent."@en ;
        <http://www.w3.org/2000/01/rdf-schema#isDefinedBy>
                <https://www.ica.org/standards/RiC/ontology> ;
        <http://www.w3.org/2000/01/rdf-schema#label>
                "Group"@en ;
        <http://www.w3.org/2000/01/rdf-schema#subClassOf>
                <https://www.ica.org/standards/RiC/ontology#Agent> ;
        <http://www.w3.org/2002/07/owl#disjointWith>
                <https://www.ica.org/standards/RiC/ontology#Position> , <https://www.ica.org/standards/RiC/ontology#Person> , <https://www.ica.org/standards/RiC/ontology#Mechanism> ;
        <http://www.w3.org/2004/02/skos/core#scopeNote>
                "Group is a kind of Agent. A Group has a socially recognized\n            identity. Each member of the Group plays a particular role or roles (that is has a\n            particular Position) in the coordinated activity of the Group. Corporate bodies and\n            families are kinds of groups, though other kinds of groups are possible. For example,\n            the “electorate” -- all of the voters in a given election. Complex, large groups may be\n            subdivided into other groups."@en ;
        <https://www.ica.org/standards/RiC/ontology#RiCCMCorrespondingComponent>
                "Corresponds to RiC-E09 (Group\n            Entity)"@en .

<https://www.ica.org/standards/RiC/ontology#groupIsTargetOfGroupSubdivisionRelation>
        a       <http://www.w3.org/2002/07/owl#ObjectProperty> ;
        <http://www.w3.org/2000/01/rdf-schema#comment>
                "Connects a Group that is a subdivision, to a Group Subdivision\n            Relation"@en ;
        <http://www.w3.org/2000/01/rdf-schema#domain>
                <https://www.ica.org/standards/RiC/ontology#Group> ;
        <http://www.w3.org/2000/01/rdf-schema#isDefinedBy>
                <https://www.ica.org/standards/RiC/ontology> ;
        <http://www.w3.org/2000/01/rdf-schema#label>
                "group is target of group subdivision relation "@en ;
        <http://www.w3.org/2000/01/rdf-schema#range>
                <https://www.ica.org/standards/RiC/ontology#GroupSubdivisionRelation> ;
        <http://www.w3.org/2000/01/rdf-schema#subPropertyOf>
                <https://www.ica.org/standards/RiC/ontology#agentIsTargetOfAgentHierarchicalRelation> , <https://www.ica.org/standards/RiC/ontology#thingIsTargetOfWholePartRelation> ;
        <http://www.w3.org/2000/01/rdf-schema#subPropertyOf>
                []  ;
        <http://www.w3.org/2000/01/rdf-schema#subPropertyOf>
                []  ;
        <http://www.w3.org/2002/07/owl#equivalentProperty>
                []  .
