<http://iflastandards.info/ns/fr/frbr/pressoo/Y45i_was_created_by>
        a       <http://www.w3.org/2002/07/owl#ObjectProperty> , <http://www.w3.org/2002/07/owl#AnnotationProperty> ;
        <http://www.w3.org/2000/01/rdf-schema#domain>
                <http://iflastandards.info/ns/fr/frbr/pressoo/Z9_Storage_Unit> ;
        <http://www.w3.org/2000/01/rdf-schema#label>
                "was created by"@en ;
        <http://www.w3.org/2000/01/rdf-schema#range>
                <http://iflastandards.info/ns/fr/frbr/pressoo/Z14_Storage_Unit_Creation> ;
        <http://www.w3.org/2000/01/rdf-schema#subPropertyOf>
                <http://www.w3.org/2002/07/owl#topObjectProperty> , <http://iflastandards.info/ns/fr/frbr/frbroo/R18i_was_created_by> .

<http://iflastandards.info/ns/fr/frbr/pressoo/Z14_Storage_Unit_Creation>
        a       <http://www.w3.org/2002/07/owl#Class> ;
        <http://www.w3.org/2000/01/rdf-schema#comment>
                "This class comprises activities through which instances of Z9 Storage Unit are produced.\nAlthough the activity of producing a storage unit can be motivated by preservation only, it inevitably results in the creation of an expression that consists of the sum of all expressions conveyed by the individual items and/or manifestation singletons that make up the resulting storage unit. Z14 Storage Unit Creation is therefore declared as a subclass of F28 Expression Creation.\nA given instance of Z14 Storage Unit Creation can involve truly artistic endeavours, such as the conception and realisation of a binding which can be regarded as a piece of cultural heritage in its own right."@en ;
        <http://www.w3.org/2000/01/rdf-schema#label>
                "Storage Unit Creation"@en ;
        <http://www.w3.org/2000/01/rdf-schema#subClassOf>
                <http://iflastandards.info/ns/fr/frbr/frbroo/F28_Expression_Creation> .

<http://iflastandards.info/ns/fr/frbr/pressoo/Y45_created>
        a       <http://www.w3.org/2002/07/owl#ObjectProperty> , <http://www.w3.org/2002/07/owl#AnnotationProperty> ;
        <http://www.w3.org/2000/01/rdf-schema#comment>
                "This property associates an instance of Z14 Storage Unit Creation with the instances of Z9 Storage Unit in which it resulted."@en ;
        <http://www.w3.org/2000/01/rdf-schema#domain>
                <http://iflastandards.info/ns/fr/frbr/pressoo/Z14_Storage_Unit_Creation> ;
        <http://www.w3.org/2000/01/rdf-schema#label>
                "created"@en ;
        <http://www.w3.org/2000/01/rdf-schema#range>
                <http://iflastandards.info/ns/fr/frbr/pressoo/Z9_Storage_Unit> ;
        <http://www.w3.org/2000/01/rdf-schema#subPropertyOf>
                <http://www.w3.org/2002/07/owl#topObjectProperty> , <http://iflastandards.info/ns/fr/frbr/frbroo/R18_created> .

<http://iflastandards.info/ns/fr/frbr/pressoo/Z9_Storage_Unit>
        a       <http://www.w3.org/2002/07/owl#Class> ;
        <http://www.w3.org/2000/01/rdf-schema#comment>
                "This class comprises unique combinations of instances of E24 Physical Man-Made Thing that are bound together, or otherwise physically united, for the sake of preservation, and are communicated to library users as single, indivisible units. The individual components of a given instance of Z9 Storage Unit are generally instances of F4 Manifestation Singleton and/or F5 Item, but the binding itself that holds them together can be a valuable piece of cultural heritage that is worth describing for its own sake. Z9 Storage Unit makes it possible to account indifferently for the description of the various materials (printed or manuscript or of any other type) that make up a holding, and of the binding (or any other type of device, e.g. a box, a casket, etc.) that was produced for that holding, if needed."@en ;
        <http://www.w3.org/2000/01/rdf-schema#label>
                "Storage Unit"@en ;
        <http://www.w3.org/2000/01/rdf-schema#subClassOf>
                <http://iflastandards.info/ns/fr/frbr/frbroo/F4_Manifestation_Singleton> .
