<http://iflastandards.info/ns/fr/frbr/pressoo/Y27i_foresees_translation_of>
        a       <http://www.w3.org/2002/07/owl#ObjectProperty> ;
        <http://www.w3.org/2000/01/rdf-schema#domain>
                <http://iflastandards.info/ns/fr/frbr/pressoo/Z12_Issuing_Rule> ;
        <http://www.w3.org/2000/01/rdf-schema#label>
                "foresees translation of"@en ;
        <http://www.w3.org/2000/01/rdf-schema#range>
                <http://iflastandards.info/ns/fr/frbr/pressoo/Z12_Issuing_Rule> ;
        <http://www.w3.org/2000/01/rdf-schema#subPropertyOf>
                <http://iflastandards.info/ns/fr/frbr/pressoo/Y26i_foresees_to_be_another_edition_of> .

<http://iflastandards.info/ns/fr/frbr/frbroo/F18_Serial_Work>
        a       <http://www.w3.org/2002/07/owl#Class> ;
        <http://www.w3.org/2000/01/rdf-schema#subClassOf>
                <http://www.w3.org/2002/07/owl#Thing> .

<http://iflastandards.info/ns/fr/frbr/pressoo/Y37i_is_former_or_current_issuing_rule_of>
        a       <http://www.w3.org/2002/07/owl#ObjectProperty> , <http://www.w3.org/2002/07/owl#AnnotationProperty> ;
        <http://www.w3.org/2000/01/rdf-schema#domain>
                <http://iflastandards.info/ns/fr/frbr/pressoo/Z12_Issuing_Rule> ;
        <http://www.w3.org/2000/01/rdf-schema#label>
                "is former or current issuing rule of"@en ;
        <http://www.w3.org/2000/01/rdf-schema#range>
                <http://iflastandards.info/ns/fr/frbr/frbroo/F18_Serial_Work> ;
        <http://www.w3.org/2000/01/rdf-schema#subPropertyOf>
                <http://www.w3.org/2002/07/owl#topObjectProperty> , <http://iflastandards.info/ns/fr/frbr/frbroo/R11i_is_issuing_rule_of> .

<http://iflastandards.info/ns/fr/frbr/pressoo/Y37_has_former_or_current_issuing_rule>
        a       <http://www.w3.org/2002/07/owl#ObjectProperty> , <http://www.w3.org/2002/07/owl#AnnotationProperty> ;
        <http://www.w3.org/2000/01/rdf-schema#comment>
                "This property associates an instance of F18 Serial Work with instances of Z12 Issuing Rule that specify aspects of the issuing policy planned at some time by this Work, such as sequencing pattern, expected frequency or expected regularity. This property does not specify whether these instances of Z12 Issuing Rule are still in force at the time of validity of the record or database containing the statement that uses this property, and it can point to obsolete instances of Z12 Issuing Rule."@en ;
        <http://www.w3.org/2000/01/rdf-schema#domain>
                <http://iflastandards.info/ns/fr/frbr/frbroo/F18_Serial_Work> ;
        <http://www.w3.org/2000/01/rdf-schema#label>
                "has former or current issuing rule"@en ;
        <http://www.w3.org/2000/01/rdf-schema#range>
                <http://iflastandards.info/ns/fr/frbr/pressoo/Z12_Issuing_Rule> ;
        <http://www.w3.org/2000/01/rdf-schema#subPropertyOf>
                <http://www.w3.org/2002/07/owl#topObjectProperty> , <http://iflastandards.info/ns/fr/frbr/frbroo/R11_has_issuing_rule> .

<http://iflastandards.info/ns/fr/frbr/pressoo/Y26_foresees_other_edition>
        a       <http://www.w3.org/2002/07/owl#ObjectProperty> ;
        <http://www.w3.org/2000/01/rdf-schema#comment>
                "This property associates an instance of Z12 Issuing Rule with an instance of Z12 Issuing Rule associated with a continuing resource that the first instance of Z12 Issuing Rule regards as another edition of the continuing resource of which it is an issuing rule.\nIt can denote a dynamic, asymmetric relationship where the range expresses the dependant publication, if such a direction can be established. Otherwise, it denotes a symmetric relationship, where none of the two continuing resources is regarded as dependant on the other.\nIn addition to being a subproperty of Y25 foresees association with (has association foreseen in), it can also be analysed as a shortcut of the more developed path: Z12 Issuing Rule Y37i is former or current issuing rule of F18 Serial Work R10i is member of F15 Complex Work R10 has member F18 Serial Work Y37 has former or current issuing rule Z12 Issuing Rule.\nThe Y26.1 has type property of the property allows the nature of the association to be specified; examples of types of association between instances of Z12 Issuing Rule include: other edition, other format, local edition, other edition on a different type of carrier, abridged edition, edition in a different language, etc."@en ;
        <http://www.w3.org/2000/01/rdf-schema#domain>
                <http://iflastandards.info/ns/fr/frbr/pressoo/Z12_Issuing_Rule> ;
        <http://www.w3.org/2000/01/rdf-schema#label>
                "foresees other edition"@en ;
        <http://www.w3.org/2000/01/rdf-schema#range>
                <http://iflastandards.info/ns/fr/frbr/pressoo/Z12_Issuing_Rule> ;
        <http://www.w3.org/2000/01/rdf-schema#subPropertyOf>
                <http://iflastandards.info/ns/fr/frbr/pressoo/Y25_foresees_association_with> .

<http://iflastandards.info/ns/fr/frbr/pressoo/Y38i_is_current_issuing_rule_of>
        a       <http://www.w3.org/2002/07/owl#ObjectProperty> ;
        <http://www.w3.org/2000/01/rdf-schema#domain>
                <http://iflastandards.info/ns/fr/frbr/pressoo/Z12_Issuing_Rule> ;
        <http://www.w3.org/2000/01/rdf-schema#label>
                "is current issuing rule of"@en ;
        <http://www.w3.org/2000/01/rdf-schema#range>
                <http://iflastandards.info/ns/fr/frbr/frbroo/F18_Serial_Work> ;
        <http://www.w3.org/2000/01/rdf-schema#subPropertyOf>
                <http://iflastandards.info/ns/fr/frbr/pressoo/Y37i_is_former_or_current_issuing_rule_of> .

<http://iflastandards.info/ns/fr/frbr/pressoo/Y25_foresees_association_with>
        a       <http://www.w3.org/2002/07/owl#ObjectProperty> , <http://www.w3.org/2002/07/owl#AnnotationProperty> ;
        <http://www.w3.org/2000/01/rdf-schema#comment>
                "This property associates an instance of Z12 Issuing Rule with an instance of Z12 Issuing Rule associated with a continuing resource that the first instance of Z12 Issuing Rule regards as related in some way with the continuing resource of which it is an issuing rule.\nIt can denote a dynamic, asymmetric relationship where the range expresses the dependant publication, if such a direction can be established. Otherwise, it denotes a symmetric relationship, where none of the two continuing resources is regarded as dependant on the other.\nThe Y25.1 has type property of the property allows the nature of the association to be specified; examples of types of association between instances of Z12 Issuing Rule include: supplement, issued with, insert, etc."@en ;
        <http://www.w3.org/2000/01/rdf-schema#domain>
                <http://iflastandards.info/ns/fr/frbr/pressoo/Z12_Issuing_Rule> ;
        <http://www.w3.org/2000/01/rdf-schema#label>
                "foresees association with"@en ;
        <http://www.w3.org/2000/01/rdf-schema#range>
                <http://iflastandards.info/ns/fr/frbr/pressoo/Z12_Issuing_Rule> ;
        <http://www.w3.org/2000/01/rdf-schema#subPropertyOf>
                <http://www.w3.org/2002/07/owl#topObjectProperty> , <http://www.cidoc-crm.org/cidoc-crm/P69_has_association_with> .

<http://iflastandards.info/ns/fr/frbr/pressoo/Y25i_has_association_foreseen_in>
        a       <http://www.w3.org/2002/07/owl#ObjectProperty> , <http://www.w3.org/2002/07/owl#AnnotationProperty> ;
        <http://www.w3.org/2000/01/rdf-schema#domain>
                <http://iflastandards.info/ns/fr/frbr/pressoo/Z12_Issuing_Rule> ;
        <http://www.w3.org/2000/01/rdf-schema#label>
                "has association foreseen in"@en ;
        <http://www.w3.org/2000/01/rdf-schema#range>
                <http://iflastandards.info/ns/fr/frbr/pressoo/Z12_Issuing_Rule> ;
        <http://www.w3.org/2000/01/rdf-schema#subPropertyOf>
                <http://www.w3.org/2002/07/owl#topObjectProperty> , <http://www.cidoc-crm.org/cidoc-crm/P69i_is_associated_with> .

<http://iflastandards.info/ns/fr/frbr/pressoo/Y26i_foresees_to_be_another_edition_of>
        a       <http://www.w3.org/2002/07/owl#ObjectProperty> ;
        <http://www.w3.org/2000/01/rdf-schema#domain>
                <http://iflastandards.info/ns/fr/frbr/pressoo/Z12_Issuing_Rule> ;
        <http://www.w3.org/2000/01/rdf-schema#label>
                "foresees to be another edition of"@en ;
        <http://www.w3.org/2000/01/rdf-schema#range>
                <http://iflastandards.info/ns/fr/frbr/pressoo/Z12_Issuing_Rule> ;
        <http://www.w3.org/2000/01/rdf-schema#subPropertyOf>
                <http://iflastandards.info/ns/fr/frbr/pressoo/Y25i_has_association_foreseen_in> .

<http://iflastandards.info/ns/fr/frbr/pressoo/Y38_has_current_issuing_rule>
        a       <http://www.w3.org/2002/07/owl#ObjectProperty> ;
        <http://www.w3.org/2000/01/rdf-schema#comment>
                "This property associates an instance of F18 Serial Work with instances of Z12 Issuing Rule that specify aspects of the issuing policy planned by this Work, such as sequencing pattern, expected frequency or expected regularity, at the time of validity of the record or database containing the statement that uses this property.\nIf the publication has ceased, this property reflects the latest known issuing rules followed by the continuing resource when its last known issue was released (i.e., the issuing rules followed in the instance of Z7 Ending of Publication associated with the continuing resource), rather than the ‘current’ issuing rules (since in that case, strictly speaking, there are no ‘current’ issuing rules)."@en ;
        <http://www.w3.org/2000/01/rdf-schema#domain>
                <http://iflastandards.info/ns/fr/frbr/frbroo/F18_Serial_Work> ;
        <http://www.w3.org/2000/01/rdf-schema#label>
                "has current issuing rule"@en ;
        <http://www.w3.org/2000/01/rdf-schema#range>
                <http://iflastandards.info/ns/fr/frbr/pressoo/Z12_Issuing_Rule> ;
        <http://www.w3.org/2000/01/rdf-schema#subPropertyOf>
                <http://iflastandards.info/ns/fr/frbr/pressoo/Y37_has_former_or_current_issuing_rule> .

<http://iflastandards.info/ns/fr/frbr/pressoo/Z12_Issuing_Rule>
        a       <http://www.w3.org/2002/07/owl#Class> ;
        <http://www.w3.org/2000/01/rdf-schema#comment>
                "This class comprises plans that specify bits of the issuing policy followed at some point in time for instances of F18 Serial Work.\nThe notion of issuing policy may include: regularity, frequency, sequencing pattern, the language of the linguistic objects contained in each issue, dimension of each issue, the font used to print each issue, the layout and editorial rules adhered to in each issue, etc.\n[Note: The notion of issuing rule is to be understood differently in PRESSOO than in FRBROO. In FRBROO, property R11 has issuing rule (is issuing rule) points to a complete issuing policy that comprises a variety of parameters (regularity, frequency, dimension, language, etc.), while in PRESSOO an instance of Z12 Issuing Rule focuses on only one of those parameters and consists of a plan for just the expected regularity, just the expected frequency, just the expected dimension, etc. This perspective shift was made necessary when it was realized that any change (i.e., any instance of Z5 Issuing Rule Change) in just one of those parameters led to a new instantiation of Z12 Issuing Rule and new instantiations of all the ranges of the associated properties, with exactly the same value for each of them except for the one parameter that changes. It was deemed preferable to associate an instance of Z12 Issuing Rule with just one parameter of the issuing policy, which makes it possible that, e.g., a monthly was transformed into a quarterly without having to repeat that the expected language of its issues remains English.]"@en ;
        <http://www.w3.org/2000/01/rdf-schema#label>
                "Issuing Rule"@en ;
        <http://www.w3.org/2000/01/rdf-schema#subClassOf>
                <http://www.cidoc-crm.org/cidoc-crm/E29_Design_or_Procedure> .

<http://iflastandards.info/ns/fr/frbr/pressoo/Y27_foresees_translation_in>
        a       <http://www.w3.org/2002/07/owl#ObjectProperty> ;
        <http://www.w3.org/2000/01/rdf-schema#comment>
                "This property associates an instance of Z12 Issuing Rule with an instance of Z12 Issuing Rule associated with a continuing resource that, according to the respective issuing policies of the\n39/105\ntwo continuing resources, should contain a translation of the content of the first continuing resource.\nThis is not the same notion as the association of a continuing resource with one or more than one ‘edition in a different language’, which is expressed through property Y26 foresees other edition (foresees to be another edition of)."@en ;
        <http://www.w3.org/2000/01/rdf-schema#domain>
                <http://iflastandards.info/ns/fr/frbr/pressoo/Z12_Issuing_Rule> ;
        <http://www.w3.org/2000/01/rdf-schema#label>
                "foresees translation in"@en ;
        <http://www.w3.org/2000/01/rdf-schema#range>
                <http://iflastandards.info/ns/fr/frbr/pressoo/Z12_Issuing_Rule> ;
        <http://www.w3.org/2000/01/rdf-schema#subPropertyOf>
                <http://iflastandards.info/ns/fr/frbr/pressoo/Y26_foresees_other_edition> .
