<https://www.ica.org/standards/RiC/ontology#Thing>
        a       <http://www.w3.org/2002/07/owl#Class> ;
        <http://www.w3.org/2000/01/rdf-schema#comment>
                "Any idea, material thing, or event within the realm of human\n            experience."@en ;
        <http://www.w3.org/2000/01/rdf-schema#isDefinedBy>
                <https://www.ica.org/standards/RiC/ontology> ;
        <http://www.w3.org/2000/01/rdf-schema#label>
                "Thing"@en ;
        <http://www.w3.org/2000/01/rdf-schema#subClassOf>
                <http://www.w3.org/2002/07/owl#Thing> ;
        <http://www.w3.org/2004/02/skos/core#scopeNote>
                "Includes all RiC entities as well as any concept, material\n            thing, or event that may be the subject of a Record Resource or associated with an\n            Activity. Examples of entities not explicitly addressed in RiC includes but is not\n            limited to the following: abstract concepts; cultural movements, named periods and\n            events; named things, objects and works; legendary, mythical or fictitious figures,\n            characters or beings."@en ;
        <https://www.ica.org/standards/RiC/ontology#RiCCMCorrespondingComponent>
                "Corresponds to RiC-E01 (Thing\n            entity)"@en .

<https://www.ica.org/standards/RiC/ontology#Name>
        a       <http://www.w3.org/2002/07/owl#Class> ;
        <http://www.w3.org/2000/01/rdf-schema#comment>
                "A label, title or term designating the entity in order to make\n            it distinguishable from other similar entities."@en ;
        <http://www.w3.org/2000/01/rdf-schema#isDefinedBy>
                <https://www.ica.org/standards/RiC/ontology> ;
        <http://www.w3.org/2000/01/rdf-schema#label>
                "Name"@en ;
        <http://www.w3.org/2000/01/rdf-schema#subClassOf>
                <https://www.ica.org/standards/RiC/ontology#Appellation> ;
        <https://www.ica.org/standards/RiC/ontology#RiCCMCorrespondingComponent>
                "Class implementation of RiC-A28 (Name attribute)\n            (see also the name data property)"@en .

<https://www.ica.org/standards/RiC/ontology#isOrWasNameOf>
        a       <http://www.w3.org/2002/07/owl#ObjectProperty> ;
        <http://www.w3.org/2000/01/rdf-schema#comment>
                "Connects a Name to a Thing that it designated or\n            designates."@en ;
        <http://www.w3.org/2000/01/rdf-schema#domain>
                <https://www.ica.org/standards/RiC/ontology#Name> ;
        <http://www.w3.org/2000/01/rdf-schema#isDefinedBy>
                <https://www.ica.org/standards/RiC/ontology> ;
        <http://www.w3.org/2000/01/rdf-schema#label>
                "is or was name of"@en ;
        <http://www.w3.org/2000/01/rdf-schema#range>
                <https://www.ica.org/standards/RiC/ontology#Thing> ;
        <http://www.w3.org/2000/01/rdf-schema#subPropertyOf>
                <https://www.ica.org/standards/RiC/ontology#isOrWasAppellationOf> ;
        <http://www.w3.org/2000/01/rdf-schema#subPropertyOf>
                []  ;
        <http://www.w3.org/2004/02/skos/core#changeNote>
                []  .

<https://www.ica.org/standards/RiC/ontology#hasOrHadName>
        a       <http://www.w3.org/2002/07/owl#ObjectProperty> ;
        <http://www.w3.org/2000/01/rdf-schema#comment>
                "Connects a Thing to one of its past or present\n            Names."@en ;
        <http://www.w3.org/2000/01/rdf-schema#domain>
                <https://www.ica.org/standards/RiC/ontology#Thing> ;
        <http://www.w3.org/2000/01/rdf-schema#isDefinedBy>
                <https://www.ica.org/standards/RiC/ontology> ;
        <http://www.w3.org/2000/01/rdf-schema#label>
                "has or had name"@en ;
        <http://www.w3.org/2000/01/rdf-schema#range>
                <https://www.ica.org/standards/RiC/ontology#Name> ;
        <http://www.w3.org/2000/01/rdf-schema#subPropertyOf>
                <https://www.ica.org/standards/RiC/ontology#hasOrHadAppellation> ;
        <http://www.w3.org/2000/01/rdf-schema#subPropertyOf>
                []  ;
        <http://www.w3.org/2002/07/owl#equivalentProperty>
                []  ;
        <http://www.w3.org/2002/07/owl#inverseOf>
                <https://www.ica.org/standards/RiC/ontology#isOrWasNameOf> ;
        <http://www.w3.org/2004/02/skos/core#changeNote>
                []  .
