<http://iflastandards.info/ns/fr/frbr/frbroo/R31_is_reproduction_of>
        a       <http://www.w3.org/2002/07/owl#ObjectProperty> ;
        <http://www.w3.org/2000/01/rdf-schema#comment>
                "This property associates an instance of E84 Information Carrier which is a reproduction of another instance of E84 Information Carrier with the latter. It is considered that a reproduction of multiple originals resulting in a single product requires a merging of those objects prior to the reproduction. Therefore an Information Carrier is regarded to be a reproduction of one and only one original. This property is a shortcut of the more fully developed path from E84 Information Carrier through R30 produced (was produced by), F33 Reproduction Event R29 reproduced (was reproduced by) to E84 Information Carrier.\n"@en ;
        <http://www.w3.org/2000/01/rdf-schema#domain>
                <http://www.cidoc-crm.org/cidoc-crm/E84_Information_Carrier> ;
        <http://www.w3.org/2000/01/rdf-schema#label>
                "is reproduction of"@en ;
        <http://www.w3.org/2000/01/rdf-schema#range>
                <http://www.cidoc-crm.org/cidoc-crm/E84_Information_Carrier> ;
        <http://www.w3.org/2000/01/rdf-schema#subPropertyOf>
                <http://www.w3.org/2002/07/owl#topObjectProperty> .

<http://iflastandards.info/ns/fr/frbr/frbroo/R30_produced>
        a       <http://www.w3.org/2002/07/owl#ObjectProperty> ;
        <http://www.w3.org/2000/01/rdf-schema#comment>
                "This property associates an instance of F33 Reproduction Event with an instance of E84 Information Carrier it produces.\n"@en ;
        <http://www.w3.org/2000/01/rdf-schema#domain>
                <http://iflastandards.info/ns/fr/frbr/frbroo/F33_Reproduction_Event> ;
        <http://www.w3.org/2000/01/rdf-schema#label>
                "produced"@en ;
        <http://www.w3.org/2000/01/rdf-schema#range>
                <http://www.cidoc-crm.org/cidoc-crm/E84_Information_Carrier> ;
        <http://www.w3.org/2000/01/rdf-schema#subPropertyOf>
                <http://www.w3.org/2002/07/owl#topObjectProperty> .

<http://www.cidoc-crm.org/cidoc-crm/E84_Information_Carrier>
        a       <http://www.w3.org/2002/07/owl#Class> ;
        <http://www.w3.org/2000/01/rdf-schema#subClassOf>
                <http://www.w3.org/2002/07/owl#Thing> .

<http://iflastandards.info/ns/fr/frbr/frbroo/R31i_has_reproduction>
        a       <http://www.w3.org/2002/07/owl#ObjectProperty> ;
        <http://www.w3.org/2000/01/rdf-schema#comment>
                "\n"@en ;
        <http://www.w3.org/2000/01/rdf-schema#domain>
                <http://www.cidoc-crm.org/cidoc-crm/E84_Information_Carrier> ;
        <http://www.w3.org/2000/01/rdf-schema#label>
                "has reproduction"@en ;
        <http://www.w3.org/2000/01/rdf-schema#range>
                <http://www.cidoc-crm.org/cidoc-crm/E84_Information_Carrier> ;
        <http://www.w3.org/2000/01/rdf-schema#subPropertyOf>
                <http://www.w3.org/2002/07/owl#topObjectProperty> .

<http://iflastandards.info/ns/fr/frbr/frbroo/F33_Reproduction_Event>
        a       <http://www.w3.org/2002/07/owl#Class> ;
        <http://www.w3.org/2000/01/rdf-schema#comment>
                "This class comprises activities that consist in making copies, more or less mechanically, of an instance of E84 Information Carrier (such as an F5 Item or an F4 Manifestation Singleton which is also instance of E84 Information Carrier), preserving the expression carried by it. A Reproduction Event results in new instances of E84 Information Carrier coming into existence. In general, the copy will have different attributes from the original and they are therefore not regarded as siblings.\nThis class makes it possible to account for the legal distinction between private copying for the purpose of “fair use,” and mass production for the purpose of dissemination.\nIt can prove difficult to determine where to draw the line between F33 Reproduction Event and F32 Carrier Production Event in cases where multiple copies are produced. In this case, the copies, but not the original, may be regarded as instances of F5 Item. It is the existence of an explicit production plan that makes the difference. As a consequence, F33 Reproduction Event and F32 Carrier Production Event are not declared as disjoint, which makes it possible to account for such situations that could be regarded as instances of both Production Event and Reproduction Event.\n"@en ;
        <http://www.w3.org/2000/01/rdf-schema#label>
                "Reproduction Event"@en ;
        <http://www.w3.org/2000/01/rdf-schema#subClassOf>
                <http://www.cidoc-crm.org/cidoc-crm/E12_Production> .

<http://iflastandards.info/ns/fr/frbr/frbroo/R29_reproduced>
        a       <http://www.w3.org/2002/07/owl#ObjectProperty> ;
        <http://www.w3.org/2000/01/rdf-schema#comment>
                "This property associates an instance of F33 Reproduction Event with an instance of E84 Information Carrier it reproduces.\n"@en ;
        <http://www.w3.org/2000/01/rdf-schema#domain>
                <http://iflastandards.info/ns/fr/frbr/frbroo/F33_Reproduction_Event> ;
        <http://www.w3.org/2000/01/rdf-schema#label>
                "reproduced"@en ;
        <http://www.w3.org/2000/01/rdf-schema#range>
                <http://www.cidoc-crm.org/cidoc-crm/E84_Information_Carrier> ;
        <http://www.w3.org/2000/01/rdf-schema#subPropertyOf>
                <http://www.w3.org/2002/07/owl#topObjectProperty> .

<http://iflastandards.info/ns/fr/frbr/frbroo/R30i_was_produced_by>
        a       <http://www.w3.org/2002/07/owl#ObjectProperty> ;
        <http://www.w3.org/2000/01/rdf-schema#comment>
                "\n"@en ;
        <http://www.w3.org/2000/01/rdf-schema#domain>
                <http://www.cidoc-crm.org/cidoc-crm/E84_Information_Carrier> ;
        <http://www.w3.org/2000/01/rdf-schema#label>
                "was produced by"@en ;
        <http://www.w3.org/2000/01/rdf-schema#range>
                <http://iflastandards.info/ns/fr/frbr/frbroo/F33_Reproduction_Event> ;
        <http://www.w3.org/2000/01/rdf-schema#subPropertyOf>
                <http://www.w3.org/2002/07/owl#topObjectProperty> .

<http://iflastandards.info/ns/fr/frbr/frbroo/R29i_was_reproduced_by>
        a       <http://www.w3.org/2002/07/owl#ObjectProperty> ;
        <http://www.w3.org/2000/01/rdf-schema#comment>
                "\n"@en ;
        <http://www.w3.org/2000/01/rdf-schema#domain>
                <http://www.cidoc-crm.org/cidoc-crm/E84_Information_Carrier> ;
        <http://www.w3.org/2000/01/rdf-schema#label>
                "was reproduced by"@en ;
        <http://www.w3.org/2000/01/rdf-schema#range>
                <http://iflastandards.info/ns/fr/frbr/frbroo/F33_Reproduction_Event> ;
        <http://www.w3.org/2000/01/rdf-schema#subPropertyOf>
                <http://www.w3.org/2002/07/owl#topObjectProperty> .
