<https://w3id.org/roar#Document>
        a       <http://www.w3.org/2002/07/owl#Class> ;
        <http://www.w3.org/2000/01/rdf-schema#comment>
                "The source (e.g. document, act, legislation, text, picture, painting, recording, obelisk) in which some entity (e.g. Person or Location) can be observed.\nIf the source that you are describing is not digitised or is not available as URI, you can define your own resource of class `roar:Document` and use for instance the properties defined by `schema:CreativeWork` to describe it. The `roar:onScan` property can then be used on an Observation to specify the location of the Entity in the source."@en ;
        <http://www.w3.org/2000/01/rdf-schema#label>
                "Document"@en ;
        <http://www.w3.org/2000/01/rdf-schema#subClassOf>
                <http://www.w3.org/2002/07/owl#Thing> .

<http://www.w3.org/ns/prov#Entity>
        a       <http://www.w3.org/2002/07/owl#Class> ;
        <http://www.w3.org/2000/01/rdf-schema#label>
                "prov:Entity"@en ;
        <http://www.w3.org/2000/01/rdf-schema#subClassOf>
                <http://www.w3.org/2002/07/owl#Thing> .

<https://w3id.org/roar#Observation>
        a       <http://www.w3.org/2002/07/owl#Class> ;
        <http://www.w3.org/2000/01/rdf-schema#comment>
                "Something of a type 'Observation' is something that is mentioned or described in a 'Document' (described by roar:inDocument). Two common subclasses are PersonObservation and LocationObservation, but one can also think about EventObservation and other entities."@en ;
        <http://www.w3.org/2000/01/rdf-schema#label>
                "Observation"@en ;
        <http://www.w3.org/2000/01/rdf-schema#subClassOf>
                <http://www.w3.org/ns/prov#Entity> ;
        <http://www.w3.org/2002/07/owl#disjointWith>
                <https://w3id.org/roar#Reconstruction> .

<https://w3id.org/roar#documentedIn>
        a       <http://www.w3.org/2002/07/owl#ObjectProperty> ;
        <http://www.w3.org/2000/01/rdf-schema#comment>
                "Refers to the Document (source, act, legislation etc.) in which the Observation is made. It is recommended to point to a resource (URI) provided by some institute/archive that hold key information on this source. You are, however, free to fill `roar:Document` with additional information."@en ;
        <http://www.w3.org/2000/01/rdf-schema#domain>
                <http://www.w3.org/ns/prov#Entity> ;
        <http://www.w3.org/2000/01/rdf-schema#label>
                "documentedIn"@en ;
        <http://www.w3.org/2000/01/rdf-schema#range>
                <https://w3id.org/roar#Document> ;
        <http://www.w3.org/2000/01/rdf-schema#subPropertyOf>
                <http://www.w3.org/2002/07/owl#topObjectProperty> .
