<https://www.ica.org/standards/RiC/ontology#activityIsTargetOfActivityDocumentationRelation>
        a       <http://www.w3.org/2002/07/owl#ObjectProperty> ;
        <http://www.w3.org/2000/01/rdf-schema#comment>
                "Connects an Activity to an Activity Documentation\n            Relation"@en ;
        <http://www.w3.org/2000/01/rdf-schema#domain>
                <https://www.ica.org/standards/RiC/ontology#Activity> ;
        <http://www.w3.org/2000/01/rdf-schema#isDefinedBy>
                <https://www.ica.org/standards/RiC/ontology> ;
        <http://www.w3.org/2000/01/rdf-schema#label>
                "activity is target of activity documentation relation\n        "@en ;
        <http://www.w3.org/2000/01/rdf-schema#range>
                <https://www.ica.org/standards/RiC/ontology#ActivityDocumentationRelation> ;
        <http://www.w3.org/2000/01/rdf-schema#subPropertyOf>
                <https://www.ica.org/standards/RiC/ontology#agentOrActivityIsTargetOfProvenanceRelation> ;
        <http://www.w3.org/2000/01/rdf-schema#subPropertyOf>
                []  .

<https://www.ica.org/standards/RiC/ontology#Activity>
        a       <http://www.w3.org/2002/07/owl#Class> ;
        <http://www.w3.org/2000/01/rdf-schema#comment>
                "The doing of something for some human purpose."@en ;
        <http://www.w3.org/2000/01/rdf-schema#isDefinedBy>
                <https://www.ica.org/standards/RiC/ontology> ;
        <http://www.w3.org/2000/01/rdf-schema#label>
                "Activity"@en ;
        <http://www.w3.org/2000/01/rdf-schema#subClassOf>
                <https://www.ica.org/standards/RiC/ontology#Event> ;
        <http://www.w3.org/2004/02/skos/core#scopeNote>
                "Activity is a kind of Event. Activity is specifically used to\n            designate purposeful human activity. Activity may be understood from two perspectives.\n            First it can be understood as leading to an end. The end is the purpose of the Activity,\n            or why the Activity is performed. Second, it can be understood in terms of the processes\n            that lead to achieving the end, how the end is realized through coordinated actions.\n            Purpose and process are complementary understandings of Activity. Together the two\n            perspectives address why the Activity is performed, the expected ends or outcomes; and\n            how the Activity fulfills the purpose. While activity has an intended end, it also has\n            unintended consequences and results, or side-effects. By and large, these may not be the\n            focus of the description, but they are, unquestionably, context. |In a corporate or\n            government context an Activity may also be called a 'function'. An Activity exists in a\n            specific social and cultural context, and within that context is subject to change over\n            time. An Activity may be composed of other Activities."@en ;
        <https://www.ica.org/standards/RiC/ontology#RiCCMCorrespondingComponent>
                "Corresponds to RiC-E15 (Activity\n            entity)"@en .

<https://www.ica.org/standards/RiC/ontology#activityDocumentationRelationHasTarget>
        a       <http://www.w3.org/2002/07/owl#ObjectProperty> ;
        <http://www.w3.org/2000/01/rdf-schema#comment>
                "Connects an Activity Documentation Relation to one of the\n            documented Activities"@en ;
        <http://www.w3.org/2000/01/rdf-schema#domain>
                <https://www.ica.org/standards/RiC/ontology#ActivityDocumentationRelation> ;
        <http://www.w3.org/2000/01/rdf-schema#isDefinedBy>
                <https://www.ica.org/standards/RiC/ontology> ;
        <http://www.w3.org/2000/01/rdf-schema#label>
                "activity documentation relation has target "@en ;
        <http://www.w3.org/2000/01/rdf-schema#range>
                <https://www.ica.org/standards/RiC/ontology#Activity> ;
        <http://www.w3.org/2000/01/rdf-schema#subPropertyOf>
                <https://www.ica.org/standards/RiC/ontology#provenanceRelationHasTarget> ;
        <http://www.w3.org/2000/01/rdf-schema#subPropertyOf>
                []  ;
        <http://www.w3.org/2002/07/owl#equivalentProperty>
                []  ;
        <http://www.w3.org/2002/07/owl#inverseOf>
                <https://www.ica.org/standards/RiC/ontology#activityIsTargetOfActivityDocumentationRelation> .

<https://www.ica.org/standards/RiC/ontology#ActivityDocumentationRelation>
        a       <http://www.w3.org/2002/07/owl#Class> ;
        <http://www.w3.org/2000/01/rdf-schema#comment>
                "Connects at least one Record Resource or Instantiation to at\n            least one Activity, when the Record Resource or Instantiation results from the\n            activity."@en ;
        <http://www.w3.org/2000/01/rdf-schema#isDefinedBy>
                <https://www.ica.org/standards/RiC/ontology> ;
        <http://www.w3.org/2000/01/rdf-schema#label>
                "Activity Documentation Relation"@en ;
        <http://www.w3.org/2000/01/rdf-schema#subClassOf>
                <https://www.ica.org/standards/RiC/ontology#ProvenanceRelation> ;
        <https://www.ica.org/standards/RiC/ontology#RiCCMCorrespondingComponent>
                "Class implementation of RiC-R033 and RiC-R033\n            relations"@en .
