<http://viaf.org/#AuthorityAgency>
        a       <http://www.w3.org/2002/07/owl#Class> ;
        <http://www.w3.org/2000/01/rdf-schema#comment>
                "\n\t\t\tNote that instances of this class live under\n\t\t\thttp://viaf.org/authorityAgency/*\n\t\t"@en ;
        <http://www.w3.org/2000/01/rdf-schema#isDefinedBy>
                <http://viaf.org/> ;
        <http://www.w3.org/2000/01/rdf-schema#subClassOf>
                <http://www.w3.org/2002/07/owl#Thing> .

<http://viaf.org/#NameAuthority>
        a       <http://www.w3.org/2002/07/owl#Class> ;
        <http://www.w3.org/2000/01/rdf-schema#comment>
                "\n\t\t\tNote that instances of this class live under\n\t\t\thttp://viaf.org/viaf/*\n\t\t"@en ;
        <http://www.w3.org/2000/01/rdf-schema#isDefinedBy>
                <http://viaf.org/> ;
        <http://www.w3.org/2000/01/rdf-schema#subClassOf>
                <http://www.w3.org/2002/07/owl#Thing> .

<http://viaf.org/#clusters>
        a       <http://www.w3.org/2002/07/owl#ObjectProperty> ;
        <http://www.w3.org/2000/01/rdf-schema#domain>
                <http://viaf.org/#NameAuthorityCluster> ;
        <http://www.w3.org/2000/01/rdf-schema#isDefinedBy>
                <http://viaf.org/> ;
        <http://www.w3.org/2000/01/rdf-schema#range>
                <http://viaf.org/#NameAuthority> ;
        <http://www.w3.org/2000/01/rdf-schema#subPropertyOf>
                <http://www.w3.org/2002/07/owl#topObjectProperty> .

<http://viaf.org/#wasCreatedBy>
        a       <http://www.w3.org/2002/07/owl#ObjectProperty> ;
        <http://www.w3.org/2000/01/rdf-schema#domain>
                <http://viaf.org/#NameAuthority> ;
        <http://www.w3.org/2000/01/rdf-schema#isDefinedBy>
                <http://viaf.org/> ;
        <http://www.w3.org/2000/01/rdf-schema#range>
                <http://viaf.org/#AuthorityAgency> ;
        <http://www.w3.org/2000/01/rdf-schema#subPropertyOf>
                <http://www.w3.org/2002/07/owl#topObjectProperty> .

<http://viaf.org/#NameAuthorityCluster>
        a       <http://www.w3.org/2002/07/owl#Class> ;
        <http://www.w3.org/2000/01/rdf-schema#comment>
                "\n\t\t\tNote that instancess of this class live under\n\t\t\thttp://viaf.org/nameAuthorityCluster/*\n\t\t"@en ;
        <http://www.w3.org/2000/01/rdf-schema#isDefinedBy>
                <http://viaf.org/> ;
        <http://www.w3.org/2000/01/rdf-schema#subClassOf>
                <http://www.w3.org/2002/07/owl#Thing> .
