<http://iflastandards.info/ns/fr/frbr/pressoo/Z2_Absorption>
        a       <http://www.w3.org/2002/07/owl#Class> ;
        <http://www.w3.org/2000/01/rdf-schema#comment>
                "This class comprises activities that result in instances of F18 Serial Work being absorbed by pre-existing instances of F18 Serial Work.\nAn absorption can be complete or only partial (e.g., a serial devoted to history in general can absorb specifically the portion devoted to the history of the Middle Ages of another serial that is devoted to the Middle Ages and Renaissance, while the portion devoted to the Renaissance is just abandoned). This information element can be reflected through the P2 has type (is type of): E55 Type from the CIDOC CRM model."@en ;
        <http://www.w3.org/2000/01/rdf-schema#label>
                "Absorption"@en ;
        <http://www.w3.org/2000/01/rdf-schema#subClassOf>
                <http://www.cidoc-crm.org/cidoc-crm/E7_Activity> .

<http://iflastandards.info/ns/fr/frbr/pressoo/Y10_enhanced>
        a       <http://www.w3.org/2002/07/owl#ObjectProperty> , <http://www.w3.org/2002/07/owl#AnnotationProperty> ;
        <http://www.w3.org/2000/01/rdf-schema#comment>
                "This property associates an instance of Z2 Absorption with an instance of F18 Serial Work that absorbed another instance of F18 Serial Work."@en ;
        <http://www.w3.org/2000/01/rdf-schema#domain>
                <http://iflastandards.info/ns/fr/frbr/pressoo/Z2_Absorption> ;
        <http://www.w3.org/2000/01/rdf-schema#label>
                "enhanced"@en ;
        <http://www.w3.org/2000/01/rdf-schema#range>
                <http://iflastandards.info/ns/fr/frbr/frbroo/F18_Serial_Work> ;
        <http://www.w3.org/2000/01/rdf-schema#subPropertyOf>
                <http://www.w3.org/2002/07/owl#topObjectProperty> , <http://www.cidoc-crm.org/cidoc-crm/P16_used_specific_object> .

<http://iflastandards.info/ns/fr/frbr/frbroo/F18_Serial_Work>
        a       <http://www.w3.org/2002/07/owl#Class> ;
        <http://www.w3.org/2000/01/rdf-schema#subClassOf>
                <http://www.w3.org/2002/07/owl#Thing> .

<http://iflastandards.info/ns/fr/frbr/pressoo/Y9_absorbed>
        a       <http://www.w3.org/2002/07/owl#ObjectProperty> , <http://www.w3.org/2002/07/owl#AnnotationProperty> ;
        <http://www.w3.org/2000/01/rdf-schema#comment>
                "This property associates an instance of Z2 Absorption with an instance of F18 Serial Work that was absorbed in another instance of F18 Serial Work."@en ;
        <http://www.w3.org/2000/01/rdf-schema#domain>
                <http://iflastandards.info/ns/fr/frbr/pressoo/Z2_Absorption> ;
        <http://www.w3.org/2000/01/rdf-schema#label>
                "absorbed"@en ;
        <http://www.w3.org/2000/01/rdf-schema#range>
                <http://iflastandards.info/ns/fr/frbr/frbroo/F18_Serial_Work> ;
        <http://www.w3.org/2000/01/rdf-schema#subPropertyOf>
                <http://www.w3.org/2002/07/owl#topObjectProperty> , <http://www.cidoc-crm.org/cidoc-crm/P16_used_specific_object> .

<http://iflastandards.info/ns/fr/frbr/pressoo/Y10i_was_enhanced_through>
        a       <http://www.w3.org/2002/07/owl#ObjectProperty> , <http://www.w3.org/2002/07/owl#AnnotationProperty> ;
        <http://www.w3.org/2000/01/rdf-schema#domain>
                <http://iflastandards.info/ns/fr/frbr/frbroo/F18_Serial_Work> ;
        <http://www.w3.org/2000/01/rdf-schema#label>
                "was enhanced through"@en ;
        <http://www.w3.org/2000/01/rdf-schema#range>
                <http://iflastandards.info/ns/fr/frbr/pressoo/Z2_Absorption> ;
        <http://www.w3.org/2000/01/rdf-schema#subPropertyOf>
                <http://www.w3.org/2002/07/owl#topObjectProperty> , <http://www.cidoc-crm.org/cidoc-crm/P16i_was_used_for> .

<http://iflastandards.info/ns/fr/frbr/pressoo/Y9i_was_absorbed_through>
        a       <http://www.w3.org/2002/07/owl#ObjectProperty> , <http://www.w3.org/2002/07/owl#AnnotationProperty> ;
        <http://www.w3.org/2000/01/rdf-schema#domain>
                <http://iflastandards.info/ns/fr/frbr/frbroo/F18_Serial_Work> ;
        <http://www.w3.org/2000/01/rdf-schema#label>
                "was absorbed through"@en ;
        <http://www.w3.org/2000/01/rdf-schema#range>
                <http://iflastandards.info/ns/fr/frbr/pressoo/Z2_Absorption> ;
        <http://www.w3.org/2000/01/rdf-schema#subPropertyOf>
                <http://www.w3.org/2002/07/owl#topObjectProperty> , <http://www.cidoc-crm.org/cidoc-crm/P16i_was_used_for> .
