<http://iflastandards.info/ns/fr/frbr/frbroo/R45_assigned_to>
        a       <http://www.w3.org/2002/07/owl#ObjectProperty> ;
        <http://www.w3.org/2000/01/rdf-schema#comment>
                "This property identifies the entity to which an actor, such as a bibliographic agency, assigned an instance of F13 Identifier.\n"@en ;
        <http://www.w3.org/2000/01/rdf-schema#domain>
                <http://iflastandards.info/ns/fr/frbr/frbroo/F40_Identifier_Assignment> ;
        <http://www.w3.org/2000/01/rdf-schema#label>
                "assigned to"@en ;
        <http://www.w3.org/2000/01/rdf-schema#range>
                <http://www.cidoc-crm.org/cidoc-crm/E1_CRM_Entity> ;
        <http://www.w3.org/2000/01/rdf-schema#subPropertyOf>
                <http://www.w3.org/2002/07/owl#topObjectProperty> .

<http://www.cidoc-crm.org/cidoc-crm/E1_CRM_Entity>
        a       <http://www.w3.org/2002/07/owl#Class> ;
        <http://www.w3.org/2000/01/rdf-schema#subClassOf>
                <http://www.w3.org/2002/07/owl#Thing> .

<http://iflastandards.info/ns/fr/frbr/frbroo/R46i_was_assigned_by>
        a       <http://www.w3.org/2002/07/owl#ObjectProperty> ;
        <http://www.w3.org/2000/01/rdf-schema#comment>
                "\n"@en ;
        <http://www.w3.org/2000/01/rdf-schema#domain>
                <http://iflastandards.info/ns/fr/frbr/frbroo/F13_Identifier> ;
        <http://www.w3.org/2000/01/rdf-schema#label>
                "was assigned by"@en ;
        <http://www.w3.org/2000/01/rdf-schema#range>
                <http://iflastandards.info/ns/fr/frbr/frbroo/F40_Identifier_Assignment> ;
        <http://www.w3.org/2000/01/rdf-schema#subPropertyOf>
                <http://www.w3.org/2002/07/owl#topObjectProperty> .

<http://iflastandards.info/ns/fr/frbr/frbroo/R45i_was_assigned_by>
        a       <http://www.w3.org/2002/07/owl#ObjectProperty> ;
        <http://www.w3.org/2000/01/rdf-schema#comment>
                "\n"@en ;
        <http://www.w3.org/2000/01/rdf-schema#domain>
                <http://www.cidoc-crm.org/cidoc-crm/E1_CRM_Entity> ;
        <http://www.w3.org/2000/01/rdf-schema#label>
                "was assigned by"@en ;
        <http://www.w3.org/2000/01/rdf-schema#range>
                <http://iflastandards.info/ns/fr/frbr/frbroo/F40_Identifier_Assignment> ;
        <http://www.w3.org/2000/01/rdf-schema#subPropertyOf>
                <http://www.w3.org/2002/07/owl#topObjectProperty> .

<http://iflastandards.info/ns/fr/frbr/frbroo/F13_Identifier>
        a       <http://www.w3.org/2002/07/owl#Class> ;
        <http://www.w3.org/2000/01/rdf-schema#comment>
                "This class comprises strings or codes assigned to instances of E1 CRM Entity in order to identify them uniquely and permanently within the context of one or more organisations. Such codes are often known as inventory numbers, registration codes, etc. and are typically composed of alphanumeric sequences. The class E42 Identifier is not normally used for machine-generated identifiers used for automated processing unless these are also used by human agents. [Adapted from the Scope Note of CIDOC CRM E42 Identifier ver. 5.0.1]\n"@en ;
        <http://www.w3.org/2000/01/rdf-schema#label>
                "Identifier"@en ;
        <http://www.w3.org/2000/01/rdf-schema#subClassOf>
                <http://www.cidoc-crm.org/cidoc-crm/E42_Identifier> , <http://iflastandards.info/ns/fr/frbr/frbroo/F12_Nomen> .

<http://iflastandards.info/ns/fr/frbr/frbroo/R46_assigned_to>
        a       <http://www.w3.org/2002/07/owl#ObjectProperty> ;
        <http://www.w3.org/2000/01/rdf-schema#comment>
                "This property associates the instance of F13 Identifier assigned to an instance of E1 CRM Entity and the event of assigning it.\n"@en ;
        <http://www.w3.org/2000/01/rdf-schema#domain>
                <http://iflastandards.info/ns/fr/frbr/frbroo/F40_Identifier_Assignment> ;
        <http://www.w3.org/2000/01/rdf-schema#label>
                "assigned to"@en ;
        <http://www.w3.org/2000/01/rdf-schema#range>
                <http://iflastandards.info/ns/fr/frbr/frbroo/F13_Identifier> ;
        <http://www.w3.org/2000/01/rdf-schema#subPropertyOf>
                <http://www.w3.org/2002/07/owl#topObjectProperty> .

<http://iflastandards.info/ns/fr/frbr/frbroo/F40_Identifier_Assignment>
        a       <http://www.w3.org/2002/07/owl#Class> ;
        <http://www.w3.org/2000/01/rdf-schema#comment>
                "This class comprises activities that result in the allocation of an identifier to an instance of any subclass of E1 CRM Entity. An F40 Identifier Assignment may include the creation of the identifier from multiple constituents. Explicit reference to the used constituents can be made using the property P142 used constituent (was used in). The syntax of the identifier and the kinds of constituents to be used in constructing it may be declared in a rule. The construction of controlled access points for the names of persons, families and corporate bodies following specific cataloguing rules is a typical library application of identifier assignment. F40 Identifier Assignment also includes the assignment of controlled access points for works or expressions.\n"@en ;
        <http://www.w3.org/2000/01/rdf-schema#label>
                "Identifier Assignment"@en ;
        <http://www.w3.org/2000/01/rdf-schema#subClassOf>
                <http://www.cidoc-crm.org/cidoc-crm/E15_Identifier_Assignment> .
