<http://iflastandards.info/ns/fr/frbr/frbroo/R12_is_realised_in>
        a       <http://www.w3.org/2002/07/owl#ObjectProperty> ;
        <http://www.w3.org/2000/01/rdf-schema#comment>
                "This property associates an instance of F20 Performance Work with an instance of F25 Performance Plan that consists of signs (words, figures, etc.) which express the directions the instance of F20 Performance Work consists of.\n"@en ;
        <http://www.w3.org/2000/01/rdf-schema#domain>
                <http://iflastandards.info/ns/fr/frbr/frbroo/F20_Performance_Work> ;
        <http://www.w3.org/2000/01/rdf-schema#label>
                "is realised in"@en ;
        <http://www.w3.org/2000/01/rdf-schema#range>
                <http://iflastandards.info/ns/fr/frbr/frbroo/F25_Performance_Plan> ;
        <http://www.w3.org/2000/01/rdf-schema#subPropertyOf>
                <http://www.w3.org/2002/07/owl#topObjectProperty> .

<http://iflastandards.info/ns/fr/frbr/frbroo/F31_Performance>
        a       <http://www.w3.org/2002/07/owl#Class> ;
        <http://www.w3.org/2000/01/rdf-schema#comment>
                "This class comprises activities that follow the directions of a performance plan, such as a theatrical play, an expression of a choreographic work or a musical work; i.e., they are intended to communicate directly or indirectly to an audience.\nSuch activities can be identified at various levels of granularity, and can be contiguous or not. Any individual performance (with or without intermissions) is a single instance of F31 Performance. In addition, a complete run of performances can also be seen as an instance of F31 Performance, with individual performances as parts. A complete run of performances may comprise an original run plus any of its extensions and tours.\nNote that a performance plan may be more or less elaborate, and may even foresee just improvisation.\n"@en ;
        <http://www.w3.org/2000/01/rdf-schema#label>
                "Performance"@en ;
        <http://www.w3.org/2000/01/rdf-schema#subClassOf>
                <http://www.cidoc-crm.org/cidoc-crm/E7_Activity> .

<http://iflastandards.info/ns/fr/frbr/frbroo/F25_Performance_Plan>
        a       <http://www.w3.org/2002/07/owl#Class> ;
        <http://www.w3.org/2000/01/rdf-schema#comment>
                "This class comprises sets of directions to which individual performances of theatrical, choreographic, or musical works and their combinations should conform.\nIn the case of theatrical performances, such directions incorporate, but are not limited nor reducible to, the text of a given version of the play performed (e.g., a translated text, some passages of which are deliberately omitted, with some rephrased lines, etc.).\nIn the case of choreographic performances, such directions may incorporate, but are neither limited nor reducible to, the notation of choreographic movements in systems such as labanotation.\nIn the case of musical performances, such directions may incorporate, but are neither limited nor reducible to, the musical score. In case of electronic music, they may incorporate software instructions.\nThese directions may or may not completely determine the form of the intended performance. Depending on the nature of the directions, the form of the intended performance, such as the sets of movements or the sound characteristics, may or may not be predictable from the directions.\nNote that a performance plan may be more or less elaborate, and may even foresee just improvisation.\n"@en ;
        <http://www.w3.org/2000/01/rdf-schema#label>
                "Performance Plan"@en ;
        <http://www.w3.org/2000/01/rdf-schema#subClassOf>
                <http://www.cidoc-crm.org/cidoc-crm/E29_Design_or_Procedure> , <http://iflastandards.info/ns/fr/frbr/frbroo/F22_Self-Contained_Expression> .

<http://iflastandards.info/ns/fr/frbr/frbroo/R25_performed>
        a       <http://www.w3.org/2002/07/owl#ObjectProperty> ;
        <http://www.w3.org/2000/01/rdf-schema#comment>
                "This property associates an instance of F31 Performance with the instance of F25 Performance Plan to which all those participating in the performance were supposed to conform.\n"@en ;
        <http://www.w3.org/2000/01/rdf-schema#domain>
                <http://iflastandards.info/ns/fr/frbr/frbroo/F31_Performance> ;
        <http://www.w3.org/2000/01/rdf-schema#label>
                "performed"@en ;
        <http://www.w3.org/2000/01/rdf-schema#range>
                <http://iflastandards.info/ns/fr/frbr/frbroo/F25_Performance_Plan> ;
        <http://www.w3.org/2000/01/rdf-schema#subPropertyOf>
                <http://www.w3.org/2002/07/owl#topObjectProperty> .

<http://iflastandards.info/ns/fr/frbr/frbroo/F20_Performance_Work>
        a       <http://www.w3.org/2002/07/owl#Class> ;
        <http://www.w3.org/2000/01/rdf-schema#comment>
                "This class comprises the sets of concepts for rendering a particular or a series of like performances.\nF20 Performance Work is declared as a subclass of F16 Container Work. This implies that the incorporated expressions (such as the text of the staged play, the text of the argument for the ballet, the recorded music to be used for the ballet, or the content of the musical score to be used for a concert, etc.) are not by themselves a part of the expression of this F1 Work. Rather, an expression (F25 Performance Plan) of the instructions the stage production, choreography or musical performance consists of incorporates (P165) that textual or musical content. In other words, the text of ‘Hamlet’ is not a component of the concepts that underlie a given mise-en-scène of ‘Hamlet’, but any staging directions (F25 Performance Plan) that convey a given director’s vision of ‘Hamlet’ must necessarily incorporate the text of ‘Hamlet’.\n"@en ;
        <http://www.w3.org/2000/01/rdf-schema#label>
                "Performance Work"@en ;
        <http://www.w3.org/2000/01/rdf-schema#subClassOf>
                <http://iflastandards.info/ns/fr/frbr/frbroo/F16_Container_Work> .

<http://iflastandards.info/ns/fr/frbr/frbroo/R12i_realises>
        a       <http://www.w3.org/2002/07/owl#ObjectProperty> ;
        <http://www.w3.org/2000/01/rdf-schema#comment>
                "\n"@en ;
        <http://www.w3.org/2000/01/rdf-schema#domain>
                <http://iflastandards.info/ns/fr/frbr/frbroo/F25_Performance_Plan> ;
        <http://www.w3.org/2000/01/rdf-schema#label>
                "realises"@en ;
        <http://www.w3.org/2000/01/rdf-schema#range>
                <http://iflastandards.info/ns/fr/frbr/frbroo/F20_Performance_Work> ;
        <http://www.w3.org/2000/01/rdf-schema#subPropertyOf>
                <http://www.w3.org/2002/07/owl#topObjectProperty> .
