<http://iflastandards.info/ns/fr/frbr/frbroo/R53i_was_assigned_by>
        a       <http://www.w3.org/2002/07/owl#ObjectProperty> ;
        <http://www.w3.org/2000/01/rdf-schema#comment>
                "\n"@en ;
        <http://www.w3.org/2000/01/rdf-schema#domain>
                <http://iflastandards.info/ns/fr/frbr/frbroo/F4_Manifestation_Singleton> ;
        <http://www.w3.org/2000/01/rdf-schema#label>
                "was assigned by"@en ;
        <http://www.w3.org/2000/01/rdf-schema#range>
                <http://iflastandards.info/ns/fr/frbr/frbroo/F41_Representative_Manifestation_Assignment> ;
        <http://www.w3.org/2000/01/rdf-schema#subPropertyOf>
                <http://www.w3.org/2002/07/owl#topObjectProperty> .

<http://iflastandards.info/ns/fr/frbr/frbroo/F2_Expression>
        a       <http://www.w3.org/2002/07/owl#Class> ;
        <http://www.w3.org/2000/01/rdf-schema#comment>
                "This class comprises the intellectual or artistic realisations of works in the form of identifiable immaterial objects, such as texts, poems, jokes, musical or choreographic notations, movement pattern, sound pattern, images, multimedia objects, or any combination of such forms that have objectively recognisable structures. The substance of F2 Expression is signs.\nExpressions cannot exist without a physical carrier, but do not depend on a specific physical carrier and can exist on one or more carriers simultaneously. Carriers may include human memory.\nInasmuch as the form of F2 Expression is an inherent characteristic of the F2 Expression, any change in form (e.g., from alpha-numeric notation to spoken word, a poem created in capitals and rendered in lower case) is a new F2 Expression. Similarly, changes in the intellectual conventions or instruments that are employed to express a work (e.g., translation from one language to another) result in the creation of a new F2 Expression. Thus, if a text is revised or modified, the resulting F2 Expression is considered to be a new F2 Expression. Minor changes, such as corrections of spelling and punctuation, etc., are normally considered variations within the same F2 Expression. On a practical level, the degree to which distinctions are made between variant expressions of a work will depend to some extent on the nature of the F1 Work itself, and on the anticipated needs of users.\nThe genre of the work may provide an indication of which features are essential to the expression. In some cases, aspects of physical form, such as typeface and page layout, are not integral to the intellectual or artistic realisation of the work as such, and therefore are not distinctive criteria for the respective expressions. For another work, features such as layout may be essential. For instance, the author or a graphic designer may wrap a poem around an image.\nAn expression of a work may include expressions of other works within it. For instance, an anthology of poems is regarded as a work in its own right that makes use of expressions of the individual poems that have been selected and ordered as part of an intellectual process. This does not make the contents of the aggregated expressions part of this work, but only parts of the resulting expression.\nIf an instance of F2 Expression is of a specific form, such as text, image, etc., it may be simultaneously instantiated in the specific classes representing these forms in CIDOC CRM. Thereby one can make use of the more specific properties of these classes, such as language (which is applicable to instances of E33 Linguistic Object only).\n"@en ;
        <http://www.w3.org/2000/01/rdf-schema#label>
                "Expression"@en ;
        <http://www.w3.org/2000/01/rdf-schema#subClassOf>
                <http://www.cidoc-crm.org/cidoc-crm/E73_Information_Object> .

<http://iflastandards.info/ns/fr/frbr/frbroo/F41_Representative_Manifestation_Assignment>
        a       <http://www.w3.org/2002/07/owl#Class> ;
        <http://www.w3.org/2000/01/rdf-schema#comment>
                "This class comprises activities through which an Agency declares (implicitly or explicitly) that a given instance of F3 Manifestation Product Type or F4 Manifestation Singleton is representative for a given F2 Expression, i.e., that some features found on that instance of F3 Manifestation Product Type or F4 Manifestation Singleton (most prominently, information about the title) can be inferred to also apply to that instance of F2 Expression, no matter within which manifestation it is embodied.\nThe reasoning behind is that the Work title is known through the title of an Expression that is deemed representative of the Work, and the title of the representative Expression is known through the title proper of a Manifestation that is deemed representative of the Expression representative of the Work.\n"@en ;
        <http://www.w3.org/2000/01/rdf-schema#label>
                "Representative Manifestation Assignment"@en ;
        <http://www.w3.org/2000/01/rdf-schema#subClassOf>
                <http://www.cidoc-crm.org/cidoc-crm/E13_Attribute_Assignment> .

<http://iflastandards.info/ns/fr/frbr/frbroo/F44_Bibliographic_Agency>
        a       <http://www.w3.org/2002/07/owl#Class> ;
        <http://www.w3.org/2000/01/rdf-schema#comment>
                "This class comprises agents who create the bibliographic description of publications and perform the authority control associated with such descriptions, for the description of copies of such publications actually held by libraries, and for the description of unique documents (manuscripts, objects…) held by libraries.\nThe activity of creating such descriptions implies that one has to make decisions (as to the controlled access point for a work, as to whether an arrangement still belongs to the same work or is definitely a new work, etc.). Since such decisions always are debatable and different agencies can make different decisions about the same real-world entities, it is important to document which agency made which decision.\n"@en ;
        <http://www.w3.org/2000/01/rdf-schema#label>
                "Bibliographic Agency"@en ;
        <http://www.w3.org/2000/01/rdf-schema#subClassOf>
                <http://www.cidoc-crm.org/cidoc-crm/E40_Legal_Body> .

<http://iflastandards.info/ns/fr/frbr/frbroo/R43_carried_out_by>
        a       <http://www.w3.org/2002/07/owl#ObjectProperty> ;
        <http://www.w3.org/2000/01/rdf-schema#comment>
                "This property associates a bibliographic agency (represented by one or more of its cataloguers) and the assigning of which Manifestation (i.e., which instance of F3 Manifestation Product Type or F4 Manifestation Singleton) is representative for a given expression.\nIn cataloguing practice, such a relationship is usually just implicit. However, it can become explicit, for example when a bibliographic agency creates an authority record for a given work and fills the “Source” field with information about the publication that contains the expression that was used by the bibliographic agency to establish the controlled access point for the work realised in that expression.\n"@en ;
        <http://www.w3.org/2000/01/rdf-schema#domain>
                <http://iflastandards.info/ns/fr/frbr/frbroo/F41_Representative_Manifestation_Assignment> ;
        <http://www.w3.org/2000/01/rdf-schema#label>
                "carried out by"@en ;
        <http://www.w3.org/2000/01/rdf-schema#range>
                <http://iflastandards.info/ns/fr/frbr/frbroo/F44_Bibliographic_Agency> ;
        <http://www.w3.org/2000/01/rdf-schema#subPropertyOf>
                <http://www.w3.org/2002/07/owl#topObjectProperty> .

<http://iflastandards.info/ns/fr/frbr/frbroo/R48_assigned_to>
        a       <http://www.w3.org/2002/07/owl#ObjectProperty> ;
        <http://www.w3.org/2000/01/rdf-schema#comment>
                "This property associates the event of assigning a representative instance of F3 Manifestation Product Type or F4 Manifestation Singleton with the expression to which it was assigned.\n"@en ;
        <http://www.w3.org/2000/01/rdf-schema#domain>
                <http://iflastandards.info/ns/fr/frbr/frbroo/F41_Representative_Manifestation_Assignment> ;
        <http://www.w3.org/2000/01/rdf-schema#label>
                "assigned to"@en ;
        <http://www.w3.org/2000/01/rdf-schema#range>
                <http://iflastandards.info/ns/fr/frbr/frbroo/F2_Expression> ;
        <http://www.w3.org/2000/01/rdf-schema#subPropertyOf>
                <http://www.w3.org/2002/07/owl#topObjectProperty> .

<http://iflastandards.info/ns/fr/frbr/frbroo/F4_Manifestation_Singleton>
        a       <http://www.w3.org/2002/07/owl#Class> ;
        <http://www.w3.org/2000/01/rdf-schema#comment>
                "This class comprises physical objects that each carry an instance of F2 Expression, and that were produced as unique objects, with no siblings intended in the course of their production. It should be noted that if all but one copy of a given publication are destroyed, then that copy does not become an instance of F4 Manifestation Singleton, because it was produced together with sibling copies, even though it now happens to be unique. Examples of instances of F4 Manifestation Singleton include manuscripts, preparatory sketches and the final clean draft sent by an author or a composer to a publisher.\n"@en ;
        <http://www.w3.org/2000/01/rdf-schema#label>
                "Manifestation Singleton"@en ;
        <http://www.w3.org/2000/01/rdf-schema#subClassOf>
                <http://www.cidoc-crm.org/cidoc-crm/E24_Physical_Man-Made_Thing> .
