<http://www.cidoc-crm.org/cidoc-crm/E73_Information_Object>
        a       <http://www.w3.org/2002/07/owl#Class> ;
        <http://www.w3.org/2000/01/rdf-schema#comment>
                "This class comprises identifiable immaterial items, such as a poems, jokes, data sets, images, texts, multimedia objects, procedural prescriptions, computer program code, algorithm or mathematical formulae, that have an objectively recognizable structure and are documented as single units. The encoding structure known as a \"named graph\" also falls under this class, so that each \"named graph\" is an instance of an E73 Information Object. \nAn E73 Information Object does not depend on a specific physical carrier, which can include human memory, and it can exist on one or more carriers simultaneously. \nInstances of E73 Information Object of a linguistic nature should be declared as instances of the E33 Linguistic Object subclass. Instances of E73 Information Object of a documentary nature should be declared as instances of the E31 Document subclass. Conceptual items such as types and classes are not instances of E73 Information Object, nor are ideas without a reproducible expression. \n "@en ;
        <http://www.w3.org/2000/01/rdf-schema#label>
                "信息物件"@zh , "Informationsgegenstand"@de , "Information Object"@en , "Objeto de Informação"@pt , "Информационный Объект"@ru , "Πληροφοριακό Αντικείμενο"@el , "Objet d'information"@fr ;
        <http://www.w3.org/2000/01/rdf-schema#subClassOf>
                <http://www.cidoc-crm.org/cidoc-crm/E89_Propositional_Object> , <http://www.cidoc-crm.org/cidoc-crm/E90_Symbolic_Object> .

<http://www.cidoc-crm.org/cidoc-crm/P165_incorporates>
        a       <http://www.w3.org/2002/07/owl#ObjectProperty> ;
        <http://www.w3.org/2000/01/rdf-schema#comment>
                "This property associates an instance of E73 Information Object with an instance of E90 Symbolic Object (or any of its subclasses) that was included in it.\nThis property makes it possible to recognise the autonomous status of the incorporated signs, which were created in a distinct context, and can be incorporated in many distinct self-contained expressions, and to highlight the difference between structural and accidental whole-part relationships between conceptual entities.\nIt accounts for many cultural facts that are quite frequent and significant: the inclusion of a poem in an anthology, the re-use of an operatic aria in a new opera, the use of a reproduction of a painting for a book cover or a CD booklet, the integration of textual quotations, the presence of lyrics in a song that sets those lyrics to music, the presence of the text of a play in a movie based on that play, etc.\nIn particular, this property allows for modelling relationships of different levels of symbolic specificity, such as the natural language words making up a particular text, the characters making up the words and punctuation, the choice of fonts and page layout for the characters.\nA digital photograph of a manuscript page incorporates the text of the manuscript page.\n\t"@en ;
        <http://www.w3.org/2000/01/rdf-schema#domain>
                <http://www.cidoc-crm.org/cidoc-crm/E73_Information_Object> ;
        <http://www.w3.org/2000/01/rdf-schema#label>
                "incorporates"@en ;
        <http://www.w3.org/2000/01/rdf-schema#range>
                <http://www.cidoc-crm.org/cidoc-crm/E90_Symbolic_Object> ;
        <http://www.w3.org/2000/01/rdf-schema#subPropertyOf>
                <http://www.cidoc-crm.org/cidoc-crm/P106_is_composed_of> .

<http://www.cidoc-crm.org/cidoc-crm/E90_Symbolic_Object>
        a       <http://www.w3.org/2002/07/owl#Class> ;
        <http://www.w3.org/2000/01/rdf-schema#comment>
                "This class comprises identifiable symbols and any aggregation of symbols, such as characters, identifiers, traffic signs, emblems, texts, data sets, images, musical scores, multimedia objects, computer program code or mathematical formulae that have an objectively recognizable structure and that are documented as single units.\n\tIt includes sets of signs of any nature, which may serve to designate something, or to communicate some propositional content.\n\tAn instance of E90 Symbolic Object does not depend on a specific physical carrier, which can include human memory, and it can exist on one or more carriers simultaneously. An instance of E90 Symbolic Object may or may not have a specific meaning, for example an arbitrary character string.\n\tIn some cases, the content of an instance of E90 Symbolic Object may completely be represented by a serialized content model, such.. as the property P3 has note allows for describing this content model…P3.1 has type: E55 Type to specify the encoding..\n"@en ;
        <http://www.w3.org/2000/01/rdf-schema#label>
                "符号物件"@zh , "Symbolisches Objekt"@de , "Symbolic Object"@en ;
        <http://www.w3.org/2000/01/rdf-schema#subClassOf>
                <http://www.cidoc-crm.org/cidoc-crm/E72_Legal_Object> , <http://www.cidoc-crm.org/cidoc-crm/E28_Conceptual_Object> .

<http://www.cidoc-crm.org/cidoc-crm/P165i_is_incorporated_in>
        a       <http://www.w3.org/2002/07/owl#ObjectProperty> ;
        <http://www.w3.org/2000/01/rdf-schema#domain>
                <http://www.cidoc-crm.org/cidoc-crm/E90_Symbolic_Object> ;
        <http://www.w3.org/2000/01/rdf-schema#label>
                "is incorporated in"@en ;
        <http://www.w3.org/2000/01/rdf-schema#range>
                <http://www.cidoc-crm.org/cidoc-crm/E73_Information_Object> ;
        <http://www.w3.org/2000/01/rdf-schema#subPropertyOf>
                <http://www.cidoc-crm.org/cidoc-crm/P106i_forms_part_of> .
