<http://iflastandards.info/ns/fr/frbr/pressoo/Y14_substituted_with>
        a       <http://www.w3.org/2002/07/owl#ObjectProperty> , <http://www.w3.org/2002/07/owl#AnnotationProperty> ;
        <http://www.w3.org/2000/01/rdf-schema#comment>
                "This property associates an instance of Z4 Temporary Substitution with an instance of F18 Serial Work that temporarily replaced a distinct instance of F18 Serial Work the publication of which was interrupted."@en ;
        <http://www.w3.org/2000/01/rdf-schema#domain>
                <http://iflastandards.info/ns/fr/frbr/pressoo/Z4_Temporary_Substitution> ;
        <http://www.w3.org/2000/01/rdf-schema#label>
                "substituted with"@en ;
        <http://www.w3.org/2000/01/rdf-schema#range>
                <http://iflastandards.info/ns/fr/frbr/frbroo/F18_Serial_Work> ;
        <http://www.w3.org/2000/01/rdf-schema#subPropertyOf>
                <http://www.w3.org/2002/07/owl#topObjectProperty> , <http://www.cidoc-crm.org/cidoc-crm/P16_used_specific_object> .

<http://iflastandards.info/ns/fr/frbr/pressoo/Y13_provided_surrogate_to>
        a       <http://www.w3.org/2002/07/owl#ObjectProperty> , <http://www.w3.org/2002/07/owl#AnnotationProperty> ;
        <http://www.w3.org/2000/01/rdf-schema#comment>
                "This property associates an instance of Z4 Temporary Substitution with an instance of F18 Serial Work the publication of which was interrupted and replaced with the publication of a distinct instance of F18 Serial Work."@en ;
        <http://www.w3.org/2000/01/rdf-schema#domain>
                <http://iflastandards.info/ns/fr/frbr/pressoo/Z4_Temporary_Substitution> ;
        <http://www.w3.org/2000/01/rdf-schema#label>
                "provided surrogate to"@en ;
        <http://www.w3.org/2000/01/rdf-schema#range>
                <http://iflastandards.info/ns/fr/frbr/frbroo/F18_Serial_Work> ;
        <http://www.w3.org/2000/01/rdf-schema#subPropertyOf>
                <http://www.w3.org/2002/07/owl#topObjectProperty> , <http://iflastandards.info/ns/fr/frbr/frbroo/R23_created_a_realization_of> .

<http://iflastandards.info/ns/fr/frbr/frbroo/F18_Serial_Work>
        a       <http://www.w3.org/2002/07/owl#Class> ;
        <http://www.w3.org/2000/01/rdf-schema#subClassOf>
                <http://www.w3.org/2002/07/owl#Thing> .

<http://iflastandards.info/ns/fr/frbr/pressoo/Y14i_became_surrogate_through>
        a       <http://www.w3.org/2002/07/owl#ObjectProperty> , <http://www.w3.org/2002/07/owl#AnnotationProperty> ;
        <http://www.w3.org/2000/01/rdf-schema#domain>
                <http://iflastandards.info/ns/fr/frbr/frbroo/F18_Serial_Work> ;
        <http://www.w3.org/2000/01/rdf-schema#label>
                "became surrogate through"@en ;
        <http://www.w3.org/2000/01/rdf-schema#range>
                <http://iflastandards.info/ns/fr/frbr/pressoo/Z4_Temporary_Substitution> ;
        <http://www.w3.org/2000/01/rdf-schema#subPropertyOf>
                <http://www.w3.org/2002/07/owl#topObjectProperty> , <http://www.cidoc-crm.org/cidoc-crm/P16i_was_used_for> .

<http://iflastandards.info/ns/fr/frbr/pressoo/Y13i_had_surrogate_through>
        a       <http://www.w3.org/2002/07/owl#ObjectProperty> , <http://www.w3.org/2002/07/owl#AnnotationProperty> ;
        <http://www.w3.org/2000/01/rdf-schema#domain>
                <http://iflastandards.info/ns/fr/frbr/frbroo/F18_Serial_Work> ;
        <http://www.w3.org/2000/01/rdf-schema#label>
                "had surrogate through"@en ;
        <http://www.w3.org/2000/01/rdf-schema#range>
                <http://iflastandards.info/ns/fr/frbr/pressoo/Z4_Temporary_Substitution> ;
        <http://www.w3.org/2000/01/rdf-schema#subPropertyOf>
                <http://www.w3.org/2002/07/owl#topObjectProperty> , <http://iflastandards.info/ns/fr/frbr/frbroo/R23i_was_realised_through> .

<http://iflastandards.info/ns/fr/frbr/pressoo/Z4_Temporary_Substitution>
        a       <http://www.w3.org/2002/07/owl#Class> ;
        <http://www.w3.org/2000/01/rdf-schema#comment>
                "replacement for another instance of F18 Serial Work. The replacing instance of F18 Serial Work can either pre-exist the replacement, or be created specifically for the purpose of replacing the other instance of F18 Serial Work."@en ;
        <http://www.w3.org/2000/01/rdf-schema#label>
                "Temporary Substitution"@en ;
        <http://www.w3.org/2000/01/rdf-schema#subClassOf>
                <http://iflastandards.info/ns/fr/frbr/frbroo/F30_Publication_Event> .
