<http://iflastandards.info/ns/fr/frbr/pressoo/Y3i_was_replaced_through>
        a       <http://www.w3.org/2002/07/owl#ObjectProperty> ;
        <http://www.w3.org/2000/01/rdf-schema#domain>
                <http://iflastandards.info/ns/fr/frbr/frbroo/F18_Serial_Work> ;
        <http://www.w3.org/2000/01/rdf-schema#label>
                "was replaced through"@en ;
        <http://www.w3.org/2000/01/rdf-schema#range>
                <http://iflastandards.info/ns/fr/frbr/pressoo/Z1_Serial_Transformation> ;
        <http://www.w3.org/2000/01/rdf-schema#subPropertyOf>
                <http://www.w3.org/2002/07/owl#topObjectProperty> .

<http://iflastandards.info/ns/fr/frbr/pressoo/Y5i_was_split_through>
        a       <http://www.w3.org/2002/07/owl#ObjectProperty> ;
        <http://www.w3.org/2000/01/rdf-schema#domain>
                <http://iflastandards.info/ns/fr/frbr/frbroo/F18_Serial_Work> ;
        <http://www.w3.org/2000/01/rdf-schema#label>
                "was split through"@en ;
        <http://www.w3.org/2000/01/rdf-schema#range>
                <http://iflastandards.info/ns/fr/frbr/pressoo/Z1_Serial_Transformation> ;
        <http://www.w3.org/2000/01/rdf-schema#subPropertyOf>
                <http://www.w3.org/2002/07/owl#topObjectProperty> .

<http://iflastandards.info/ns/fr/frbr/pressoo/Y8_merged_into>
        a       <http://www.w3.org/2002/07/owl#ObjectProperty> , <http://www.w3.org/2002/07/owl#AnnotationProperty> ;
        <http://www.w3.org/2000/01/rdf-schema#comment>
                "This property associates an instance of Z1 Serial Transformation with the instance of F18 Serial Work that resulted from merging other instances of F18 Serial Work."@en ;
        <http://www.w3.org/2000/01/rdf-schema#domain>
                <http://iflastandards.info/ns/fr/frbr/pressoo/Z1_Serial_Transformation> ;
        <http://www.w3.org/2000/01/rdf-schema#label>
                "merged into"@en ;
        <http://www.w3.org/2000/01/rdf-schema#range>
                <http://iflastandards.info/ns/fr/frbr/frbroo/F18_Serial_Work> ;
        <http://www.w3.org/2000/01/rdf-schema#subPropertyOf>
                <http://www.w3.org/2002/07/owl#topObjectProperty> , <http://iflastandards.info/ns/fr/frbr/frbroo/R16_initiated> .

<http://iflastandards.info/ns/fr/frbr/pressoo/Y1_provided_a_continuation_to>
        a       <http://www.w3.org/2002/07/owl#ObjectProperty> ;
        <http://www.w3.org/2000/01/rdf-schema#comment>
                "This property associates an instance of Z1 Serial Transformation with an instance of F18 Serial Work that underwent a ‘major’ title change that transformed it into another instance of F18 Serial Work."@en ;
        <http://www.w3.org/2000/01/rdf-schema#domain>
                <http://iflastandards.info/ns/fr/frbr/pressoo/Z1_Serial_Transformation> ;
        <http://www.w3.org/2000/01/rdf-schema#label>
                "provided a continuation to"@en ;
        <http://www.w3.org/2000/01/rdf-schema#range>
                <http://iflastandards.info/ns/fr/frbr/frbroo/F18_Serial_Work> ;
        <http://www.w3.org/2000/01/rdf-schema#subPropertyOf>
                <http://www.w3.org/2002/07/owl#topObjectProperty> .

<http://iflastandards.info/ns/fr/frbr/pressoo/Y7_merged>
        a       <http://www.w3.org/2002/07/owl#ObjectProperty> ;
        <http://www.w3.org/2000/01/rdf-schema#comment>
                "This property associates an instance of Z1 Serial Transformation with any one of the instances of F18 Serial Work that were merged with each other in order to create a new instance of F18 Serial Work."@en ;
        <http://www.w3.org/2000/01/rdf-schema#domain>
                <http://iflastandards.info/ns/fr/frbr/pressoo/Z1_Serial_Transformation> ;
        <http://www.w3.org/2000/01/rdf-schema#label>
                "merged"@en ;
        <http://www.w3.org/2000/01/rdf-schema#range>
                <http://iflastandards.info/ns/fr/frbr/frbroo/F18_Serial_Work> ;
        <http://www.w3.org/2000/01/rdf-schema#subPropertyOf>
                <http://www.w3.org/2002/07/owl#topObjectProperty> .

<http://iflastandards.info/ns/fr/frbr/pressoo/Y6_initiated>
        a       <http://www.w3.org/2002/07/owl#ObjectProperty> , <http://www.w3.org/2002/07/owl#AnnotationProperty> ;
        <http://www.w3.org/2000/01/rdf-schema#comment>
                "This property associates an instance of Z1 Serial Transformation with one or more than one instance of F18 Serial Work that resulted from splitting another instance of F18 Serial Work."@en ;
        <http://www.w3.org/2000/01/rdf-schema#domain>
                <http://iflastandards.info/ns/fr/frbr/pressoo/Z1_Serial_Transformation> ;
        <http://www.w3.org/2000/01/rdf-schema#label>
                "initiated"@en ;
        <http://www.w3.org/2000/01/rdf-schema#range>
                <http://iflastandards.info/ns/fr/frbr/frbroo/F18_Serial_Work> ;
        <http://www.w3.org/2000/01/rdf-schema#subPropertyOf>
                <http://www.w3.org/2002/07/owl#topObjectProperty> , <http://iflastandards.info/ns/fr/frbr/frbroo/R16_initiated> .

<http://iflastandards.info/ns/fr/frbr/pressoo/Z1_Serial_Transformation>
        a       <http://www.w3.org/2002/07/owl#Class> ;
        <http://www.w3.org/2000/01/rdf-schema#comment>
                "This class comprises activities that transform instances of F18 Serial Work into new instances of F18 Serial Work.\nAn instance of Z1 Serial Transformation consists of having the idea of starting the publication of one or more than one new serial (this is a particular case of F27 Work Conception), with a distinct intention of thus prolonging, under a new identity, one or more than one earlier serial, the publication of which has ceased, either due directly to the transformation project, or for any other reason.\nThe idea of starting a new serial can be contiguous with the disappearance of a serial, or occur quite some time after that event.\nA transformation can be complete or only partial (e.g., a serial devoted to history of the Middle Ages and Renaissance can cease to be published as such and be continued by a new serial that is devoted to the Middle Ages only). This information element can be reflected through the P2 has type (is type of): E55 Type from the CIDOC CRM model.\nThe most frequent cases of serial transformation are: continuation (in which a serial undergoes a major title change), replacement (in which a new serial supersedes an earlier serial), split (in which one serial is transformed into at least two serials), and merger (in which at least two serials are transformed into one serial).\nThe temporary substitution of a serial with another serial (either pre-existing or created for that purpose) is not regarded as a serial transformation but simply as an episode within the publication process of the serial that temporarily disappeared (see Scope Note for Z4 Temporary Substitution).\nCases of separation and absorption are not regarded as serial transformations either, as they do not involve the combination of the disappearance of a serial and the appearance of another serial, but just either the latter or the former."@en ;
        <http://www.w3.org/2000/01/rdf-schema#label>
                "Serial Transformation"@en ;
        <http://www.w3.org/2000/01/rdf-schema#subClassOf>
                <http://iflastandards.info/ns/fr/frbr/frbroo/F27_Work_Conception> .

<http://iflastandards.info/ns/fr/frbr/pressoo/Y2i_was_initiated_as_continuation_through>
        a       <http://www.w3.org/2002/07/owl#ObjectProperty> , <http://www.w3.org/2002/07/owl#AnnotationProperty> ;
        <http://www.w3.org/2000/01/rdf-schema#domain>
                <http://iflastandards.info/ns/fr/frbr/frbroo/F18_Serial_Work> ;
        <http://www.w3.org/2000/01/rdf-schema#label>
                "was initiated as continuation through"@en ;
        <http://www.w3.org/2000/01/rdf-schema#range>
                <http://iflastandards.info/ns/fr/frbr/pressoo/Z1_Serial_Transformation> ;
        <http://www.w3.org/2000/01/rdf-schema#subPropertyOf>
                <http://www.w3.org/2002/07/owl#topObjectProperty> , <http://iflastandards.info/ns/fr/frbr/frbroo/R16i_was_initiated_by> .

<http://iflastandards.info/ns/fr/frbr/pressoo/Y8i_resulted_from_merger>
        a       <http://www.w3.org/2002/07/owl#ObjectProperty> , <http://www.w3.org/2002/07/owl#AnnotationProperty> ;
        <http://www.w3.org/2000/01/rdf-schema#domain>
                <http://iflastandards.info/ns/fr/frbr/frbroo/F18_Serial_Work> ;
        <http://www.w3.org/2000/01/rdf-schema#label>
                "resulted from merger"@en ;
        <http://www.w3.org/2000/01/rdf-schema#range>
                <http://iflastandards.info/ns/fr/frbr/pressoo/Z1_Serial_Transformation> ;
        <http://www.w3.org/2000/01/rdf-schema#subPropertyOf>
                <http://www.w3.org/2002/07/owl#topObjectProperty> , <http://iflastandards.info/ns/fr/frbr/frbroo/R16i_was_initiated_by> .

<http://iflastandards.info/ns/fr/frbr/pressoo/Y5_split>
        a       <http://www.w3.org/2002/07/owl#ObjectProperty> ;
        <http://www.w3.org/2000/01/rdf-schema#comment>
                "This property associates an instance of Z1 Serial Transformation with an instance of F18 Serial Work that was split in order to create new instances of F18 Serial Work."@en ;
        <http://www.w3.org/2000/01/rdf-schema#domain>
                <http://iflastandards.info/ns/fr/frbr/pressoo/Z1_Serial_Transformation> ;
        <http://www.w3.org/2000/01/rdf-schema#label>
                "split"@en ;
        <http://www.w3.org/2000/01/rdf-schema#range>
                <http://iflastandards.info/ns/fr/frbr/frbroo/F18_Serial_Work> ;
        <http://www.w3.org/2000/01/rdf-schema#subPropertyOf>
                <http://www.w3.org/2002/07/owl#topObjectProperty> .

<http://iflastandards.info/ns/fr/frbr/pressoo/Y7i_was_merged_through>
        a       <http://www.w3.org/2002/07/owl#ObjectProperty> ;
        <http://www.w3.org/2000/01/rdf-schema#domain>
                <http://iflastandards.info/ns/fr/frbr/frbroo/F18_Serial_Work> ;
        <http://www.w3.org/2000/01/rdf-schema#label>
                "was merged through"@en ;
        <http://www.w3.org/2000/01/rdf-schema#range>
                <http://iflastandards.info/ns/fr/frbr/pressoo/Z1_Serial_Transformation> ;
        <http://www.w3.org/2000/01/rdf-schema#subPropertyOf>
                <http://www.w3.org/2002/07/owl#topObjectProperty> .

<http://iflastandards.info/ns/fr/frbr/pressoo/Y6i_resulted_from_split>
        a       <http://www.w3.org/2002/07/owl#ObjectProperty> , <http://www.w3.org/2002/07/owl#AnnotationProperty> ;
        <http://www.w3.org/2000/01/rdf-schema#domain>
                <http://iflastandards.info/ns/fr/frbr/frbroo/F18_Serial_Work> ;
        <http://www.w3.org/2000/01/rdf-schema#label>
                "resulted from split"@en ;
        <http://www.w3.org/2000/01/rdf-schema#range>
                <http://iflastandards.info/ns/fr/frbr/pressoo/Z1_Serial_Transformation> ;
        <http://www.w3.org/2000/01/rdf-schema#subPropertyOf>
                <http://www.w3.org/2002/07/owl#topObjectProperty> , <http://iflastandards.info/ns/fr/frbr/frbroo/R16i_was_initiated_by> .

<http://iflastandards.info/ns/fr/frbr/pressoo/Y4i_was_initiated_as_replacement_through>
        a       <http://www.w3.org/2002/07/owl#ObjectProperty> , <http://www.w3.org/2002/07/owl#AnnotationProperty> ;
        <http://www.w3.org/2000/01/rdf-schema#domain>
                <http://iflastandards.info/ns/fr/frbr/frbroo/F18_Serial_Work> ;
        <http://www.w3.org/2000/01/rdf-schema#label>
                "was initiated as replacement through"@en ;
        <http://www.w3.org/2000/01/rdf-schema#range>
                <http://iflastandards.info/ns/fr/frbr/pressoo/Z1_Serial_Transformation> ;
        <http://www.w3.org/2000/01/rdf-schema#subPropertyOf>
                <http://www.w3.org/2002/07/owl#topObjectProperty> , <http://iflastandards.info/ns/fr/frbr/frbroo/R16i_was_initiated_by> .

<http://iflastandards.info/ns/fr/frbr/pressoo/Y2_initiated_as_continuation>
        a       <http://www.w3.org/2002/07/owl#ObjectProperty> , <http://www.w3.org/2002/07/owl#AnnotationProperty> ;
        <http://www.w3.org/2000/01/rdf-schema#comment>
                "This property associates an instance of Z1 Serial Transformation with an instance of F18 Serial Work that resulted from a ‘major’ title change that affected another instance of F18 Serial Work."@en ;
        <http://www.w3.org/2000/01/rdf-schema#domain>
                <http://iflastandards.info/ns/fr/frbr/pressoo/Z1_Serial_Transformation> ;
        <http://www.w3.org/2000/01/rdf-schema#label>
                "initiated as continuation"@en ;
        <http://www.w3.org/2000/01/rdf-schema#range>
                <http://iflastandards.info/ns/fr/frbr/frbroo/F18_Serial_Work> ;
        <http://www.w3.org/2000/01/rdf-schema#subPropertyOf>
                <http://www.w3.org/2002/07/owl#topObjectProperty> , <http://iflastandards.info/ns/fr/frbr/frbroo/R16_initiated> .

<http://iflastandards.info/ns/fr/frbr/pressoo/Y3_provided_a_replacement_to>
        a       <http://www.w3.org/2002/07/owl#ObjectProperty> ;
        <http://www.w3.org/2000/01/rdf-schema#comment>
                "This property associates an instance of Z1 Serial Transformation with an instance of F18 Serial Work the publication of which had ceased and that was superseded by one or more than one instance of F18 Serial Work."@en ;
        <http://www.w3.org/2000/01/rdf-schema#domain>
                <http://iflastandards.info/ns/fr/frbr/pressoo/Z1_Serial_Transformation> ;
        <http://www.w3.org/2000/01/rdf-schema#label>
                "provided a replacement to"@en ;
        <http://www.w3.org/2000/01/rdf-schema#range>
                <http://iflastandards.info/ns/fr/frbr/frbroo/F18_Serial_Work> ;
        <http://www.w3.org/2000/01/rdf-schema#subPropertyOf>
                <http://www.w3.org/2002/07/owl#topObjectProperty> .

<http://iflastandards.info/ns/fr/frbr/pressoo/Y1i_was_continued_through>
        a       <http://www.w3.org/2002/07/owl#ObjectProperty> ;
        <http://www.w3.org/2000/01/rdf-schema#domain>
                <http://iflastandards.info/ns/fr/frbr/frbroo/F18_Serial_Work> ;
        <http://www.w3.org/2000/01/rdf-schema#label>
                "was continued through"@en ;
        <http://www.w3.org/2000/01/rdf-schema#range>
                <http://iflastandards.info/ns/fr/frbr/pressoo/Z1_Serial_Transformation> ;
        <http://www.w3.org/2000/01/rdf-schema#subPropertyOf>
                <http://www.w3.org/2002/07/owl#topObjectProperty> .

<http://iflastandards.info/ns/fr/frbr/pressoo/Y4_initiated_as_replacement>
        a       <http://www.w3.org/2002/07/owl#ObjectProperty> , <http://www.w3.org/2002/07/owl#AnnotationProperty> ;
        <http://www.w3.org/2000/01/rdf-schema#comment>
                "This property associates an instance of Z1 Serial Transformation with an instance of F18 Serial Work that was created with the distinct intention of being published in lieu of another instance of F18 Serial Work the publication of which had ceased."@en ;
        <http://www.w3.org/2000/01/rdf-schema#domain>
                <http://iflastandards.info/ns/fr/frbr/pressoo/Z1_Serial_Transformation> ;
        <http://www.w3.org/2000/01/rdf-schema#label>
                "initiated as replacement"@en ;
        <http://www.w3.org/2000/01/rdf-schema#range>
                <http://iflastandards.info/ns/fr/frbr/frbroo/F18_Serial_Work> ;
        <http://www.w3.org/2000/01/rdf-schema#subPropertyOf>
                <http://www.w3.org/2002/07/owl#topObjectProperty> , <http://iflastandards.info/ns/fr/frbr/frbroo/R16_initiated> .

<http://iflastandards.info/ns/fr/frbr/frbroo/F18_Serial_Work>
        a       <http://www.w3.org/2002/07/owl#Class> ;
        <http://www.w3.org/2000/01/rdf-schema#subClassOf>
                <http://www.w3.org/2002/07/owl#Thing> .
