<http://purl.org/vocab/frbr/extended#referentiallyComplementsWork>
        a       <http://www.w3.org/2002/07/owl#ObjectProperty> ;
        <http://www.w3.org/2000/01/rdf-schema#isDefinedBy>
                <http://purl.org/vocab/frbr/extended#> ;
        <http://www.w3.org/2000/01/rdf-schema#label>
                "referentially complements work"@en ;
        <http://www.w3.org/2000/01/rdf-schema#range>
                <http://purl.org/vocab/frbr/core#Work> ;
        <http://www.w3.org/2000/01/rdf-schema#subPropertyOf>
                <http://purl.org/vocab/frbr/extended#isReferentiallyRelatedToWork> .

<http://purl.org/vocab/frbr/extended#supplementsWork>
        a       <http://www.w3.org/2002/07/owl#ObjectProperty> ;
        <http://www.w3.org/2000/01/rdf-schema#comment>
                "Referential: index, concordance, teacher's guide, gloss, supplement, appendix, etc.\nAutonomous: supplement, appendix, etc."@en ;
        <http://www.w3.org/2000/01/rdf-schema#isDefinedBy>
                <http://purl.org/vocab/frbr/extended#> ;
        <http://www.w3.org/2000/01/rdf-schema#label>
                "supplements work"@en ;
        <http://www.w3.org/2000/01/rdf-schema#range>
                <http://purl.org/vocab/frbr/core#Work> ;
        <http://www.w3.org/2000/01/rdf-schema#subPropertyOf>
                <http://purl.org/vocab/frbr/extended#isRelatedToWork> .

<http://purl.org/vocab/frbr/extended#isATransformationOfWork>
        a       <http://www.w3.org/2002/07/owl#ObjectProperty> ;
        <http://www.w3.org/2000/01/rdf-schema#comment>
                "Dramatisation, novelisation, versification, screenplay, etc.\nThe subject is not dependent on the object for meaning."@en ;
        <http://www.w3.org/2000/01/rdf-schema#isDefinedBy>
                <http://purl.org/vocab/frbr/extended#> ;
        <http://www.w3.org/2000/01/rdf-schema#label>
                "is a transformation of work"@en ;
        <http://www.w3.org/2000/01/rdf-schema#range>
                <http://purl.org/vocab/frbr/core#Work> ;
        <http://www.w3.org/2000/01/rdf-schema#subPropertyOf>
                <http://purl.org/vocab/frbr/extended#isAutonomouslyRelatedToWork> ;
        <http://www.w3.org/2000/01/rdf-schema#subPropertyOf>
                []  .

<http://purl.org/vocab/frbr/extended#isAnAlternativeManifestationTo>
        a       <http://www.w3.org/2002/07/owl#ObjectProperty> ;
        <http://www.w3.org/2000/01/rdf-schema#comment>
                "Alternate is an Americanism."@en ;
        <http://www.w3.org/2000/01/rdf-schema#isDefinedBy>
                <http://purl.org/vocab/frbr/extended#> ;
        <http://www.w3.org/2000/01/rdf-schema#label>
                "is an alternative manifestation to"@en ;
        <http://www.w3.org/2000/01/rdf-schema#range>
                <http://purl.org/vocab/frbr/core#Endeavour> ;
        <http://www.w3.org/2000/01/rdf-schema#subPropertyOf>
                <http://purl.org/vocab/frbr/extended#isRelatedToManifestation> .

<http://purl.org/vocab/frbr/core#Work>
        a       <http://www.w3.org/2002/07/owl#Class> ;
        <http://www.w3.org/2000/01/rdf-schema#subClassOf>
                <http://www.w3.org/2002/07/owl#Thing> .

<http://purl.org/vocab/frbr/core#Endeavour>
        a       <http://www.w3.org/2002/07/owl#Class> ;
        <http://www.w3.org/2000/01/rdf-schema#subClassOf>
                <http://www.w3.org/2002/07/owl#Thing> .

<http://purl.org/vocab/frbr/extended#isAnImitationOfWork>
        a       <http://www.w3.org/2002/07/owl#ObjectProperty> ;
        <http://www.w3.org/2000/01/rdf-schema#comment>
                "Parody, imitation, travesty, etc.\nThe subject is not dependent on the object for meaning."@en ;
        <http://www.w3.org/2000/01/rdf-schema#isDefinedBy>
                <http://purl.org/vocab/frbr/extended#> ;
        <http://www.w3.org/2000/01/rdf-schema#label>
                "is an imitation of work"@en ;
        <http://www.w3.org/2000/01/rdf-schema#range>
                <http://purl.org/vocab/frbr/core#Work> ;
        <http://www.w3.org/2000/01/rdf-schema#subPropertyOf>
                []  ;
        <http://www.w3.org/2002/07/owl#equivalentProperty>
                []  ;
        <http://www.w3.org/2002/07/owl#inverseOf>
                <http://purl.org/vocab/frbr/extended#isAutonomouslyRelatedToWork> .

<http://purl.org/vocab/frbr/extended#complementsWork>
        a       <http://www.w3.org/2002/07/owl#ObjectProperty> ;
        <http://www.w3.org/2000/01/rdf-schema#comment>
                "Referential: cadenza, libretto, choreography, ending for unfinished work, etc.\nAutonomous: incidental music, musical setting for a text, pendant, etc."@en ;
        <http://www.w3.org/2000/01/rdf-schema#isDefinedBy>
                <http://purl.org/vocab/frbr/extended#> ;
        <http://www.w3.org/2000/01/rdf-schema#label>
                "complements work"@en ;
        <http://www.w3.org/2000/01/rdf-schema#range>
                <http://purl.org/vocab/frbr/core#Work> ;
        <http://www.w3.org/2000/01/rdf-schema#subPropertyOf>
                <http://purl.org/vocab/frbr/extended#isRelatedToWork> .

<http://purl.org/vocab/frbr/core#relatedEndeavour>
        a       <http://www.w3.org/2002/07/owl#ObjectProperty> ;
        <http://www.w3.org/2000/01/rdf-schema#subPropertyOf>
                <http://www.w3.org/2002/07/owl#topObjectProperty> .

<http://purl.org/vocab/frbr/extended#isAReproductionOfManifestation>
        a       <http://www.w3.org/2002/07/owl#ObjectProperty> ;
        <http://www.w3.org/2000/01/rdf-schema#isDefinedBy>
                <http://purl.org/vocab/frbr/extended#> ;
        <http://www.w3.org/2000/01/rdf-schema#label>
                "is a reproduction of manifestation"@en ;
        <http://www.w3.org/2000/01/rdf-schema#range>
                <http://purl.org/vocab/frbr/core#Endeavour> ;
        <http://www.w3.org/2000/01/rdf-schema#subPropertyOf>
                <http://purl.org/vocab/frbr/extended#isRelatedToManifestation> .

<http://purl.org/vocab/frbr/extended#isASuccessorToWork>
        a       <http://www.w3.org/2002/07/owl#ObjectProperty> ;
        <http://www.w3.org/2000/01/rdf-schema#comment>
                "Referential: sequel, etc.\nAutonomous: sequel, succeeding work, etc."@en ;
        <http://www.w3.org/2000/01/rdf-schema#isDefinedBy>
                <http://purl.org/vocab/frbr/extended#> ;
        <http://www.w3.org/2000/01/rdf-schema#label>
                "is a sucessor to work"@en ;
        <http://www.w3.org/2000/01/rdf-schema#range>
                <http://purl.org/vocab/frbr/core#Work> ;
        <http://www.w3.org/2000/01/rdf-schema#subPropertyOf>
                <http://purl.org/vocab/frbr/extended#isRelatedToWork> .
