<https://www.ica.org/standards/RiC/ontology#ContentType>
        a       <http://www.w3.org/2002/07/owl#Class> ;
        <http://www.w3.org/2000/01/rdf-schema#comment>
                "The fundamental form of communication in which a Record is\n            expressed and the human sense through which it is intended to be\n            perceived."@en ;
        <http://www.w3.org/2000/01/rdf-schema#isDefinedBy>
                <https://www.ica.org/standards/RiC/ontology> ;
        <http://www.w3.org/2000/01/rdf-schema#label>
                "Content Type"@en ;
        <http://www.w3.org/2000/01/rdf-schema#subClassOf>
                <https://www.ica.org/standards/RiC/ontology#Type> ;
        <http://www.w3.org/2004/02/skos/core#scopeNote>
                "Should not be confused with Representation Type or Carrier\n            Type of a related Instantiation since the form of communication can be independent of\n            the representation or carrier, for example, a map (Content Type: cartographic image) can\n            be represented as a sketch (Representation Type: graphic) or as a GIS-coded elements\n            (Representation Type: computer)."@en ;
        <https://www.ica.org/standards/RiC/ontology#RiCCMCorrespondingComponent>
                "Corresponds to RiC-A10 (Content Type\n            attribute)"@en .

<https://www.ica.org/standards/RiC/ontology#RecordSet>
        a       <http://www.w3.org/2002/07/owl#Class> ;
        <http://www.w3.org/2000/01/rdf-schema#comment>
                "One or more records that are associated by categorization and/or\n            physical aggregation by the creator or other Agent."@en ;
        <http://www.w3.org/2000/01/rdf-schema#isDefinedBy>
                <https://www.ica.org/standards/RiC/ontology> ;
        <http://www.w3.org/2000/01/rdf-schema#label>
                "Record Set"@en ;
        <http://www.w3.org/2000/01/rdf-schema#subClassOf>
                <https://www.ica.org/standards/RiC/ontology#RecordResource> ;
        <http://www.w3.org/2004/02/skos/core#scopeNote>
                "Record Set is a kind of Record Resource. The Record members in\n            a Record Set may physically reside together, though physical proximity is not essential.\n            In a particular context, an Agent (e.g. administrator, records manager, archivist,\n            end-user, etc.) may select the Record members of a Record Set based on a shared\n            attribute or attributes, or a shared Relation or Relations. The grouping of the Records\n            serves a purpose or purposes specific to the context of the Agent. All Record members of\n            a Record Set may share the attribute of having been accumulated by the same Agent, or\n            all share the same Documentary Form Type and are created over time by the same Activity.\n            A Record Set may represent the act of classifying the Records in accordance with a\n            formal classification scheme that may be based on Activity, subject, organizational\n            structure, or other criteria; an act of archival arrangement (e.g. based on common\n            provenance); or some other selection and grouping that fulfils a particular purpose or\n            purposes (e.g. a classification that reflects or supports the purposes of a researcher).\n            By exception, some Records are brought together based on their not belonging in the\n            context of selection to other designated groups: a ‘Miscellaneous’ series, for example.\n            A Record Set accumulated by an Agent in the course of life or work Activity should be\n            kept in a manner that preserves context and evidential value. Records Sets may also\n            contain other Records Sets. Both a Record Set and a Record may simultaneously be a\n            member of more than one Record Set, and over the course of its existence, a Record Set\n            or Record may be a member of an indeterminate number of Record Sets in an indeterminate\n            number of contexts. Record Sets and Records contained within a Record Set may be ordered\n            into a sequence based on a common property or relation, or common properties or\n            relations (e.g. alphabetical by Agent or related Place name; chronological order by an\n            allocated Date); or some other criterion (e.g. an imposed order by\n            relevance)."@en ;
        <https://www.ica.org/standards/RiC/ontology#RiCCMCorrespondingComponent>
                "Corresponds to RiC-E03 (Record Set\n            entity)"@en .

<https://www.ica.org/standards/RiC/ontology#accrual>
        a       <http://www.w3.org/2002/07/owl#DatatypeProperty> ;
        <http://www.w3.org/2000/01/rdf-schema#comment>
                "Information on the anticipated accession(s) to the Record\n            Set."@en ;
        <http://www.w3.org/2000/01/rdf-schema#domain>
                <https://www.ica.org/standards/RiC/ontology#RecordSet> ;
        <http://www.w3.org/2000/01/rdf-schema#isDefinedBy>
                <https://www.ica.org/standards/RiC/ontology> ;
        <http://www.w3.org/2000/01/rdf-schema#label>
                "accrual"@en ;
        <http://www.w3.org/2000/01/rdf-schema#range>
                <http://www.w3.org/2000/01/rdf-schema#Literal> ;
        <http://www.w3.org/2000/01/rdf-schema#subPropertyOf>
                <http://www.w3.org/2002/07/owl#topDataProperty> ;
        <http://www.w3.org/2004/02/skos/core#scopeNote>
                "See also accrualStatus"@en ;
        <https://www.ica.org/standards/RiC/ontology#RiCCMCorrespondingComponent>
                "corresponds to RiC-A01 (Accrual\n            attribute)"@en .

<https://www.ica.org/standards/RiC/ontology#accrualStatus>
        a       <http://www.w3.org/2002/07/owl#DatatypeProperty> ;
        <http://www.w3.org/2000/01/rdf-schema#comment>
                "Information on the status of an Accrual"@en ;
        <http://www.w3.org/2000/01/rdf-schema#domain>
                <https://www.ica.org/standards/RiC/ontology#RecordSet> ;
        <http://www.w3.org/2000/01/rdf-schema#isDefinedBy>
                <https://www.ica.org/standards/RiC/ontology> ;
        <http://www.w3.org/2000/01/rdf-schema#label>
                "accrual status"@en ;
        <http://www.w3.org/2000/01/rdf-schema#range>
                <http://www.w3.org/2000/01/rdf-schema#Literal> ;
        <http://www.w3.org/2000/01/rdf-schema#subPropertyOf>
                <http://www.w3.org/2002/07/owl#topDataProperty> ;
        <http://www.w3.org/2004/02/skos/core#changeNote>
                []  ;
        <http://www.w3.org/2004/02/skos/core#scopeNote>
                "A text statement or single words such as “Closed” to indicate\n            that no additional Record Resource will (or is anticipated to) be added to the Record\n            Set; “Open” to indicate that additional records or record sets will (or are expected to)\n            be added to the Record Set; or “Unknown” to indicate that this information is not\n            available, for example. See also accrual"@en ;
        <https://www.ica.org/standards/RiC/ontology#RiCCMCorrespondingComponent>
                "corresponds to RiC-A01 (Accrual\n            attribute)"@en .

<https://www.ica.org/standards/RiC/ontology#hasOrHadAllMembersWithContentType>
        a       <http://www.w3.org/2002/07/owl#ObjectProperty> ;
        <http://www.w3.org/2000/01/rdf-schema#comment>
                "Connects a Record Set and a Content Type that categorizes all\n            the Records or Record Parts that are or were included in the Record Set."@en ;
        <http://www.w3.org/2000/01/rdf-schema#domain>
                <https://www.ica.org/standards/RiC/ontology#RecordSet> ;
        <http://www.w3.org/2000/01/rdf-schema#isDefinedBy>
                <https://www.ica.org/standards/RiC/ontology> ;
        <http://www.w3.org/2000/01/rdf-schema#label>
                "has of had all members with content type"@en ;
        <http://www.w3.org/2000/01/rdf-schema#range>
                <https://www.ica.org/standards/RiC/ontology#ContentType> ;
        <http://www.w3.org/2000/01/rdf-schema#subPropertyOf>
                <https://www.ica.org/standards/RiC/ontology#hasOrHadAllMembersWithCategory> ;
        <http://www.w3.org/2000/01/rdf-schema#subPropertyOf>
                []  ;
        <http://www.w3.org/2002/07/owl#equivalentProperty>
                []  ;
        <http://www.w3.org/2004/02/skos/core#changeNote>
                []  .
