<http://iflastandards.info/ns/fr/frbr/frbroo/F27_Work_Conception>
        a       <http://www.w3.org/2002/07/owl#Class> ;
        <http://www.w3.org/2000/01/rdf-schema#comment>
                "This class comprises beginnings of evolutions of works.\nAn instance of F27 Work Conception marks the initiation of the creation of a work. The work, as an intellectual construction, evolves from this point on, until the last known expression of it. The instance of E39 Actor with which a work is associated through the chain of properties F1 Work R16i was initiated by F27 Work Conception P14 carried out by E39 Actor corresponds to the notion of the “creator” of the work. In the case of commissioned works, it is not the commissioning that is regarded as the work conception, but the acceptance of the commission.\nThis event does not always correlate with the date assigned in common library practice to the work, which is usually a later event (such as the date of completion of the first clean draft).\nIn addition, F27 Work Conception can serve to document the circumstances that surrounded the appearance of the original idea for a work, when these are known.\n\n"@en ;
        <http://www.w3.org/2000/01/rdf-schema#label>
                "Work Conception"@en ;
        <http://www.w3.org/2000/01/rdf-schema#subClassOf>
                <http://www.cidoc-crm.org/cidoc-crm/E65_Creation> .

<http://iflastandards.info/ns/fr/frbr/frbroo/F1_Work>
        a       <http://www.w3.org/2002/07/owl#Class> ;
        <http://www.w3.org/2000/01/rdf-schema#comment>
                "This class comprises distinct concepts or combinations of concepts identified in artistic and intellectual expressions, such as poems, stories or musical compositions. Such concepts may appear in the course of the coherent evolution of an original idea into one or more expressions that are dominated by the original idea. A Work may be elaborated by one or more Actors simultaneously or over time. The substance of Work is ideas. A Work may have members that are works in their own right.\nA Work can be either individual or complex. If it is individual its concept is completely realised in a single F22 Self-Contained Expression. If it is complex its concept is embedded in an F15 Complex Work. An F15 Complex Work consists of alternative members that are either F15 Complex Works themselves or F14 Individual Works. \nA Work is the product of an intellectual process of one or more persons, yet only indirect evidence about it is at our hands. This can be contextual information such as the existence of an order for a work, reflections of the creators themselves that are documented somewhere, and finally the expressions of the work created. As ideas normally take shape during discussion, elaboration and implementation, it is not reasonable to assume that a work starts with a complete concept. In some cases, it can be very difficult or impossible to define the whole of the concept of a work at a particular time. The objective evidence for such a notion can only be based on a stage of expressions at a given time. In this sense, the sets of ideas that constitute  particular self-contained expressions may be regarded as a kind of “snap-shot” of a work.\nA Work may include the concept of aggregating expressions of other works into a new expression. For instance, an anthology of poems is regarded as a work in its own right that makes use of expressions of the individual poems that have been selected and ordered as part of an intellectual process. This does not make the contents of the aggregated expressions part of this work, but only parts of the resulting expression.\n"@en ;
        <http://www.w3.org/2000/01/rdf-schema#label>
                "Work"@en ;
        <http://www.w3.org/2000/01/rdf-schema#subClassOf>
                <http://www.cidoc-crm.org/cidoc-crm/E89_Propositional_Object> .

<http://iflastandards.info/ns/fr/frbr/frbroo/R16i_was_initiated_by>
        a       <http://www.w3.org/2002/07/owl#ObjectProperty> ;
        <http://www.w3.org/2000/01/rdf-schema#comment>
                "\n"@en ;
        <http://www.w3.org/2000/01/rdf-schema#domain>
                <http://iflastandards.info/ns/fr/frbr/frbroo/F1_Work> ;
        <http://www.w3.org/2000/01/rdf-schema#label>
                "was initiated by"@en ;
        <http://www.w3.org/2000/01/rdf-schema#range>
                <http://iflastandards.info/ns/fr/frbr/frbroo/F27_Work_Conception> ;
        <http://www.w3.org/2000/01/rdf-schema#subPropertyOf>
                <http://www.w3.org/2002/07/owl#topObjectProperty> .

<http://iflastandards.info/ns/fr/frbr/frbroo/R16_initiated>
        a       <http://www.w3.org/2002/07/owl#ObjectProperty> ;
        <http://www.w3.org/2000/01/rdf-schema#comment>
                "This property associates the first conception of a work and the work itself that ensued from a given initial idea.\nIt marks the origin of the causality chain that results in a work’s coming into existence.\n"@en ;
        <http://www.w3.org/2000/01/rdf-schema#domain>
                <http://iflastandards.info/ns/fr/frbr/frbroo/F27_Work_Conception> ;
        <http://www.w3.org/2000/01/rdf-schema#label>
                "initiated"@en ;
        <http://www.w3.org/2000/01/rdf-schema#range>
                <http://iflastandards.info/ns/fr/frbr/frbroo/F1_Work> ;
        <http://www.w3.org/2000/01/rdf-schema#subPropertyOf>
                <http://www.w3.org/2002/07/owl#topObjectProperty> .
