<http://www.loc.gov/mods/rdf/v1#titleUniform>
        a       <http://www.w3.org/2002/07/owl#ObjectProperty> ;
        <http://www.w3.org/2000/01/rdf-schema#comment>
                "A title which has been distinguished as a uniform title. (This corresponds to a MODS XML titleInfo with 'type=uniform' attribute.) There should be no more than one uniform title.  Represented as a MADS Title, or, if there is a primary name, it is represented as a MADS NameTitle.  " ;
        <http://www.w3.org/2000/01/rdf-schema#domain>
                <http://www.loc.gov/mods/rdf/v1#ModsResource> ;
        <http://www.w3.org/2000/01/rdf-schema#label>
                "Title - Uniform" ;
        <http://www.w3.org/2000/01/rdf-schema#range>
                <http://www.loc.gov/mads/rdf/v1#Title> ;
        <http://www.w3.org/2000/01/rdf-schema#subPropertyOf>
                <http://www.loc.gov/mods/rdf/v1#title> .

<http://www.loc.gov/mods/rdf/v1#title>
        a       <http://www.w3.org/2002/07/owl#ObjectProperty> ;
        <http://www.w3.org/2000/01/rdf-schema#comment>
                "A title for the resource. Represented as a MADS Title." ;
        <http://www.w3.org/2000/01/rdf-schema#domain>
                <http://www.loc.gov/mods/rdf/v1#ModsResource> ;
        <http://www.w3.org/2000/01/rdf-schema#label>
                "Title" ;
        <http://www.w3.org/2000/01/rdf-schema#range>
                <http://www.loc.gov/mads/rdf/v1#Title> .

<http://www.loc.gov/mods/rdf/v1#subjectTitle>
        a       <http://www.w3.org/2002/07/owl#ObjectProperty> ;
        <http://www.w3.org/2000/01/rdf-schema#comment>
                "A subject of the resource which is a title, expressed in terms of a MADS Title." ;
        <http://www.w3.org/2000/01/rdf-schema#domain>
                <http://www.loc.gov/mods/rdf/v1#ModsResource> ;
        <http://www.w3.org/2000/01/rdf-schema#label>
                "Subject - Title" ;
        <http://www.w3.org/2000/01/rdf-schema#range>
                <http://www.loc.gov/mads/rdf/v1#Title> ;
        <http://www.w3.org/2000/01/rdf-schema#subPropertyOf>
                <http://www.loc.gov/mods/rdf/v1#subject> .

<http://www.loc.gov/mods/rdf/v1#ModsResource>
        a       <http://www.w3.org/2002/07/owl#Class> ;
        <http://www.w3.org/2000/01/rdf-schema#comment>
                "\nThe resource which is the subject of this description.\n  " ;
        <http://www.w3.org/2000/01/rdf-schema#label>
                "MODS - A  MODS Resource" ;
        <http://www.w3.org/2002/07/owl#equivalentClass>
                <http://id.loc.gov/vocabulary/resourceTypes/Res> .

<http://www.loc.gov/mods/rdf/v1#titlePrincipal>
        a       <http://www.w3.org/2002/07/owl#ObjectProperty> ;
        <http://www.w3.org/2000/01/rdf-schema#comment>
                "A title which has been distinguished as the principal  title. (This corresponds to a MODS XML titleInfo with  no type attribute.) There should be no more than one principal title. Represented as a MADS Title." ;
        <http://www.w3.org/2000/01/rdf-schema#domain>
                <http://www.loc.gov/mods/rdf/v1#ModsResource> ;
        <http://www.w3.org/2000/01/rdf-schema#label>
                "Title - Principal" ;
        <http://www.w3.org/2000/01/rdf-schema#range>
                <http://www.loc.gov/mads/rdf/v1#Title> ;
        <http://www.w3.org/2000/01/rdf-schema#subPropertyOf>
                <http://www.loc.gov/mods/rdf/v1#title> .
