<http://www.loc.gov/mods/rdf/v1#relatedSeries>
        a       <http://www.w3.org/2002/07/owl#ObjectProperty> ;
        <http://www.w3.org/2000/01/rdf-schema#comment>
                "Relates the described resource to a another MODS resource which is a series of which the described resource is a part." ;
        <http://www.w3.org/2000/01/rdf-schema#domain>
                <http://www.loc.gov/mods/rdf/v1#ModsResource> ;
        <http://www.w3.org/2000/01/rdf-schema#label>
                "Related item - Series" ;
        <http://www.w3.org/2000/01/rdf-schema#range>
                <http://www.loc.gov/mods/rdf/v1#ModsResource> ;
        <http://www.w3.org/2000/01/rdf-schema#subPropertyOf>
                <http://www.loc.gov/mods/rdf/v1#relatedItem> .

<http://www.loc.gov/mods/rdf/v1#relatedReference>
        a       <http://www.w3.org/2002/07/owl#ObjectProperty> ;
        <http://www.w3.org/2000/01/rdf-schema#comment>
                "Relates the described MODS resource to another MODS resource which the described resource references." ;
        <http://www.w3.org/2000/01/rdf-schema#domain>
                <http://www.loc.gov/mods/rdf/v1#ModsResource> ;
        <http://www.w3.org/2000/01/rdf-schema#label>
                "Related item - Reference" ;
        <http://www.w3.org/2000/01/rdf-schema#range>
                <http://www.loc.gov/mods/rdf/v1#ModsResource> ;
        <http://www.w3.org/2000/01/rdf-schema#subPropertyOf>
                <http://www.loc.gov/mods/rdf/v1#relatedItem> .

<http://www.loc.gov/mods/rdf/v1#cartographics>
        a       <http://www.w3.org/2002/07/owl#ObjectProperty> ;
        <http://www.w3.org/2000/01/rdf-schema#comment>
                "A geographic entity expressed in cartographic terms." ;
        <http://www.w3.org/2000/01/rdf-schema#domain>
                <http://www.loc.gov/mods/rdf/v1#ModsResource> ;
        <http://www.w3.org/2000/01/rdf-schema#label>
                "Cartographics " ;
        <http://www.w3.org/2000/01/rdf-schema#range>
                <http://www.loc.gov/mods/rdf/v1#Cartographics> .

<http://www.loc.gov/mods/rdf/v1#ModsResource>
        a       <http://www.w3.org/2002/07/owl#Class> ;
        <http://www.w3.org/2000/01/rdf-schema#comment>
                "\nThe resource which is the subject of this description.\n  " ;
        <http://www.w3.org/2000/01/rdf-schema#label>
                "MODS - A  MODS Resource" ;
        <http://www.w3.org/2002/07/owl#equivalentClass>
                <http://id.loc.gov/vocabulary/resourceTypes/Res> .

<http://www.loc.gov/mods/rdf/v1#relatedPreceding>
        a       <http://www.w3.org/2002/07/owl#ObjectProperty> ;
        <http://www.w3.org/2000/01/rdf-schema#comment>
                "Relates the described MODS resource to a MODS resource which preceded the described resource." ;
        <http://www.w3.org/2000/01/rdf-schema#domain>
                <http://www.loc.gov/mods/rdf/v1#ModsResource> ;
        <http://www.w3.org/2000/01/rdf-schema#label>
                "Related item - Preceding" ;
        <http://www.w3.org/2000/01/rdf-schema#range>
                <http://www.loc.gov/mods/rdf/v1#ModsResource> ;
        <http://www.w3.org/2000/01/rdf-schema#subPropertyOf>
                <http://www.loc.gov/mods/rdf/v1#relatedItem> .

<http://www.loc.gov/mods/rdf/v1#edition>
        a       <http://www.w3.org/2002/07/owl#DatatypeProperty> ;
        <http://www.w3.org/2000/01/rdf-schema#comment>
                "Version of the resource." ;
        <http://www.w3.org/2000/01/rdf-schema#domain>
                <http://www.loc.gov/mods/rdf/v1#ModsResource> ;
        <http://www.w3.org/2000/01/rdf-schema#label>
                "Edition" ;
        <http://www.w3.org/2000/01/rdf-schema#range>
                <http://www.w3.org/2001/XMLSchema#string> .

<http://www.loc.gov/mods/rdf/v1#relatedVersion>
        a       <http://www.w3.org/2002/07/owl#ObjectProperty> ;
        <http://www.w3.org/2000/01/rdf-schema#comment>
                "Relates the described MODS resource to another MODS resource which is a different version of the described resource." ;
        <http://www.w3.org/2000/01/rdf-schema#domain>
                <http://www.loc.gov/mods/rdf/v1#ModsResource> ;
        <http://www.w3.org/2000/01/rdf-schema#label>
                "Related Item - Other Version" ;
        <http://www.w3.org/2000/01/rdf-schema#range>
                <http://www.loc.gov/mods/rdf/v1#ModsResource> ;
        <http://www.w3.org/2000/01/rdf-schema#subPropertyOf>
                <http://www.loc.gov/mods/rdf/v1#relatedItem> .

<http://www.loc.gov/mods/rdf/v1#note>
        a       <http://www.w3.org/2002/07/owl#DatatypeProperty> ;
        <http://www.w3.org/2000/01/rdf-schema#comment>
                "Textual information about the resource. This property is used when no type is specified. (In contrast to hasTypedNote, whose object is an aggregator that includes both the type and note.)" ;
        <http://www.w3.org/2000/01/rdf-schema#domain>
                <http://www.loc.gov/mods/rdf/v1#ModsResource> ;
        <http://www.w3.org/2000/01/rdf-schema#label>
                "Note" ;
        <http://www.w3.org/2000/01/rdf-schema#range>
                <http://www.w3.org/2001/XMLSchema#string> .

<http://www.loc.gov/mods/rdf/v1#relatedOriginal>
        a       <http://www.w3.org/2002/07/owl#ObjectProperty> ;
        <http://www.w3.org/2000/01/rdf-schema#comment>
                "Relates the described MODS resource to another MODS resource which is an original of the described resource." ;
        <http://www.w3.org/2000/01/rdf-schema#domain>
                <http://www.loc.gov/mods/rdf/v1#ModsResource> ;
        <http://www.w3.org/2000/01/rdf-schema#label>
                "Related item - Original" ;
        <http://www.w3.org/2000/01/rdf-schema#range>
                <http://www.loc.gov/mods/rdf/v1#ModsResource> ;
        <http://www.w3.org/2000/01/rdf-schema#subPropertyOf>
                <http://www.loc.gov/mods/rdf/v1#relatedItem> .

<http://www.loc.gov/mods/rdf/v1#relatedHost>
        a       <http://www.w3.org/2002/07/owl#ObjectProperty> ;
        <http://www.w3.org/2000/01/rdf-schema#comment>
                "Relates the described MODS resource to another MODS resource which is a host of the described resource." ;
        <http://www.w3.org/2000/01/rdf-schema#domain>
                <http://www.loc.gov/mods/rdf/v1#ModsResource> ;
        <http://www.w3.org/2000/01/rdf-schema#label>
                "Related item - Host" ;
        <http://www.w3.org/2000/01/rdf-schema#range>
                <http://www.loc.gov/mods/rdf/v1#ModsResource> ;
        <http://www.w3.org/2000/01/rdf-schema#subPropertyOf>
                <http://www.loc.gov/mods/rdf/v1#relatedItem> .

<http://www.loc.gov/mods/rdf/v1#relatedInstantiation>
        a       <http://www.w3.org/2002/07/owl#ObjectProperty> ;
        <http://www.w3.org/2000/01/rdf-schema#comment>
                "Relates the described resource to a another MODS resource with different origination information." ;
        <http://www.w3.org/2000/01/rdf-schema#domain>
                <http://www.loc.gov/mods/rdf/v1#ModsResource> ;
        <http://www.w3.org/2000/01/rdf-schema#label>
                "Related item - Instantiation" ;
        <http://www.w3.org/2000/01/rdf-schema#range>
                <http://www.loc.gov/mods/rdf/v1#ModsResource> ;
        <http://www.w3.org/2000/01/rdf-schema#subPropertyOf>
                <http://www.loc.gov/mods/rdf/v1#relatedItem> .

<http://www.loc.gov/mods/rdf/v1#issuance>
        a       <http://www.w3.org/2002/07/owl#DatatypeProperty> ;
        <http://www.w3.org/2000/01/rdf-schema#comment>
                "Describes the issuance of the resource." ;
        <http://www.w3.org/2000/01/rdf-schema#domain>
                <http://www.loc.gov/mods/rdf/v1#ModsResource> ;
        <http://www.w3.org/2000/01/rdf-schema#label>
                "Issuance" ;
        <http://www.w3.org/2000/01/rdf-schema#range>
                <http://www.w3.org/2001/XMLSchema#string> .

<http://www.loc.gov/mods/rdf/v1#physicalExtent>
        a       <http://www.w3.org/2002/07/owl#DatatypeProperty> ;
        <http://www.w3.org/2000/01/rdf-schema#comment>
                "a statement of the number and specific material of the units of the resource that express physical extent." ;
        <http://www.w3.org/2000/01/rdf-schema#domain>
                <http://www.loc.gov/mods/rdf/v1#ModsResource> ;
        <http://www.w3.org/2000/01/rdf-schema#label>
                "Physical Extent" ;
        <http://www.w3.org/2000/01/rdf-schema#range>
                <http://www.w3.org/2001/XMLSchema#string> .

<http://www.loc.gov/mods/rdf/v1#frequency>
        a       <http://www.w3.org/2002/07/owl#DatatypeProperty> ;
        <http://www.w3.org/2000/01/rdf-schema#comment>
                "publication frequency" ;
        <http://www.w3.org/2000/01/rdf-schema#domain>
                <http://www.loc.gov/mods/rdf/v1#ModsResource> ;
        <http://www.w3.org/2000/01/rdf-schema#label>
                "Frequency" ;
        <http://www.w3.org/2000/01/rdf-schema#range>
                <http://www.w3.org/2001/XMLSchema#string> .

<http://www.loc.gov/mods/rdf/v1#relatedSucceeding>
        a       <http://www.w3.org/2002/07/owl#ObjectProperty> ;
        <http://www.w3.org/2000/01/rdf-schema#comment>
                "Relates the described resource to a another MODS resource which suceeded it." ;
        <http://www.w3.org/2000/01/rdf-schema#domain>
                <http://www.loc.gov/mods/rdf/v1#ModsResource> ;
        <http://www.w3.org/2000/01/rdf-schema#label>
                "Related item - Suceeding" ;
        <http://www.w3.org/2000/01/rdf-schema#range>
                <http://www.loc.gov/mods/rdf/v1#ModsResource> ;
        <http://www.w3.org/2000/01/rdf-schema#subPropertyOf>
                <http://www.loc.gov/mods/rdf/v1#relatedItem> .

<http://www.loc.gov/mods/rdf/v1#relatedReferencedBy>
        a       <http://www.w3.org/2002/07/owl#ObjectProperty> ;
        <http://www.w3.org/2000/01/rdf-schema#comment>
                "Relates the described MODS resource to another MODS resource which references the described resource." , "" ;
        <http://www.w3.org/2000/01/rdf-schema#domain>
                <http://www.loc.gov/mods/rdf/v1#ModsResource> ;
        <http://www.w3.org/2000/01/rdf-schema#label>
                "Related item - Referenced By" ;
        <http://www.w3.org/2000/01/rdf-schema#range>
                <http://www.loc.gov/mods/rdf/v1#ModsResource> ;
        <http://www.w3.org/2000/01/rdf-schema#subPropertyOf>
                <http://www.loc.gov/mods/rdf/v1#relatedItem> .

<http://www.loc.gov/mods/rdf/v1#statementOfResponsibility>
        a       <http://www.w3.org/2002/07/owl#DatatypeProperty> ;
        <http://www.w3.org/2000/01/rdf-schema#comment>
                "A note, when the note type is \"statement of responsibility\"" ;
        <http://www.w3.org/2000/01/rdf-schema#domain>
                <http://www.loc.gov/mods/rdf/v1#ModsResource> ;
        <http://www.w3.org/2000/01/rdf-schema#label>
                "Statement of Responsibility" ;
        <http://www.w3.org/2000/01/rdf-schema#range>
                <http://www.w3.org/2001/XMLSchema#string> .

<http://www.loc.gov/mods/rdf/v1#relatedReview>
        a       <http://www.w3.org/2002/07/owl#ObjectProperty> ;
        <http://www.w3.org/2000/01/rdf-schema#comment>
                "Relates the described MODS resource to another MODS resource which is review of the described resource." ;
        <http://www.w3.org/2000/01/rdf-schema#domain>
                <http://www.loc.gov/mods/rdf/v1#ModsResource> ;
        <http://www.w3.org/2000/01/rdf-schema#label>
                "Related item - Review" ;
        <http://www.w3.org/2000/01/rdf-schema#range>
                <http://www.loc.gov/mods/rdf/v1#ModsResource> ;
        <http://www.w3.org/2000/01/rdf-schema#subPropertyOf>
                <http://www.loc.gov/mods/rdf/v1#relatedItem> .

<http://www.loc.gov/mods/rdf/v1#relatedConstituent>
        a       <http://www.w3.org/2002/07/owl#ObjectProperty> ;
        <http://www.w3.org/2000/01/rdf-schema#comment>
                "Relates the described MODS resource to another MODS resource which is a constituent of the described resource. " ;
        <http://www.w3.org/2000/01/rdf-schema#domain>
                <http://www.loc.gov/mods/rdf/v1#ModsResource> ;
        <http://www.w3.org/2000/01/rdf-schema#label>
                "Related item - Constituent" ;
        <http://www.w3.org/2000/01/rdf-schema#range>
                <http://www.loc.gov/mods/rdf/v1#ModsResource> ;
        <http://www.w3.org/2000/01/rdf-schema#subPropertyOf>
                <http://www.loc.gov/mods/rdf/v1#relatedItem> .

<http://www.loc.gov/mods/rdf/v1#Cartographics>
        a       <http://www.w3.org/2002/07/owl#Class> ;
        <http://www.w3.org/2000/01/rdf-schema#comment>
                "Aggregates cartographic properties." ;
        <http://www.w3.org/2000/01/rdf-schema#label>
                "MODS - Cartographic Information" ;
        <http://www.w3.org/2000/01/rdf-schema#subClassOf>
                <http://www.w3.org/2002/07/owl#Thing> .

<http://www.loc.gov/mods/rdf/v1#relatedFormat>
        a       <http://www.w3.org/2002/07/owl#ObjectProperty> ;
        <http://www.w3.org/2000/01/rdf-schema#comment>
                "Relates the described MODS resource to a similar MODS resource of a different format." ;
        <http://www.w3.org/2000/01/rdf-schema#domain>
                <http://www.loc.gov/mods/rdf/v1#ModsResource> ;
        <http://www.w3.org/2000/01/rdf-schema#label>
                "Related item - Other Format" ;
        <http://www.w3.org/2000/01/rdf-schema#range>
                <http://www.loc.gov/mods/rdf/v1#ModsResource> ;
        <http://www.w3.org/2000/01/rdf-schema#subPropertyOf>
                <http://www.loc.gov/mods/rdf/v1#relatedItem> .

<http://www.loc.gov/mods/rdf/v1#mediaType>
        a       <http://www.w3.org/2002/07/owl#DatatypeProperty> ;
        <http://www.w3.org/2000/01/rdf-schema#comment>
                "An Internet Media (MIME) type e.g. text/html. " ;
        <http://www.w3.org/2000/01/rdf-schema#domain>
                <http://www.loc.gov/mods/rdf/v1#ModsResource> ;
        <http://www.w3.org/2000/01/rdf-schema#label>
                "Media Type" ;
        <http://www.w3.org/2000/01/rdf-schema#range>
                <http://www.w3.org/2001/XMLSchema#string> .

<http://www.loc.gov/mods/rdf/v1#relatedItem>
        a       <http://www.w3.org/2002/07/owl#ObjectProperty> ;
        <http://www.w3.org/2000/01/rdf-schema#comment>
                "Relates the described MODS resource to another, related MODS resource." ;
        <http://www.w3.org/2000/01/rdf-schema#domain>
                <http://www.loc.gov/mods/rdf/v1#ModsResource> ;
        <http://www.w3.org/2000/01/rdf-schema#label>
                "Related Item" ;
        <http://www.w3.org/2000/01/rdf-schema#range>
                <http://www.loc.gov/mods/rdf/v1#ModsResource> .
