<http://www.loc.gov/mods/rdf/v1#locationCopySublocation>
        a       <http://www.w3.org/2002/07/owl#DatatypeProperty> ;
        <http://www.w3.org/2000/01/rdf-schema#comment>
                "Department, division, or section of an institution holding a copy of the resource." ;
        <http://www.w3.org/2000/01/rdf-schema#domain>
                <http://www.loc.gov/mods/rdf/v1#LocationCopy> ;
        <http://www.w3.org/2000/01/rdf-schema#label>
                "Location - Copy -- Sublocation" ;
        <http://www.w3.org/2000/01/rdf-schema#range>
                <http://www.w3.org/2001/XMLSchema#string> .

<http://www.loc.gov/mods/rdf/v1#LocationCopy>
        a       <http://www.w3.org/2002/07/owl#Class> ;
        <http://www.w3.org/2000/01/rdf-schema#comment>
                " An aggregator for copy properties." ;
        <http://www.w3.org/2000/01/rdf-schema#label>
                "MODS - Location - Copy" .

<http://www.loc.gov/mods/rdf/v1#locationCopyForm>
        a       <http://www.w3.org/2002/07/owl#DatatypeProperty> ;
        <http://www.w3.org/2000/01/rdf-schema#comment>
                "The form of a particular copy may be indicated when the general description refers to multiple forms and there is different detailed holdings information associated with different forms." ;
        <http://www.w3.org/2000/01/rdf-schema#domain>
                <http://www.loc.gov/mods/rdf/v1#LocationCopy> ;
        <http://www.w3.org/2000/01/rdf-schema#label>
                "Location - Copy -- Form" ;
        <http://www.w3.org/2000/01/rdf-schema#range>
                <http://www.w3.org/2001/XMLSchema#string> .

<http://www.loc.gov/mods/rdf/v1#locationCopyElectronicLocator>
        a       <http://www.w3.org/2002/07/owl#DatatypeProperty> ;
        <http://www.w3.org/2000/01/rdf-schema#comment>
                "URI of the copy of the resource." ;
        <http://www.w3.org/2000/01/rdf-schema#domain>
                <http://www.loc.gov/mods/rdf/v1#LocationCopy> ;
        <http://www.w3.org/2000/01/rdf-schema#label>
                "Location - Copy -- Electronic Locator" ;
        <http://www.w3.org/2000/01/rdf-schema#range>
                <http://www.w3.org/2001/XMLSchema#string> .

<http://www.loc.gov/mods/rdf/v1#locationCopyEnumerationAndChronology>
        a       <http://www.w3.org/2002/07/owl#DatatypeProperty> ;
        <http://www.w3.org/2000/01/rdf-schema#comment>
                "A summary holdings statement for the copy. A string with information including volume or issue, date of publication or date of issue of a component of a multi-part resource, distinguishing it from other components of the same resource. " ;
        <http://www.w3.org/2000/01/rdf-schema#domain>
                <http://www.loc.gov/mods/rdf/v1#LocationCopy> ;
        <http://www.w3.org/2000/01/rdf-schema#label>
                "Location - Copy  - Enumeration And Chronology" ;
        <http://www.w3.org/2000/01/rdf-schema#range>
                <http://www.w3.org/2001/XMLSchema#string> .

<http://www.loc.gov/mods/rdf/v1#locationCopyNote>
        a       <http://www.w3.org/2002/07/owl#DatatypeProperty> ;
        <http://www.w3.org/2000/01/rdf-schema#comment>
                "A note pertaining to a specific copy." ;
        <http://www.w3.org/2000/01/rdf-schema#domain>
                <http://www.loc.gov/mods/rdf/v1#LocationCopy> ;
        <http://www.w3.org/2000/01/rdf-schema#label>
                "Location - Copy -- Note" ;
        <http://www.w3.org/2000/01/rdf-schema#range>
                <http://www.w3.org/2001/XMLSchema#string> .

<http://www.loc.gov/mods/rdf/v1#locationCopyEnumerationAndChronologySupplement>
        a       <http://www.w3.org/2002/07/owl#DatatypeProperty> ;
        <http://www.w3.org/2000/01/rdf-schema#comment>
                "One of three levels  of enumerationAndChronology:'supplement'" ;
        <http://www.w3.org/2000/01/rdf-schema#domain>
                <http://www.loc.gov/mods/rdf/v1#LocationCopy> ;
        <http://www.w3.org/2000/01/rdf-schema#label>
                "Location - Copy  - Enumeration And Chronology -- Supplement" ;
        <http://www.w3.org/2000/01/rdf-schema#range>
                <http://www.w3.org/2001/XMLSchema#string> ;
        <http://www.w3.org/2000/01/rdf-schema#subPropertyOf>
                <http://www.loc.gov/mods/rdf/v1#locationCopyEnumerationAndChronology> .

<http://www.loc.gov/mods/rdf/v1#locationCopyEnumerationAndChronologyBasic>
        a       <http://www.w3.org/2002/07/owl#DatatypeProperty> ;
        <http://www.w3.org/2000/01/rdf-schema#comment>
                "One of three levels of enumerationAndChronology: 'basic'" ;
        <http://www.w3.org/2000/01/rdf-schema#domain>
                <http://www.loc.gov/mods/rdf/v1#LocationCopy> ;
        <http://www.w3.org/2000/01/rdf-schema#label>
                "Location - Copy  - Enumeration And Chronology -- Basic" ;
        <http://www.w3.org/2000/01/rdf-schema#range>
                <http://www.w3.org/2001/XMLSchema#string> ;
        <http://www.w3.org/2000/01/rdf-schema#subPropertyOf>
                <http://www.loc.gov/mods/rdf/v1#locationCopyEnumerationAndChronology> .

<http://www.loc.gov/mods/rdf/v1#locationCopyShelfLocator>
        a       <http://www.w3.org/2002/07/owl#DatatypeProperty> ;
        <http://www.w3.org/2000/01/rdf-schema#comment>
                "Shelfmark or other shelving designation that indicates the location identifier for a copy." ;
        <http://www.w3.org/2000/01/rdf-schema#domain>
                <http://www.loc.gov/mods/rdf/v1#LocationCopy> ;
        <http://www.w3.org/2000/01/rdf-schema#label>
                "Location - Copy -- Shelf Locator" ;
        <http://www.w3.org/2000/01/rdf-schema#range>
                <http://www.w3.org/2001/XMLSchema#string> .

<http://www.loc.gov/mods/rdf/v1#locationCopyEnumerationAndChronologyIndex>
        a       <http://www.w3.org/2002/07/owl#DatatypeProperty> ;
        <http://www.w3.org/2000/01/rdf-schema#comment>
                "One of three levels of enumerationAndChronology:'index'" ;
        <http://www.w3.org/2000/01/rdf-schema#domain>
                <http://www.loc.gov/mods/rdf/v1#LocationCopy> ;
        <http://www.w3.org/2000/01/rdf-schema#label>
                "Location - Copy  - Enumeration And Chronology -- Index" ;
        <http://www.w3.org/2000/01/rdf-schema#range>
                <http://www.w3.org/2001/XMLSchema#string> ;
        <http://www.w3.org/2000/01/rdf-schema#subPropertyOf>
                <http://www.loc.gov/mods/rdf/v1#locationCopyEnumerationAndChronology> .
