<?xml version="1.0" encoding="UTF-8"?>
<rdf:RDF
   xmlns:dc="http://purl.org/dc/elements/1.1/"
   xmlns:owl="http://www.w3.org/2002/07/owl#"
   xmlns:rdf="http://www.w3.org/1999/02/22-rdf-syntax-ns#"
   xmlns:rdfs="http://www.w3.org/2000/01/rdf-schema#"
   xmlns:terms="http://purl.org/dc/terms/"
>
  <rdf:Description rdf:about="http://purl.org/emmedi/oaentry/hasFormerWork">
    <rdfs:domain rdf:resource="http://www.w3.org/ns/prov#Influence"/>
    <rdfs:subPropertyOf rdf:resource="http://www.w3.org/ns/prov#entity"/>
    <rdfs:label xml:lang="en">has former work</rdfs:label>
    <rdf:type rdf:resource="http://www.w3.org/2002/07/owl#ObjectProperty"/>
    <rdfs:comment xml:lang="en">A property relating an entity describing the influence an entity, e.g. a work of art, may have on a derivative one, e.g. a copy or a fake of the former work.</rdfs:comment>
  </rdf:Description>
  <rdf:Description rdf:about="http://purl.org/emmedi/oaentry/CopyOrDerivation">
    <rdfs:subClassOf rdf:resource="http://www.w3.org/ns/prov#EntityInfluence"/>
    <rdfs:label xml:lang="en">Copy or Derivation</rdfs:label>
    <rdf:type rdf:resource="http://www.w3.org/2002/07/owl#Class"/>
    <rdfs:comment xml:lang="en">A class representing an uncertain influence an entity may have on another one, i.e. being a copy of or a derivation from a former created work of art.</rdfs:comment>
  </rdf:Description>
  <rdf:Description rdf:about="http://purl.org/emmedi/oaentry/cosmographer">
    <rdf:type rdf:resource="http://purl.org/emmedi/oaentry/ArtisticRole"/>
    <rdfs:label xml:lang="en">cosmographer</rdfs:label>
    <rdf:type rdf:resource="http://www.w3.org/2002/07/owl#NamedIndividual"/>
    <rdfs:comment xml:lang="en">The role of the person who studies and maps main features of the universe.</rdfs:comment>
  </rdf:Description>
  <rdf:Description rdf:about="http://purl.org/emmedi/oaentry/cataloguer">
    <rdf:type rdf:resource="http://www.w3.org/2002/07/owl#NamedIndividual"/>
    <rdfs:label xml:lang="en">cataloguer</rdfs:label>
    <rdfs:comment xml:lang="en">The role held by the responsible agent with respect to the metadata entry describing a cultural heritage object.</rdfs:comment>
    <rdf:type rdf:resource="http://purl.org/emmedi/oaentry/CataloguingRole"/>
  </rdf:Description>
  <rdf:Description rdf:about="http://purl.org/emmedi/oaentry/designer">
    <rdf:type rdf:resource="http://purl.org/emmedi/oaentry/ArtisticRole"/>
    <rdfs:label xml:lang="en">designer</rdfs:label>
    <rdf:type rdf:resource="http://www.w3.org/2002/07/owl#NamedIndividual"/>
    <rdfs:comment xml:lang="en">The role of a persone who devises and executes designs, as for works of art, clothes, machines, etc.</rdfs:comment>
  </rdf:Description>
  <rdf:Description rdf:about="http://purl.org/emmedi/oaentry/lutist">
    <rdf:type rdf:resource="http://www.w3.org/2002/07/owl#NamedIndividual"/>
    <rdf:type rdf:resource="http://purl.org/emmedi/oaentry/ArtisticRole"/>
    <rdfs:comment xml:lang="en">The role of a person who makes lutes.</rdfs:comment>
    <rdfs:label xml:lang="en">lutist</rdfs:label>
  </rdf:Description>
  <rdf:Description rdf:about="http://purl.org/emmedi/oaentry/date-attribution">
    <rdf:type rdf:resource="http://purl.org/emmedi/hico/InterpretationType"/>
    <rdf:type rdf:resource="http://www.w3.org/2002/07/owl#NamedIndividual"/>
  </rdf:Description>
  <rdf:Description rdf:nodeID="N1a37e603017e4c7d9c2a25746b1a980f">
    <rdf:first rdf:resource="http://purl.org/spar/fabio/Work"/>
    <rdf:rest rdf:resource="http://www.w3.org/1999/02/22-rdf-syntax-ns#nil"/>
  </rdf:Description>
  <rdf:Description rdf:about="http://purl.org/emmedi/oaentry/Model">
    <rdfs:subClassOf rdf:resource="http://purl.org/emmedi/oaentry/PartialModel"/>
    <rdfs:comment xml:lang="en">A class representing the influence a work of art may have on another one when the former is a model of the latter one.</rdfs:comment>
    <rdf:type rdf:resource="http://www.w3.org/2002/07/owl#Class"/>
    <rdfs:label xml:lang="en">Model</rdfs:label>
  </rdf:Description>
  <rdf:Description rdf:about="http://purl.org/emmedi/oaentry/engineer">
    <rdfs:label xml:lang="en">engineer</rdfs:label>
    <rdfs:comment xml:lang="en">The role of a person who designs and builds machines, equipments, roads, buldings or other things.</rdfs:comment>
    <rdf:type rdf:resource="http://www.w3.org/2002/07/owl#NamedIndividual"/>
    <rdf:type rdf:resource="http://purl.org/emmedi/oaentry/ArtisticRole"/>
  </rdf:Description>
  <rdf:Description rdf:about="http://purl.org/emmedi/oaentry/decorator">
    <rdfs:comment xml:lang="en">The role of a person who paints the inside/outside of buildings and other works.</rdfs:comment>
    <rdf:type rdf:resource="http://www.w3.org/2002/07/owl#NamedIndividual"/>
    <rdfs:label xml:lang="en">decorator</rdfs:label>
    <rdf:type rdf:resource="http://purl.org/emmedi/oaentry/ArtisticRole"/>
  </rdf:Description>
  <rdf:Description rdf:about="http://purl.org/emmedi/oaentry/musician">
    <rdf:type rdf:resource="http://www.w3.org/2002/07/owl#NamedIndividual"/>
    <rdfs:label xml:lang="en">musician</rdfs:label>
    <rdf:type rdf:resource="http://purl.org/emmedi/oaentry/ArtisticRole"/>
    <rdfs:comment xml:lang="en">The role of a person who plays a musical instrument.</rdfs:comment>
  </rdf:Description>
  <rdf:Description rdf:about="http://purl.org/emmedi/oaentry/Underdrawing">
    <rdfs:subClassOf rdf:resource="http://www.w3.org/ns/prov#EntityInfluence"/>
    <rdf:type rdf:resource="http://www.w3.org/2002/07/owl#Class"/>
    <rdfs:comment xml:lang="en">A class representing the influence a work of art may have on another one when the former is an underdrawing of the latter one.</rdfs:comment>
    <rdfs:label xml:lang="en">Underdrawing</rdfs:label>
  </rdf:Description>
  <rdf:Description rdf:about="http://purl.org/emmedi/oaentry/influence-between-works-attribution">
    <rdf:type rdf:resource="http://purl.org/emmedi/hico/InterpretationType"/>
    <rdf:type rdf:resource="http://www.w3.org/2002/07/owl#NamedIndividual"/>
  </rdf:Description>
  <rdf:Description rdf:about="http://purl.org/emmedi/oaentry/cataloguing-supervisor">
    <rdf:type rdf:resource="http://www.w3.org/2002/07/owl#NamedIndividual"/>
    <rdf:type rdf:resource="http://purl.org/emmedi/oaentry/CataloguingRole"/>
    <rdfs:label xml:lang="en">cataloguing supervisor</rdfs:label>
    <rdfs:comment xml:lang="en">The role held by the responsible agent supervising the filling of a metadata entry describing a cultural heritage object.</rdfs:comment>
  </rdf:Description>
  <rdf:Description rdf:about="http://purl.org/emmedi/oaentry/Copy">
    <rdfs:label xml:lang="en">Copy</rdfs:label>
    <rdf:type rdf:resource="http://www.w3.org/2002/07/owl#Class"/>
    <rdfs:subClassOf rdf:resource="http://purl.org/emmedi/oaentry/PartialCopy"/>
    <rdfs:comment xml:lang="en">A class representing the influence a work of art may have on another one when the latter is considered a copy of the former one.</rdfs:comment>
  </rdf:Description>
  <rdf:Description rdf:about="http://purl.org/emmedi/oaentry/architect">
    <rdf:type rdf:resource="http://purl.org/emmedi/oaentry/ArtisticRole"/>
    <rdfs:comment xml:lang="en">The role connected to the person responsible for designing buildings and making certain that they are built correctly.</rdfs:comment>
    <rdf:type rdf:resource="http://www.w3.org/2002/07/owl#NamedIndividual"/>
    <rdfs:label xml:lang="en">architect</rdfs:label>
  </rdf:Description>
  <rdf:Description rdf:about="http://purl.org/emmedi/oaentry/painter">
    <rdfs:label xml:lang="en">painter</rdfs:label>
    <rdf:type rdf:resource="http://purl.org/emmedi/oaentry/ArtisticRole"/>
    <rdf:type rdf:resource="http://www.w3.org/2002/07/owl#NamedIndividual"/>
    <rdfs:comment xml:lang="en">The role of a person who paints pictures.</rdfs:comment>
  </rdf:Description>
  <rdf:Description rdf:about="http://purl.org/emmedi/oaentry">
    <owl:imports rdf:resource="http://www.w3.org/ns/prov-o#"/>
    <dc:creator>Marilena Daquino</dc:creator>
    <owl:imports rdf:resource="http://purl.org/spar/pro/"/>
    <rdfs:comment xml:lang="en">OAEntry Ontology aims to represent fundamental entities related to works of art description, according to the ICCD Italian content strandard &lt;a href="http://www.iccd.beniculturali.it/index.php?it/253/beni-storici-e-artistici"&gt;Scheda OA&lt;/a&gt;, i.e. OA Entry. OAEntry Ontology enriches CIDOC-CRM descriptive capabilities by defining several possible relations between works of art, by also extending PROV Ontology.&lt;a href="http://purl.org/emmedi/hico"&gt;HiCO - Historical Context Ontology&lt;/a&gt; is imported in order to fully describe the workflow required by a cataloguer, or an art criticist, for defining a questionable information (e.g. relations between works of art) as an entity born out from a subjective interpretation/attribution.&lt;a href="http://purl.org/spar/fabio"&gt;FaBiO - FRBR-Aligned Ontology&lt;/a&gt;, &lt;a href="http://purl.org/spar/pro"&gt;PRO - Publishing Roles Ontology&lt;/a&gt; and &lt;a href="http://purl.org/spar/cito"&gt;CiTO - Citation Typing Ontology&lt;/a&gt; from &lt;a href="http://www.sparontologies.net/"&gt;SPAR Ontologies&lt;/a&gt; are also imported, to model respectively works of art as FRBR entities, to describe roles involved in the work of art lifecycle, and to define cataloguers' citations when an source of an attribution is provided. Moreover, also OA Entry Ontology extends with several new individuals the class pro:Role, defining new roles involved in the artwork lifecycle and in the cataloguing of cultural objects. Moreover, also the HiCo Ontology is extended, by means of new individuals of the class hico:InterpretationType in order to specify the sort of interpretation needed to state something questionable.</rdfs:comment>
    <owl:imports rdf:resource="http://purl.org/spar/cito/"/>
    <rdfs:label xml:lang="en">OA Entry Ontology</rdfs:label>
    <rdf:type rdf:resource="http://www.w3.org/2002/07/owl#Ontology"/>
    <terms:date xml:lang="en">2/9/2015</terms:date>
    <owl:imports rdf:resource="http://purl.org/emmedi/hico"/>
    <terms:contributor>Silvio Peroni</terms:contributor>
    <owl:imports rdf:resource="http://purl.org/spar/fabio/"/>
  </rdf:Description>
  <rdf:Description rdf:about="http://purl.org/emmedi/oaentry/ReplicaWithVariants">
    <rdfs:label xml:lang="en">Replica with variants</rdfs:label>
    <rdfs:subClassOf rdf:resource="http://purl.org/emmedi/oaentry/Replica"/>
    <rdfs:comment xml:lang="en">A class representing the influence a work of art may have on another one when the latter is considered a replica, woth some variants, of the former one.</rdfs:comment>
    <rdf:type rdf:resource="http://www.w3.org/2002/07/owl#Class"/>
  </rdf:Description>
  <rdf:Description rdf:about="http://purl.org/emmedi/oaentry/isFormerWorkOf">
    <rdfs:comment xml:lang="en">A property relating an entity, e.g. a work of art, to the entity describing its influence on a derivative work, e.g. a copy or a fake of the former work.</rdfs:comment>
    <rdfs:range rdf:resource="http://www.w3.org/ns/prov#Influence"/>
    <rdf:type rdf:resource="http://www.w3.org/2002/07/owl#ObjectProperty"/>
    <rdfs:label xml:lang="en">is former work of</rdfs:label>
    <owl:inverseOf rdf:resource="http://purl.org/emmedi/oaentry/hasFormerWork"/>
  </rdf:Description>
  <rdf:Description rdf:about="http://purl.org/emmedi/oaentry/isConceivedByMeansOf">
    <rdfs:range rdf:resource="http://www.w3.org/ns/prov#Influence"/>
    <rdfs:comment xml:lang="en">A property relating an entity, e.g. a work of art, to the entity which describes specific features related to the entity conception, e.g. being a copy or a fake of another work.</rdfs:comment>
    <rdfs:subPropertyOf rdf:resource="http://www.w3.org/ns/prov#qualifiedInfluence"/>
    <rdf:type rdf:resource="http://www.w3.org/2002/07/owl#ObjectProperty"/>
    <rdfs:label xml:lang="en">is conceived by means of</rdfs:label>
  </rdf:Description>
  <rdf:Description rdf:about="http://purl.org/emmedi/oaentry/smelter">
    <rdf:type rdf:resource="http://purl.org/emmedi/oaentry/ArtisticRole"/>
    <rdfs:label xml:lang="en">smelter</rdfs:label>
    <rdf:type rdf:resource="http://www.w3.org/2002/07/owl#NamedIndividual"/>
    <rdfs:comment xml:lang="en">The role of a person who works where ores are smelted.</rdfs:comment>
  </rdf:Description>
  <rdf:Description rdf:about="http://purl.org/emmedi/oaentry/CataloguingRole">
    <rdfs:label xml:lang="en">Cataloguing role</rdfs:label>
    <rdfs:comment xml:lang="en">A role an agent may have with respect to a cultural heritage object cataloguing
.</rdfs:comment>
    <rdf:type rdf:resource="http://www.w3.org/2002/07/owl#Class"/>
    <rdfs:subClassOf rdf:resource="http://purl.org/spar/pro/Role"/>
  </rdf:Description>
  <rdf:Description rdf:nodeID="Na3533143607448dc8622af7915ed0b28">
    <rdf:rest rdf:nodeID="N66089d7ac2424207a31527bfe6aa8499"/>
    <rdf:first rdf:resource="http://purl.org/spar/fabio/Item"/>
  </rdf:Description>
  <rdf:Description rdf:about="http://purl.org/emmedi/oaentry/Cartoon">
    <rdfs:subClassOf rdf:resource="http://purl.org/emmedi/oaentry/PartialCartoon"/>
    <rdfs:comment xml:lang="en">A class representing the influence a work of art may have on another one when the former is a cartoon of another work.</rdfs:comment>
    <rdfs:label xml:lang="en">Cartoon</rdfs:label>
    <rdf:type rdf:resource="http://www.w3.org/2002/07/owl#Class"/>
  </rdf:Description>
  <rdf:Description rdf:about="http://purl.org/emmedi/oaentry/sculptor">
    <rdfs:comment xml:lang="en">The role of a person who creates sculptures.</rdfs:comment>
    <rdf:type rdf:resource="http://www.w3.org/2002/07/owl#NamedIndividual"/>
    <rdf:type rdf:resource="http://purl.org/emmedi/oaentry/ArtisticRole"/>
    <rdfs:label xml:lang="en">sculptor</rdfs:label>
  </rdf:Description>
  <rdf:Description rdf:about="http://purl.org/emmedi/oaentry/cabinetmaker">
    <rdf:type rdf:resource="http://www.w3.org/2002/07/owl#NamedIndividual"/>
    <rdf:type rdf:resource="http://purl.org/emmedi/oaentry/ArtisticRole"/>
    <rdfs:comment xml:lang="en">The role of a person who makes or repair good quality furniture.</rdfs:comment>
    <rdfs:label xml:lang="en">cabinetmaker (or woodworker)</rdfs:label>
  </rdf:Description>
  <rdf:Description rdf:about="http://purl.org/emmedi/oaentry/ceramist">
    <rdfs:comment xml:lang="en">The role held by a person who makes pottery.</rdfs:comment>
    <rdfs:label xml:lang="en">ceramist</rdfs:label>
    <rdf:type rdf:resource="http://www.w3.org/2002/07/owl#NamedIndividual"/>
    <rdf:type rdf:resource="http://purl.org/emmedi/oaentry/ArtisticRole"/>
  </rdf:Description>
  <rdf:Description rdf:about="http://purl.org/emmedi/oaentry/Derivation">
    <rdfs:comment xml:lang="en">A class representing the influence a work of art may have on another one when the latter is considered a derivation of the former one.</rdfs:comment>
    <rdfs:subClassOf rdf:resource="http://purl.org/emmedi/oaentry/PartialDerivation"/>
    <rdf:type rdf:resource="http://www.w3.org/2002/07/owl#Class"/>
    <rdfs:label xml:lang="en">Derivation</rdfs:label>
  </rdf:Description>
  <rdf:Description rdf:about="http://purl.org/emmedi/oaentry/competent-institution">
    <rdfs:label xml:lang="en">competent institution</rdfs:label>
    <rdfs:comment xml:lang="en">The role held by the competent corporate body when a catalogued cultural heritage object falls under its jurisdiction.</rdfs:comment>
    <rdf:type rdf:resource="http://www.w3.org/2002/07/owl#NamedIndividual"/>
    <rdf:type rdf:resource="http://purl.org/emmedi/oaentry/CataloguingRole"/>
  </rdf:Description>
  <rdf:Description rdf:about="http://purl.org/emmedi/oaentry/draughtsman">
    <rdf:type rdf:resource="http://purl.org/emmedi/oaentry/ArtisticRole"/>
    <rdfs:comment xml:lang="en">The role of a person who details drawings of works of art.</rdfs:comment>
    <rdf:type rdf:resource="http://www.w3.org/2002/07/owl#NamedIndividual"/>
    <rdfs:label xml:lang="en">draughtsman</rdfs:label>
  </rdf:Description>
  <rdf:Description rdf:about="http://purl.org/emmedi/oaentry/CopyWithVariants">
    <rdfs:label xml:lang="en">Copy with variants</rdfs:label>
    <rdfs:comment xml:lang="en">A class representing the influence a work of art may have on another one when the latter is considered a copy, with some variants, of the former one.</rdfs:comment>
    <rdfs:subClassOf rdf:resource="http://purl.org/emmedi/oaentry/Copy"/>
    <rdf:type rdf:resource="http://www.w3.org/2002/07/owl#Class"/>
  </rdf:Description>
  <rdf:Description rdf:about="http://purl.org/emmedi/oaentry/gem-cutter">
    <rdf:type rdf:resource="http://www.w3.org/2002/07/owl#NamedIndividual"/>
    <rdfs:label xml:lang="en">gem-cutter</rdfs:label>
    <rdfs:comment xml:lang="en">The role of a person who carves gems for creating jewellery.</rdfs:comment>
    <rdf:type rdf:resource="http://purl.org/emmedi/oaentry/ArtisticRole"/>
  </rdf:Description>
  <rdf:Description rdf:about="http://purl.org/emmedi/oaentry/PartialScaleModel">
    <rdfs:comment xml:lang="en">A class representing the influence a work of art may have on another one when one is a partial scale model of the other one.</rdfs:comment>
    <rdfs:subClassOf rdf:resource="http://www.w3.org/ns/prov#EntityInfluence"/>
    <rdfs:label xml:lang="en">Partial scale model</rdfs:label>
    <rdf:type rdf:resource="http://www.w3.org/2002/07/owl#Class"/>
  </rdf:Description>
  <rdf:Description rdf:about="http://purl.org/emmedi/oaentry/PartialCopy">
    <rdfs:subClassOf rdf:resource="http://purl.org/emmedi/oaentry/CopyOrDerivation"/>
    <rdf:type rdf:resource="http://www.w3.org/2002/07/owl#Class"/>
    <rdfs:label xml:lang="en">Partial copy</rdfs:label>
    <rdfs:comment xml:lang="en">A class representing the influence a work of art may have on another one when the latter is considered a partial copy of the former one.</rdfs:comment>
  </rdf:Description>
  <rdf:Description rdf:about="http://purl.org/emmedi/oaentry/PartialSinopia">
    <rdfs:label xml:lang="en">Partial sinopia</rdfs:label>
    <rdfs:comment xml:lang="en">A class representing the influence a work of art may have on another one when the former is a partial sinopia of the latter one.</rdfs:comment>
    <rdfs:subClassOf rdf:resource="http://www.w3.org/ns/prov#EntityInfluence"/>
    <rdf:type rdf:resource="http://www.w3.org/2002/07/owl#Class"/>
  </rdf:Description>
  <rdf:Description rdf:about="http://purl.org/emmedi/oaentry/Replica">
    <rdfs:label xml:lang="en">Replica</rdfs:label>
    <rdfs:subClassOf rdf:resource="http://purl.org/emmedi/oaentry/PartialReplica"/>
    <rdfs:comment xml:lang="en">A class representing the influence a work of art may have on another one when the latter is considered a replica of the former one.</rdfs:comment>
    <rdf:type rdf:resource="http://www.w3.org/2002/07/owl#Class"/>
  </rdf:Description>
  <rdf:Description rdf:about="http://purl.org/emmedi/oaentry/art-dealer">
    <rdfs:comment xml:lang="en">The role of a person or a corporate body selling works of art.</rdfs:comment>
    <rdfs:label xml:lang="en">art dealer</rdfs:label>
    <rdf:type rdf:resource="http://purl.org/emmedi/oaentry/ArtisticRole"/>
    <rdf:type rdf:resource="http://www.w3.org/2002/07/owl#NamedIndividual"/>
  </rdf:Description>
  <rdf:Description rdf:nodeID="N66089d7ac2424207a31527bfe6aa8499">
    <rdf:first rdf:resource="http://purl.org/spar/fabio/Manifestation"/>
    <rdf:rest rdf:nodeID="N1a37e603017e4c7d9c2a25746b1a980f"/>
  </rdf:Description>
  <rdf:Description rdf:about="http://purl.org/emmedi/oaentry/OAEntry">
    <rdfs:comment xml:lang="en">It is a document containing metadata about a work of art, i.e. a fabio:ArtisticWork, and about the concrete object portrayed by the work of art.</rdfs:comment>
    <rdf:type rdf:resource="http://www.w3.org/2002/07/owl#Class"/>
    <rdfs:label xml:lang="en">OA Entry </rdfs:label>
    <rdfs:subClassOf rdf:resource="http://purl.org/spar/fabio/EntityMetadata"/>
  </rdf:Description>
  <rdf:Description rdf:about="http://purl.org/emmedi/oaentry/PartialCopyWithVariants">
    <rdfs:comment xml:lang="en">A class representing the influence a work of art may have on another one when the latter is considered a partial copy, with some variants, of the former one.</rdfs:comment>
    <rdfs:subClassOf rdf:resource="http://purl.org/emmedi/oaentry/PartialCopy"/>
    <rdfs:label xml:lang="en">Partial copy with variants</rdfs:label>
    <rdf:type rdf:resource="http://www.w3.org/2002/07/owl#Class"/>
  </rdf:Description>
  <rdf:Description rdf:about="http://purl.org/emmedi/oaentry/Mold">
    <rdfs:label xml:lang="en">Mold</rdfs:label>
    <rdfs:comment xml:lang="en">A class representing the influence a work of art may have on another one when the former is a mold of the latter one.</rdfs:comment>
    <rdfs:subClassOf rdf:resource="http://purl.org/emmedi/oaentry/PartialMold"/>
    <rdf:type rdf:resource="http://www.w3.org/2002/07/owl#Class"/>
  </rdf:Description>
  <rdf:Description rdf:about="http://purl.org/emmedi/oaentry/antiquarian">
    <rdf:type rdf:resource="http://purl.org/emmedi/oaentry/ArtisticRole"/>
    <rdfs:comment xml:lang="en">The role connected to the trade, collection, or study of rare objects.
</rdfs:comment>
    <rdf:type rdf:resource="http://www.w3.org/2002/07/owl#NamedIndividual"/>
    <rdfs:label xml:lang="en">antiquarian</rdfs:label>
  </rdf:Description>
  <rdf:Description rdf:about="http://purl.org/emmedi/oaentry/engraver">
    <rdfs:comment xml:lang="en">The role of a person who etches into metal.</rdfs:comment>
    <rdf:type rdf:resource="http://purl.org/emmedi/oaentry/ArtisticRole"/>
    <rdf:type rdf:resource="http://www.w3.org/2002/07/owl#NamedIndividual"/>
    <rdfs:label xml:lang="en">engraver</rdfs:label>
  </rdf:Description>
  <rdf:Description rdf:about="http://purl.org/emmedi/oaentry/hasConceived">
    <rdfs:comment xml:lang="en">A property relating an entity which describes the influence an entity may have on another one, e.g. a work of art is copied or counterfait by another one, to the resulting entity, e.g. the copy or the fake.</rdfs:comment>
    <rdf:type rdf:resource="http://www.w3.org/2002/07/owl#ObjectProperty"/>
    <rdfs:label xml:lang="en">has conceived</rdfs:label>
    <owl:inverseOf rdf:resource="http://purl.org/emmedi/oaentry/isConceivedByMeansOf"/>
    <rdfs:domain rdf:resource="http://www.w3.org/ns/prov#Influence"/>
  </rdf:Description>
  <rdf:Description rdf:about="http://purl.org/emmedi/oaentry/PartialDerivation">
    <rdf:type rdf:resource="http://www.w3.org/2002/07/owl#Class"/>
    <rdfs:subClassOf rdf:resource="http://purl.org/emmedi/oaentry/CopyOrDerivation"/>
    <rdfs:comment xml:lang="en">A class representing the influence a work of art may have on another one when the latter is considered a partial derivation of the former one.</rdfs:comment>
    <rdfs:label xml:lang="en">Partial derivation</rdfs:label>
  </rdf:Description>
  <rdf:Description rdf:about="http://purl.org/emmedi/oaentry/cartographer">
    <rdf:type rdf:resource="http://www.w3.org/2002/07/owl#NamedIndividual"/>
    <rdfs:label xml:lang="en">cartographer</rdfs:label>
    <rdfs:comment xml:lang="en">The role of a person who makes or draws maps.</rdfs:comment>
    <rdf:type rdf:resource="http://purl.org/emmedi/oaentry/ArtisticRole"/>
  </rdf:Description>
  <rdf:Description rdf:about="http://purl.org/emmedi/oaentry/miniaturist">
    <rdf:type rdf:resource="http://www.w3.org/2002/07/owl#NamedIndividual"/>
    <rdfs:comment xml:lang="en">The role of a person who makes small paintings.</rdfs:comment>
    <rdf:type rdf:resource="http://purl.org/emmedi/oaentry/ArtisticRole"/>
    <rdfs:label xml:lang="en">miniaturist</rdfs:label>
  </rdf:Description>
  <rdf:Description rdf:about="http://purl.org/emmedi/oaentry/Drawing">
    <rdfs:subClassOf rdf:resource="http://www.w3.org/ns/prov#EntityInfluence"/>
    <rdf:type rdf:resource="http://www.w3.org/2002/07/owl#Class"/>
    <rdfs:comment xml:lang="en">A class representing the influence a work of art may have on another one when the former is a drawing of the latter one.</rdfs:comment>
    <rdfs:label xml:lang="en">Drawing</rdfs:label>
  </rdf:Description>
  <rdf:Description rdf:about="http://purl.org/emmedi/oaentry/PartialModel">
    <rdfs:subClassOf rdf:resource="http://www.w3.org/ns/prov#EntityInfluence"/>
    <rdf:type rdf:resource="http://www.w3.org/2002/07/owl#Class"/>
    <rdfs:comment xml:lang="en">A class representing the influence a work of art may have on another one when the former is a partial model of the latter one.</rdfs:comment>
    <rdfs:label xml:lang="en">Partial model</rdfs:label>
  </rdf:Description>
  <rdf:Description rdf:about="http://purl.org/emmedi/oaentry/Sinopia">
    <rdfs:label xml:lang="en">Sinopia</rdfs:label>
    <rdfs:subClassOf rdf:resource="http://purl.org/emmedi/oaentry/PartialSinopia"/>
    <rdf:type rdf:resource="http://www.w3.org/2002/07/owl#Class"/>
    <rdfs:comment xml:lang="en">A class representing the influence a work of art may have on another one when the former is a sinopia of the latter one.</rdfs:comment>
  </rdf:Description>
  <rdf:Description rdf:about="http://purl.org/emmedi/oaentry/printer">
    <rdfs:comment xml:lang="en">The role of a person who prints books.</rdfs:comment>
    <rdfs:label xml:lang="en">printer</rdfs:label>
    <rdf:type rdf:resource="http://www.w3.org/2002/07/owl#NamedIndividual"/>
    <rdf:type rdf:resource="http://purl.org/emmedi/oaentry/ArtisticRole"/>
  </rdf:Description>
  <rdf:Description rdf:about="http://purl.org/emmedi/oaentry/title-attribution">
    <rdf:type rdf:resource="http://www.w3.org/2002/07/owl#NamedIndividual"/>
    <rdf:type rdf:resource="http://purl.org/emmedi/hico/InterpretationType"/>
  </rdf:Description>
  <rdf:Description rdf:about="http://purl.org/emmedi/oaentry/artist">
    <rdf:type rdf:resource="http://purl.org/emmedi/oaentry/ArtisticRole"/>
    <rdfs:label xml:lang="en">artist</rdfs:label>
    <rdfs:comment xml:lang="en">The role of a person responsible for the conception and the execution of a work of art.</rdfs:comment>
    <rdf:type rdf:resource="http://www.w3.org/2002/07/owl#NamedIndividual"/>
  </rdf:Description>
  <rdf:Description rdf:about="http://purl.org/emmedi/oaentry/medalist">
    <rdf:type rdf:resource="http://www.w3.org/2002/07/owl#NamedIndividual"/>
    <rdf:type rdf:resource="http://purl.org/emmedi/oaentry/ArtisticRole"/>
    <rdfs:label xml:lang="en">medalist</rdfs:label>
    <rdfs:comment xml:lang="en">The role of a person who designs medals.</rdfs:comment>
  </rdf:Description>
  <rdf:Description rdf:about="http://purl.org/emmedi/oaentry/Sketch">
    <rdfs:subClassOf rdf:resource="http://www.w3.org/ns/prov#EntityInfluence"/>
    <rdf:type rdf:resource="http://www.w3.org/2002/07/owl#Class"/>
    <rdfs:label xml:lang="en">Sketch</rdfs:label>
    <rdfs:comment xml:lang="en">A class representing the influence a work of art may have on another one when the former is a sketch of the latter one.</rdfs:comment>
  </rdf:Description>
  <rdf:Description rdf:nodeID="N6c53906619c141018ff3d02f0f951fe5">
    <rdf:first rdf:resource="http://purl.org/spar/fabio/Expression"/>
    <rdf:rest rdf:nodeID="Na3533143607448dc8622af7915ed0b28"/>
  </rdf:Description>
  <rdf:Description rdf:about="http://purl.org/emmedi/oaentry/scenographer">
    <rdf:type rdf:resource="http://www.w3.org/2002/07/owl#NamedIndividual"/>
    <rdfs:label xml:lang="en">scenographer</rdfs:label>
    <rdf:type rdf:resource="http://purl.org/emmedi/oaentry/ArtisticRole"/>
    <rdfs:comment xml:lang="en">The role of a person who designs visual elements of a performance.</rdfs:comment>
  </rdf:Description>
  <rdf:Description rdf:about="http://www.essepuntato.it/2014/03/fentry/FEntry">
    <rdf:type rdf:resource="http://www.w3.org/2002/07/owl#Class"/>
    <rdfs:label xml:lang="en">F Entry</rdfs:label>
    <rdfs:subClassOf rdf:resource="http://purl.org/spar/fabio/EntityMetadata"/>
    <rdfs:comment xml:lang="en">It is a document containing metadata about a photograph and about the concrete object portrayed by the photograph.</rdfs:comment>
  </rdf:Description>
  <rdf:Description rdf:about="http://purl.org/emmedi/oaentry/ArtisticRole">
    <rdf:type rdf:resource="http://www.w3.org/2002/07/owl#Class"/>
    <rdfs:comment xml:lang="en">A role an agent may have with respect to a work of art conception or execution.</rdfs:comment>
    <rdfs:label xml:lang="en">Artistic role</rdfs:label>
    <rdfs:subClassOf rdf:resource="http://purl.org/spar/pro/Role"/>
  </rdf:Description>
  <rdf:Description rdf:about="http://purl.org/emmedi/oaentry/PartialMatrix">
    <rdf:type rdf:resource="http://www.w3.org/2002/07/owl#Class"/>
    <rdfs:comment xml:lang="en">A class representing the influence a work of art may have on another one when the former is a partial matrix of the latter one.</rdfs:comment>
    <rdfs:label xml:lang="en">Partial matrix</rdfs:label>
    <rdfs:subClassOf rdf:resource="http://www.w3.org/ns/prov#EntityInfluence"/>
  </rdf:Description>
  <rdf:Description rdf:about="http://purl.org/emmedi/oaentry/ScaleModel">
    <rdf:type rdf:resource="http://www.w3.org/2002/07/owl#Class"/>
    <rdfs:label xml:lang="en">Scale model</rdfs:label>
    <rdfs:comment xml:lang="en">A class representing the influence a work of art may have on another one, when one is a scale model of the other one.</rdfs:comment>
    <rdfs:subClassOf rdf:resource="http://purl.org/emmedi/oaentry/PartialScaleModel"/>
  </rdf:Description>
  <rdf:Description rdf:about="http://purl.org/emmedi/oaentry/glassmaker">
    <rdf:type rdf:resource="http://www.w3.org/2002/07/owl#NamedIndividual"/>
    <rdfs:label xml:lang="en">glassmaker</rdfs:label>
    <rdf:type rdf:resource="http://purl.org/emmedi/oaentry/ArtisticRole"/>
    <rdfs:comment xml:lang="en">The role of a person who makes glass or glass objects.</rdfs:comment>
  </rdf:Description>
  <rdf:Description rdf:about="http://purl.org/emmedi/oaentry/Remake">
    <rdfs:subClassOf rdf:resource="http://www.w3.org/ns/prov#EntityInfluence"/>
    <rdf:type rdf:resource="http://www.w3.org/2002/07/owl#Class"/>
    <rdfs:label xml:lang="en">Remake</rdfs:label>
    <rdfs:comment xml:lang="en">A class representing the influence a work of art may have on another one when the latter is a remake of the former one.</rdfs:comment>
  </rdf:Description>
  <rdf:Description rdf:about="http://purl.org/emmedi/oaentry/role-attribution">
    <rdf:type rdf:resource="http://www.w3.org/2002/07/owl#NamedIndividual"/>
  </rdf:Description>
  <rdf:Description rdf:about="http://purl.org/dc/elements/1.1/creator">
    <rdf:type rdf:resource="http://www.w3.org/2002/07/owl#AnnotationProperty"/>
  </rdf:Description>
  <rdf:Description rdf:about="http://purl.org/emmedi/oaentry/PartialMold">
    <rdf:type rdf:resource="http://www.w3.org/2002/07/owl#Class"/>
    <rdfs:subClassOf rdf:resource="http://www.w3.org/ns/prov#EntityInfluence"/>
    <rdfs:label xml:lang="en">Partial mold</rdfs:label>
    <rdfs:comment xml:lang="en">A class representing the influence a work of art may have on another one when the former is a partial mold of the latter one.</rdfs:comment>
  </rdf:Description>
  <rdf:Description rdf:about="http://purl.org/emmedi/oaentry/Fake">
    <rdfs:subClassOf rdf:resource="http://www.w3.org/ns/prov#EntityInfluence"/>
    <rdfs:label xml:lang="en">Fake</rdfs:label>
    <rdf:type rdf:resource="http://www.w3.org/2002/07/owl#Class"/>
    <rdfs:comment xml:lang="en">A class representing the influence a work of art may have on another one when the latter is considered a fake of the former one.</rdfs:comment>
  </rdf:Description>
  <rdf:Description rdf:about="http://purl.org/emmedi/oaentry/describes">
    <rdfs:range rdf:nodeID="Ne51ca3abd6bb4e4686b640a9aff3bde3"/>
    <rdf:type rdf:resource="http://www.w3.org/2002/07/owl#ObjectProperty"/>
    <rdfs:domain rdf:resource="http://purl.org/emmedi/oaentry/OAEntry"/>
  </rdf:Description>
  <rdf:Description rdf:about="http://purl.org/emmedi/oaentry/isDescribedBy">
    <owl:inverseOf rdf:resource="http://purl.org/emmedi/oaentry/describes"/>
    <rdf:type rdf:resource="http://www.w3.org/2002/07/owl#ObjectProperty"/>
  </rdf:Description>
  <rdf:Description rdf:about="http://purl.org/emmedi/oaentry/inlayer">
    <rdf:type rdf:resource="http://www.w3.org/2002/07/owl#NamedIndividual"/>
    <rdfs:label xml:lang="en">inlayer</rdfs:label>
    <rdfs:comment xml:lang="en">The role of a person who puts decorative patterns into the surface of an object.</rdfs:comment>
    <rdf:type rdf:resource="http://purl.org/emmedi/oaentry/ArtisticRole"/>
  </rdf:Description>
  <rdf:Description rdf:about="http://purl.org/emmedi/oaentry/PartialCartoon">
    <rdfs:label xml:lang="en">Partial cartoon</rdfs:label>
    <rdf:type rdf:resource="http://www.w3.org/2002/07/owl#Class"/>
    <rdfs:subClassOf rdf:resource="http://www.w3.org/ns/prov#EntityInfluence"/>
    <rdfs:comment xml:lang="en">A class representing the influence a work of art may have on another one when the former is a partial cartoon of the latter one.</rdfs:comment>
  </rdf:Description>
  <rdf:Description rdf:about="http://purl.org/emmedi/oaentry/PartialReplica">
    <rdfs:comment xml:lang="en">A class representing the influence a work of art may have on another one when the latter is a partial replica of the former one.</rdfs:comment>
    <rdfs:label xml:lang="en">Partial replica</rdfs:label>
    <rdfs:subClassOf rdf:resource="http://www.w3.org/ns/prov#EntityInfluence"/>
    <rdf:type rdf:resource="http://www.w3.org/2002/07/owl#Class"/>
  </rdf:Description>
  <rdf:Description rdf:about="http://purl.org/emmedi/oaentry/goldsmith">
    <rdf:type rdf:resource="http://www.w3.org/2002/07/owl#NamedIndividual"/>
    <rdfs:label xml:lang="en">goldsmith</rdfs:label>
    <rdfs:comment xml:lang="en">The role of a person who makes objects from gold.</rdfs:comment>
    <rdf:type rdf:resource="http://purl.org/emmedi/oaentry/ArtisticRole"/>
  </rdf:Description>
  <rdf:Description rdf:about="http://purl.org/emmedi/oaentry/inventor">
    <rdf:type rdf:resource="http://purl.org/emmedi/oaentry/ArtisticRole"/>
    <rdf:type rdf:resource="http://www.w3.org/2002/07/owl#NamedIndividual"/>
    <rdfs:comment xml:lang="en">The role of a person who produces or contrives something. </rdfs:comment>
    <rdfs:label xml:lang="en">inventor</rdfs:label>
  </rdf:Description>
  <rdf:Description rdf:nodeID="Ne51ca3abd6bb4e4686b640a9aff3bde3">
    <owl:unionOf rdf:nodeID="N6c53906619c141018ff3d02f0f951fe5"/>
    <rdf:type rdf:resource="http://www.w3.org/2002/07/owl#Class"/>
  </rdf:Description>
  <rdf:Description rdf:about="http://purl.org/emmedi/oaentry/restorer">
    <rdf:type rdf:resource="http://www.w3.org/2002/07/owl#NamedIndividual"/>
    <rdf:type rdf:resource="http://purl.org/emmedi/oaentry/ArtisticRole"/>
    <rdfs:comment xml:lang="en">The role of a person who restores buildings, furniture, or paintings to thier original condition.</rdfs:comment>
    <rdfs:label xml:lang="en">restorer</rdfs:label>
  </rdf:Description>
  <rdf:Description rdf:about="http://purl.org/emmedi/oaentry/Prototype">
    <rdfs:comment xml:lang="en">A class representing the influence a work of art may have on another one when the former is a prototype of the latter one.</rdfs:comment>
    <rdfs:subClassOf rdf:resource="http://www.w3.org/ns/prov#EntityInfluence"/>
    <rdf:type rdf:resource="http://www.w3.org/2002/07/owl#Class"/>
    <rdfs:label xml:lang="en">Prototype</rdfs:label>
  </rdf:Description>
  <rdf:Description rdf:about="http://purl.org/emmedi/oaentry/SpecularCopy">
    <rdfs:subClassOf rdf:resource="http://purl.org/emmedi/oaentry/Copy"/>
    <rdfs:comment xml:lang="en">A class representing the influence a work of art may have on another one when the latter is considered a specular copy of the former one.</rdfs:comment>
    <rdf:type rdf:resource="http://www.w3.org/2002/07/owl#Class"/>
    <rdfs:label xml:lang="en">Specular copy</rdfs:label>
  </rdf:Description>
  <rdf:Description rdf:about="http://purl.org/emmedi/oaentry/cataloguing-institution">
    <rdf:type rdf:resource="http://www.w3.org/2002/07/owl#NamedIndividual"/>
    <rdfs:label xml:lang="en">cataloguing institution</rdfs:label>
    <rdfs:comment xml:lang="en">The role held by the responsible corporate body with respect to the catalogued cultural heritage object.</rdfs:comment>
    <rdf:type rdf:resource="http://purl.org/emmedi/oaentry/CataloguingRole"/>
  </rdf:Description>
  <rdf:Description rdf:about="http://purl.org/dc/terms/date">
    <rdf:type rdf:resource="http://www.w3.org/2002/07/owl#AnnotationProperty"/>
  </rdf:Description>
  <rdf:Description rdf:about="http://purl.org/emmedi/oaentry/carver">
    <rdf:type rdf:resource="http://www.w3.org/2002/07/owl#NamedIndividual"/>
    <rdfs:label xml:lang="en">carver</rdfs:label>
    <rdf:type rdf:resource="http://purl.org/emmedi/oaentry/ArtisticRole"/>
    <rdfs:comment xml:lang="en">The role of a person who carves wood.</rdfs:comment>
  </rdf:Description>
  <rdf:Description rdf:about="http://purl.org/emmedi/oaentry/mosaicist">
    <rdf:type rdf:resource="http://www.w3.org/2002/07/owl#NamedIndividual"/>
    <rdf:type rdf:resource="http://purl.org/emmedi/oaentry/ArtisticRole"/>
    <rdfs:comment xml:lang="en">The role of a person who creates pictures by using small pieces of coloured stones or glass.</rdfs:comment>
    <rdfs:label xml:lang="en">mosaicist</rdfs:label>
  </rdf:Description>
  <rdf:Description rdf:about="http://purl.org/emmedi/oaentry/carving-master">
    <rdf:type rdf:resource="http://purl.org/emmedi/oaentry/ArtisticRole"/>
    <rdfs:comment xml:lang="en">The role of a person expert in carving.</rdfs:comment>
    <rdfs:label xml:lang="en">carving master</rdfs:label>
    <rdf:type rdf:resource="http://www.w3.org/2002/07/owl#NamedIndividual"/>
  </rdf:Description>
  <rdf:Description rdf:about="http://purl.org/emmedi/oaentry/Matrix">
    <rdfs:label xml:lang="en">Matrix</rdfs:label>
    <rdf:type rdf:resource="http://www.w3.org/2002/07/owl#Class"/>
    <rdfs:subClassOf rdf:resource="http://purl.org/emmedi/oaentry/PartialMatrix"/>
    <rdfs:comment xml:lang="en">A class representing the influence a work of art may have on another one when the former is a matrix of the latter one.</rdfs:comment>
  </rdf:Description>
  <rdf:Description rdf:about="http://purl.org/emmedi/oaentry/authorship-attribution">
    <rdf:type rdf:resource="http://purl.org/emmedi/hico/InterpretationType"/>
    <rdf:type rdf:resource="http://www.w3.org/2002/07/owl#NamedIndividual"/>
  </rdf:Description>
</rdf:RDF>
